<?xml version="1.0" encoding="UTF-8"?>
<!DOCTYPE rdf:RDF [
  <!ENTITY Government "http://reliant.teknowledge.com/DAML/Government.owl#">
  <!ENTITY Mid-level-ontology "http://reliant.teknowledge.com/DAML/Mid-level-ontology.owl#">
  <!ENTITY SUMO "http://reliant.teknowledge.com/DAML/SUMO.owl#">
  <!ENTITY Transportation "http://reliant.teknowledge.com/DAML/Transportation.owl#">
  <!ENTITY Transportation.owl "http://reliant.teknowledge.com/DAML/Transportation.owl">
  <!ENTITY owl "http://www.w3.org/2002/07/owl#">
  <!ENTITY rdf "http://www.w3.org/1999/02/22-rdf-syntax-ns#">
  <!ENTITY rdfs "http://www.w3.org/2000/01/rdf-schema#">
  <!ENTITY xsd "http://www.w3.org/2001/XMLSchema#">
]>
<rdf:RDF xml:base="&Transportation.owl;"
         xmlns:Government="&Government;"
         xmlns:Mid-level-ontology="&Mid-level-ontology;"
         xmlns:SUMO="&SUMO;"
         xmlns:Transportation="&Transportation;"
         xmlns:owl="&owl;"
         xmlns:rdf="&rdf;"
         xmlns:rdfs="&rdfs;">

<!-- Ontology Information -->
  <owl:Ontology rdf:about=""/>

<!-- Classes -->
  <owl:Class rdf:about="#AidToNavigation">
    <rdfs:comment>AidToNavigation is the subclass of 

TransportationControlDevices that are designed for guiding Ships or 

Aircraft in finding their location or avoiding hazards.  There are 

several systems of Navigation in use, depending upon GeographicArea.</rdfs:comment>
    <rdfs:subClassOf rdf:resource="#TransportationControlDevice"/>
    <rdfs:subClassOf rdf:resource="&SUMO;ContentBearingObject"/>
    <owl:disjointWith rdf:resource="#BillOfLading"/>
    <owl:disjointWith rdf:resource="#CargoManifest"/>
    <owl:disjointWith rdf:resource="#CertificateOfRegistry"/>
    <owl:disjointWith rdf:resource="#CrewList"/>
    <owl:disjointWith rdf:resource="#ShipRegister"/>
    <owl:disjointWith rdf:resource="#TransportationSchedule"/>
    <owl:disjointWith rdf:resource="#VehicleRegistration"/>
  </owl:Class>

  <owl:Class rdf:about="#AirRoute">
    <rdfs:comment>AirRoute is the subclass of AirTransitways 

that are officially recognized by some authority, civilian or military, 

and which are formally designated by name, headings, boundaries, or 

waypoints for use by an Aircraft; for example, commercial air routes or 

military designated air corridors.</rdfs:comment>
    <rdfs:subClassOf rdf:resource="#AirTransitway"/>
    <rdfs:subClassOf rdf:resource="#TransitRoute"/>
    <owl:disjointWith rdf:resource="#Heliport"/>
    <owl:disjointWith rdf:resource="&Mid-level-ontology;Airport"/>
  </owl:Class>

  <owl:Class rdf:about="#AirTrafficControlCenter">
    <rdfs:comment>AirTrafficControlCenter is the 

subclass of Organizations whose principal members are Air Traffic 

Controllers.</rdfs:comment>
    <rdfs:subClassOf rdf:resource="&SUMO;Organization"/>
  </owl:Class>

  <owl:Class rdf:about="#AirTrafficControlEnRouteCenter">
    <rdfs:comment>AirTrafficControlEnRouteCenter is the subclass of 

AirTrafficControlCenters that control traffic between airports and 

at or above 17,000 feet.  In the U.S., ATC en route centers are not located 

at the airports but in one of two dozen centers across the country.</rdfs:comment>
    <rdfs:subClassOf rdf:resource="#AirTrafficControlCenter"/>
  </owl:Class>

  <owl:Class rdf:about="#AirTrafficControlProcedure">
    <rdfs:comment>AirTrafficControlProcedure is 

the subclass of TrafficControlProcesses directed at controlling the 

movement of Aircraft.</rdfs:comment>
    <rdfs:subClassOf rdf:resource="#TrafficControlProcess"/>
  </owl:Class>

  <owl:Class rdf:about="#AirTrafficControlRadarRoom">
    <rdfs:comment>AirTrafficControlRadarRoom 

is the subclass of AirTrafficControlCenters in which 

AirTrafficControllers work at Radar.</rdfs:comment>
    <rdfs:subClassOf rdf:resource="#AirTrafficControlCenter"/>
    <rdfs:subClassOf rdf:resource="#RadarFacility"/>
  </owl:Class>

  <owl:Class rdf:about="#AirTrafficControlTower">
    <rdfs:comment>AirTrafficControlTower is the 

subclass of AirTrafficControlCenters that are located at Airports.</rdfs:comment>
    <rdfs:subClassOf rdf:resource="#AirTrafficControlCenter"/>
  </owl:Class>

  <Transportation:ModeOfTransit rdf:about="#AirTransitway">
    <rdf:type rdf:resource="&owl;Class"/>
    <rdfs:comment>AirTransitway is the subclass of 

Transitways through the medium of air.  If an area is an 

AirTransitway, then some kind of Aircraft can travel through that 

airspace.</rdfs:comment>
    <rdfs:subClassOf rdf:resource="&Mid-level-ontology;AtmosphericRegion"/>
    <rdfs:subClassOf rdf:resource="&SUMO;Transitway"/>
    <owl:disjointWith rdf:resource="#OneWayTransitway"/>
    <owl:disjointWith rdf:resource="#SingleTrafficLane"/>
    <owl:disjointWith rdf:resource="#TransitRoute"/>
    <owl:disjointWith rdf:resource="&Mid-level-ontology;Pipeline"/>
    <owl:disjointWith rdf:resource="&Mid-level-ontology;TransitwayJunction"/>
    <owl:disjointWith rdf:resource="&Mid-level-ontology;Tunnel"/>
    <owl:disjointWith rdf:resource="&Mid-level-ontology;Waterway"/>
    <owl:disjointWith rdf:resource="&SUMO;LandTransitway"/>
  </Transportation:ModeOfTransit>

  <owl:Class rdf:about="#AirportByRunwaySurface">
    <rdfs:comment>AirportByRunwaySurface is a 

subclass of AirportClassification attributes used to describe an 

airport according to the surface type of its longest runway.</rdfs:comment>
    <rdfs:subClassOf rdf:resource="#AirportClassification"/>
    <owl:disjointWith rdf:resource="#CIAAirportLengthClassification"/>
  </owl:Class>

  <owl:Class rdf:about="#AirportClassification">
    <rdfs:comment>AirportClassification 

is a class of Attributes for representing systems that categorize 

Airports according to some criteria.  There are several such systems, 

including the International Civil Aviation Organization categories A to 

E, based on runway lengths; the Federal Aviation Administration system 

associated with airport functions, and the airport categorization by 

runway length used in the CIA World Fact Book.</rdfs:comment>
    <rdfs:subClassOf rdf:resource="&SUMO;Attribute"/>
    <owl:disjointWith rdf:resource="&Mid-level-ontology;DeviceStateAttribute"/>
  </owl:Class>

  <owl:Class rdf:about="#Ambulance">
    <rdfs:comment>Ambulance is the subclass of 

EmergencyRoadVehicles that represents ambulances.</rdfs:comment>
    <rdfs:subClassOf rdf:resource="#EmergencyRoadVehicle"/>
  </owl:Class>

  <owl:Class rdf:about="#Anchorage">
    <rdfs:comment>Anchorage is the subclass of WaterAreas 

where Watercraft may anchor with some shelter or safety.  Anchorages 

may be inside a Harbor or offshore.</rdfs:comment>
    <rdfs:subClassOf rdf:resource="&SUMO;WaterArea"/>
    <owl:disjointWith rdf:resource="#DeepDraftWaterArea"/>
    <owl:disjointWith rdf:resource="#Harbor"/>
    <owl:disjointWith rdf:resource="#ShipBerth"/>
    <owl:disjointWith rdf:resource="&Mid-level-ontology;Waterway"/>
  </owl:Class>

  <owl:Class rdf:about="#AnimalPoweredVehicle">
    <rdfs:comment>AnimalPoweredVehicle is the 

subclass of Vehicles whose motive power is provided by an animal or 

animals.  Examples: horse-drawn carriages, oxcarts, pony carts.</rdfs:comment>
    <rdfs:subClassOf rdf:resource="&Mid-level-ontology;AnimalPoweredDevice"/>
    <rdfs:subClassOf rdf:resource="&SUMO;Vehicle"/>
  </owl:Class>

  <owl:Class rdf:about="#Axle">
    <rdfs:comment>Axle is a class of Devices each of which can 

be paired with two VehicleWheels to rotate and move a RoadVehicle.</rdfs:comment>
    <rdfs:subClassOf rdf:resource="&SUMO;Device"/>
    <owl:disjointWith rdf:resource="#CanalLockGate"/>
    <owl:disjointWith rdf:resource="#Drawbridge"/>
    <owl:disjointWith rdf:resource="#HumanPoweredDevice"/>
    <owl:disjointWith rdf:resource="#TransportationControlDevice"/>
    <owl:disjointWith rdf:resource="#VehicleWheel"/>
    <owl:disjointWith rdf:resource="#WindPoweredDevice"/>
    <owl:disjointWith rdf:resource="&Mid-level-ontology;AnimalPoweredDevice"/>
    <owl:disjointWith rdf:resource="&Mid-level-ontology;Battery"/>
    <owl:disjointWith rdf:resource="&Mid-level-ontology;HoistingDevice"/>
    <owl:disjointWith rdf:resource="&Mid-level-ontology;MaterialHandlingEquipment"/>
    <owl:disjointWith rdf:resource="&Mid-level-ontology;UserPoweredDevice"/>
  </owl:Class>

  <owl:Class rdf:about="#Barge">
    <rdfs:comment>Barge is the subclass of flat-bottomed, 

shallow-draft vessels designed to carry cargo on inland waterways. 

Barges are generally not self-powered and rely on Tugboats for 

transportion.</rdfs:comment>
    <rdfs:subClassOf rdf:resource="&Mid-level-ontology;Watercraft"/>
  </owl:Class>

  <owl:Class rdf:about="#BargeCarrierShip"
             rdfs:label="Lighter Aboard Ship">
    <rdfs:comment>BargeCarrierShip is a subclass of 

Ships that are oceangoing vessels designed to carry barges, which are 

lifted aboard.  They may also be designed to carry some CargoContainers.</rdfs:comment>
    <rdfs:subClassOf rdf:resource="#CargoShip"/>
    <rdfs:subClassOf rdf:resource="#Freighter"/>
  </owl:Class>

  <owl:Class rdf:about="#Bicycle">
    <rdfs:comment>Bicycle is a class of two-wheeled, 

UserPoweredVehicles.</rdfs:comment>
    <rdfs:subClassOf rdf:resource="#Cycle-TransportationDevice"/>
    <rdfs:subClassOf rdf:resource="&Mid-level-ontology;Cycle"/>
  </owl:Class>

  <owl:Class rdf:about="#BillOfLading">
    <rdfs:comment>BillOfLading is the subclass of 

ContentBearingObjects which are shipping records recording the 

consignment of specified goods by one agent to another for the purpose of 

Shipping them to a specified destination.  A BillOfLading is a document 

listing the goods, consignee, carrier, destination, and the rate charged 

for freight.  In the case of Shipping aboard a Ship, the names of the 

ship, port, and the ShipMaster will be included in the bill of lading.</rdfs:comment>
    <rdfs:subClassOf rdf:resource="&SUMO;ContentBearingObject"/>
    <owl:disjointWith rdf:resource="#AidToNavigation"/>
    <owl:disjointWith rdf:resource="#CargoManifest"/>
    <owl:disjointWith rdf:resource="#CertificateOfRegistry"/>
    <owl:disjointWith rdf:resource="#CrewList"/>
    <owl:disjointWith rdf:resource="#ShipRegister"/>
    <owl:disjointWith rdf:resource="#TransportationSchedule"/>
    <owl:disjointWith rdf:resource="#VehicleRegistration"/>
  </owl:Class>

  <owl:Class rdf:about="#Boxcar">
    <rdfs:comment>Boxcar is the subclass of Railcars that are 

general-purpose closed cars for hauling freight.</rdfs:comment>
    <rdfs:subClassOf rdf:resource="#FreightCar"/>
  </owl:Class>

  <owl:Class rdf:about="#BroadGaugeRailway">
    <rdfs:comment>BroadGaugeRailway is the class of 

Railway that has a distance greater than 1.44 Meters between its 

rails.</rdfs:comment>
    <rdfs:subClassOf rdf:resource="&Mid-level-ontology;Railway"/>
  </owl:Class>

  <owl:Class rdf:about="#BulkCargo">
    <rdfs:comment>BulkCargo is the subclass of shipped goods 

that are homogeneous in nature, liquid or dry, and are shipped in a 

loose, uncontainerized form in the holds of a CargoShip.</rdfs:comment>
    <rdfs:subClassOf rdf:resource="&SUMO;Substance"/>
  </owl:Class>

  <owl:Class rdf:about="#Bulkhead">
    <rdfs:comment>Bulkhead is a class of vertical walls or 

partitions within a Vehicle that prevent cargo from shifting during 

transit.  On a ship, Bulkheads may form the walls of a ShipCompartment.</rdfs:comment>
    <rdfs:subClassOf rdf:resource="&SUMO;StationaryArtifact"/>
    <owl:disjointWith rdf:resource="#CanalLock"/>
    <owl:disjointWith rdf:resource="#CanalStructure"/>
    <owl:disjointWith rdf:resource="#Pier"/>
    <owl:disjointWith rdf:resource="&Mid-level-ontology;Bridge"/>
    <owl:disjointWith rdf:resource="&Mid-level-ontology;RailroadTrack"/>
    <owl:disjointWith rdf:resource="&Mid-level-ontology;Railway"/>
    <owl:disjointWith rdf:resource="&Mid-level-ontology;TransitTerminal"/>
    <owl:disjointWith rdf:resource="&Mid-level-ontology;Tunnel"/>
  </owl:Class>

  <owl:Class rdf:about="#Bus">
    <rdfs:comment>Bus is the subclass of SelfPoweredRoadVehicles 

that can transport large numbers of passengers (i.e., dozens) at one 

time.</rdfs:comment>
    <rdfs:subClassOf rdf:resource="#FHWAVehicleClass4"/>
    <rdfs:subClassOf rdf:resource="#SelfPoweredRoadVehicle"/>
    <owl:disjointWith rdf:resource="&Mid-level-ontology;Automobile"/>
  </owl:Class>

  <owl:Class rdf:about="#BusinessRailcar">
    <rdfs:comment>BusinessRailcar is the subclass of 

PassengerRailCars that are reserved by a railway company for use of 

its own employees while travelling on business purposes.</rdfs:comment>
    <rdfs:subClassOf rdf:resource="#PassengerRailwayCar"/>
    <rdfs:subClassOf rdf:resource="#Railcar"/>
  </owl:Class>

  <owl:Class rdf:about="#CIAAirportLengthClassification">
    <rdfs:comment>CIAAirportLengthClassification is a class of Attributes used to 

characterize Airports according to the length of their longest  

usable runway.</rdfs:comment>
    <rdfs:subClassOf rdf:resource="#AirportClassification"/>
    <owl:disjointWith rdf:resource="#AirportByRunwaySurface"/>
  </owl:Class>

  <owl:Class rdf:about="#CabCar">
    <rdfs:comment>CabCar is the class of powered passenger cars  

that have an operating cab in one end from which train motion can be 

controlled in 'push' mode.  A CabCar is placed on the opposite end of 

the train from the locomotive.</rdfs:comment>
    <rdfs:subClassOf rdf:resource="#PassengerRailwayCar"/>
    <rdfs:subClassOf rdf:resource="#SelfPoweredVehicle"/>
    <owl:disjointWith rdf:resource="#ElectrifiedRailwayCar"/>
    <owl:disjointWith rdf:resource="&Mid-level-ontology;Airplane"/>
  </owl:Class>

  <owl:Class rdf:about="#CableShip">
    <rdfs:subClassOf rdf:resource="&Mid-level-ontology;Ship"/>
    <owl:disjointWith rdf:resource="#CargoShip"/>
    <owl:disjointWith rdf:resource="#CraneShip"/>
    <owl:disjointWith rdf:resource="#Dredger"/>
    <owl:disjointWith rdf:resource="#DrillingShip"/>
    <owl:disjointWith rdf:resource="#IceBreakerShip"/>
    <owl:disjointWith rdf:resource="#MerchantMarineShip"/>
    <owl:disjointWith rdf:resource="#MotorHopper"/>
    <owl:disjointWith rdf:resource="#OffshoreSupplyShip"/>
    <owl:disjointWith rdf:resource="#OffshoreSupportShip"/>
    <owl:disjointWith rdf:resource="#OffshoreWellProductionShip"/>
    <owl:disjointWith rdf:resource="#PassengerShip"/>
    <owl:disjointWith rdf:resource="#ResearchShip"/>
    <owl:disjointWith rdf:resource="#SludgeDisposalVessel"/>
  </owl:Class>

  <owl:Class rdf:about="#Cabotage">
    <rdfs:comment>Cabotage is the subclass of Transportation 

events that are commercial shipping of cargo or passengers conducted 

between Ports within the same Nation.</rdfs:comment>
    <rdfs:subClassOf rdf:resource="&SUMO;Transportation"/>
  </owl:Class>

  <owl:Class rdf:about="#CanalLock">
    <rdfs:comment>CanalLock is the subclass of Artifacts  

that are built along a Canal, in order to raise and lower vessels 

as required along the canal route.</rdfs:comment>
    <rdfs:subClassOf rdf:resource="&SUMO;StationaryArtifact"/>
    <owl:disjointWith rdf:resource="#Bulkhead"/>
    <owl:disjointWith rdf:resource="#CanalStructure"/>
    <owl:disjointWith rdf:resource="#Pier"/>
    <owl:disjointWith rdf:resource="&Mid-level-ontology;Bridge"/>
    <owl:disjointWith rdf:resource="&Mid-level-ontology;RailroadTrack"/>
    <owl:disjointWith rdf:resource="&Mid-level-ontology;Railway"/>
    <owl:disjointWith rdf:resource="&Mid-level-ontology;TransitTerminal"/>
    <owl:disjointWith rdf:resource="&Mid-level-ontology;Tunnel"/>
  </owl:Class>

  <owl:Class rdf:about="#CanalLockGate">
    <rdfs:subClassOf rdf:resource="#TransitwayObstacle"/>
    <rdfs:subClassOf rdf:resource="&SUMO;Device"/>
    <owl:disjointWith rdf:resource="#Axle"/>
    <owl:disjointWith rdf:resource="#Drawbridge"/>
    <owl:disjointWith rdf:resource="#HumanPoweredDevice"/>
    <owl:disjointWith rdf:resource="#TransportationControlDevice"/>
    <owl:disjointWith rdf:resource="#VehicleWheel"/>
    <owl:disjointWith rdf:resource="#WindPoweredDevice"/>
    <owl:disjointWith rdf:resource="&Mid-level-ontology;AnimalPoweredDevice"/>
    <owl:disjointWith rdf:resource="&Mid-level-ontology;Battery"/>
    <owl:disjointWith rdf:resource="&Mid-level-ontology;HoistingDevice"/>
    <owl:disjointWith rdf:resource="&Mid-level-ontology;MaterialHandlingEquipment"/>
    <owl:disjointWith rdf:resource="&Mid-level-ontology;UserPoweredDevice"/>
  </owl:Class>

  <owl:Class rdf:about="#CanalStructure">
    <rdfs:comment>CanalStructure is the subclass of 

StationaryArtifacts consisting of the constructed framework, including 

CanalLocks (if any), that contains the waters of a Canal.</rdfs:comment>
    <rdfs:subClassOf rdf:resource="&SUMO;StationaryArtifact"/>
    <owl:disjointWith rdf:resource="#Bulkhead"/>
    <owl:disjointWith rdf:resource="#CanalLock"/>
    <owl:disjointWith rdf:resource="#Pier"/>
    <owl:disjointWith rdf:resource="&Mid-level-ontology;Bridge"/>
    <owl:disjointWith rdf:resource="&Mid-level-ontology;RailroadTrack"/>
    <owl:disjointWith rdf:resource="&Mid-level-ontology;Railway"/>
    <owl:disjointWith rdf:resource="&Mid-level-ontology;TransitTerminal"/>
    <owl:disjointWith rdf:resource="&Mid-level-ontology;Tunnel"/>
  </owl:Class>

  <owl:Class rdf:about="#CanalSystem">
    <rdfs:comment>CanalSystem is the subclass of 

WaterTransportationSystems with substantial parts consisting of 

Canals, linked by connecting Waterways.</rdfs:comment>
    <rdfs:subClassOf rdf:resource="#WaterTransportationSystem"/>
  </owl:Class>

  <owl:Class rdf:about="#Canoe">
    <rdfs:subClassOf rdf:resource="#HumanPoweredDevice"/>
    <rdfs:subClassOf rdf:resource="&Mid-level-ontology;Watercraft"/>
    <owl:disjointWith rdf:resource="#Kayak"/>
  </owl:Class>

  <owl:Class rdf:about="#CarDistributionSystem">
    <rdfs:comment>CarDistributionSystem is the 

overall process of routing railway cars and composing trains according to 

policy and instructions.</rdfs:comment>
    <rdfs:subClassOf rdf:resource="&SUMO;Managing"/>
  </owl:Class>

  <owl:Class rdf:about="#CargoContainer">
    <rdfs:comment>CargoContainer is the class of specialized 

large containers designed for shipping goods aboard ContainerShips.  Some 

containers are sized for transfer to Trains or TruckTrailers.</rdfs:comment>
    <rdfs:subClassOf rdf:resource="&Mid-level-ontology;Container"/>
    <rdfs:subClassOf rdf:resource="&SUMO;TransportationDevice"/>
    <owl:disjointWith rdf:resource="#FuelTank"/>
    <owl:disjointWith rdf:resource="#TankCar"/>
    <owl:disjointWith rdf:resource="&Mid-level-ontology;Aircraft"/>
    <owl:disjointWith rdf:resource="&Mid-level-ontology;Crane"/>
    <owl:disjointWith rdf:resource="&Mid-level-ontology;RefrigeratedCompartment"/>
    <owl:disjointWith rdf:resource="&Mid-level-ontology;SelfPoweredDevice"/>
    <owl:disjointWith rdf:resource="&Mid-level-ontology;Watercraft"/>
    <owl:disjointWith rdf:resource="&SUMO;Vehicle"/>
  </owl:Class>

  <owl:Class rdf:about="#CargoHandling">
    <rdfs:comment>CargoHandling is the subclass of 

Transportation that involves loading freight on and off a CargoShip.</rdfs:comment>
    <rdfs:subClassOf rdf:resource="&SUMO;Transportation"/>
  </owl:Class>

  <owl:Class rdf:about="#CargoManifest">
    <rdfs:comment>CargoManifest is the subclass of 

ContentBearingObjects that list all the cargo carried during an 

individual Shipping event.</rdfs:comment>
    <rdfs:subClassOf rdf:resource="&SUMO;ContentBearingObject"/>
    <owl:disjointWith rdf:resource="#AidToNavigation"/>
    <owl:disjointWith rdf:resource="#BillOfLading"/>
    <owl:disjointWith rdf:resource="#CertificateOfRegistry"/>
    <owl:disjointWith rdf:resource="#CrewList"/>
    <owl:disjointWith rdf:resource="#ShipRegister"/>
    <owl:disjointWith rdf:resource="#TransportationSchedule"/>
    <owl:disjointWith rdf:resource="#VehicleRegistration"/>
  </owl:Class>

  <owl:Class rdf:about="#CargoShip">
    <rdfs:comment>CargoShip is the subclass of Ships that 

transport goods in exchange for payment.  CargoShip includes ships 

that carry all kinds of cargo, including oil and bulk products as well 

as packaged, palletized, or containerized goods.</rdfs:comment>
    <rdfs:label>breakbulk carrier</rdfs:label>
    <rdfs:label>breakbulk ship</rdfs:label>
    <rdfs:label>cargo ship</rdfs:label>
    <rdfs:label>general cargo ship</rdfs:label>
    <rdfs:subClassOf rdf:resource="&Mid-level-ontology;Ship"/>
    <owl:disjointWith rdf:resource="#CableShip"/>
    <owl:disjointWith rdf:resource="#CraneShip"/>
    <owl:disjointWith rdf:resource="#Dredger"/>
    <owl:disjointWith rdf:resource="#DrillingShip"/>
    <owl:disjointWith rdf:resource="#IceBreakerShip"/>
    <owl:disjointWith rdf:resource="#MerchantMarineShip"/>
    <owl:disjointWith rdf:resource="#OffshoreSupplyShip"/>
    <owl:disjointWith rdf:resource="#OffshoreSupportShip"/>
    <owl:disjointWith rdf:resource="#OffshoreWellProductionShip"/>
    <owl:disjointWith rdf:resource="#PassengerShip"/>
    <owl:disjointWith rdf:resource="#ResearchShip"/>
    <owl:disjointWith rdf:resource="#SludgeDisposalVessel"/>
  </owl:Class>

  <owl:Class rdf:about="#Catamaran">
    <rdfs:comment>Catamaran is the subclass of 

PlaningHullWatercraft that have two or more hulls connected by a 

ShipDeck or other superstructure.</rdfs:comment>
    <rdfs:subClassOf rdf:resource="#PlaningHullWatercraft"/>
  </owl:Class>

  <owl:Class rdf:about="#CementCarrierShip">
    <rdfs:comment>CementCarrierShip is the subclass of 

CargoShips that carry Cement.</rdfs:comment>
    <rdfs:subClassOf rdf:resource="#DryBulkCarrierShip"/>
  </owl:Class>

  <owl:Class rdf:about="#CertificateOfRegistry">
    <rdfs:comment>CertificateOfRegistry is the class 

of all official documents containing information about the ownership, size, 

and flag of registry (flagState) of an individual Ship, as registered 

in a ShipRegister maintained by the maritime authorities of a 

particular Nation or OverseasArea.  A registered vessel flies the 

flag of its registry nation (or area), and the ship is subject to the 

maritime regulations and rules of taxation of that flagState.</rdfs:comment>
    <rdfs:label>certificate of registry</rdfs:label>
    <rdfs:label>ship registration</rdfs:label>
    <rdfs:subClassOf rdf:resource="&SUMO;ContentBearingObject"/>
    <owl:disjointWith rdf:resource="#AidToNavigation"/>
    <owl:disjointWith rdf:resource="#BillOfLading"/>
    <owl:disjointWith rdf:resource="#CargoManifest"/>
    <owl:disjointWith rdf:resource="#CrewList"/>
    <owl:disjointWith rdf:resource="#ShipRegister"/>
    <owl:disjointWith rdf:resource="#TransportationSchedule"/>
    <owl:disjointWith rdf:resource="#VehicleRegistration"/>
  </owl:Class>

  <owl:Class rdf:about="#ChemicalAndPetroleumTankerShip">
    <rdfs:comment>ChemicalAndPetroleumTankerShip is the subclass of ships that can 

carry ChemicalProducts or PetroleumProducts.</rdfs:comment>
    <rdfs:subClassOf rdf:resource="#ChemicalTankerShip"/>
    <rdfs:subClassOf rdf:resource="#PetroleumTankerShip"/>
  </owl:Class>

  <owl:Class rdf:about="#ChemicalTankerShip"
             rdfs:label="chemical carrier">
    <rdfs:comment>ChemicalTankerShip is the 

subclass of ships that carry ChemicalProducts.</rdfs:comment>
    <rdfs:subClassOf rdf:resource="#CargoShip"/>
  </owl:Class>

  <owl:Class rdf:about="#ClassIIIRailroad">
    <rdfs:comment>ClassIIIRailroad is the 

subclass of RailroadCompany whose instances have an 

average annual gross revenue below $20.5 million 

UnitedStatesDollars.</rdfs:comment>
    <rdfs:subClassOf rdf:resource="&Mid-level-ontology;RailroadCompany"/>
    <owl:disjointWith rdf:resource="#ClassIIRailroad"/>
    <owl:disjointWith rdf:resource="#ClassIRailroad"/>
  </owl:Class>

  <owl:Class rdf:about="#ClassIIRailroad">
    <rdfs:comment>ClassIIRailroad is the 

subclass of RailroadCompany whose instances have an 

average annual gross revenue between $20.5 and $256.4 million 

UnitedStatesDollars.</rdfs:comment>
    <rdfs:subClassOf rdf:resource="&Mid-level-ontology;RailroadCompany"/>
    <owl:disjointWith rdf:resource="#ClassIIIRailroad"/>
    <owl:disjointWith rdf:resource="#ClassIRailroad"/>
  </owl:Class>

  <owl:Class rdf:about="#ClassIRailroad">
    <rdfs:comment>ClassIRailroad is the 

subclass of RailroadCompany whose instances have an 

average annual gross revenue above $256.4 million 

UnitedStatesDollars.</rdfs:comment>
    <rdfs:subClassOf rdf:resource="&Mid-level-ontology;RailroadCompany"/>
    <owl:disjointWith rdf:resource="#ClassIIIRailroad"/>
    <owl:disjointWith rdf:resource="#ClassIIRailroad"/>
  </owl:Class>

  <owl:Class rdf:about="#CoachRailcar">
    <rdfs:comment>CoachRailcar is the subclass of Railcars 

that are designed for seated transportation of paid passengers.</rdfs:comment>
    <rdfs:subClassOf rdf:resource="#PassengerRailwayCar"/>
    <rdfs:subClassOf rdf:resource="#Railcar"/>
  </owl:Class>

  <owl:Class rdf:about="#CombinationBulkAndOilCarrierShip">
    <rdfs:comment>CombinationBulkAndOilCarrierShip is the subclass of 

CombinationCarrierShips that are designed to carry both bulk cargo 

and oil.</rdfs:comment>
    <rdfs:comment>CombinationBulkAndOilCarrierShip is the subclass of 

CombinationCarrierShips that are designed to carry both ore and oil.</rdfs:comment>
    <rdfs:subClassOf rdf:resource="#CombinationCarrierShip"/>
  </owl:Class>

  <owl:Class rdf:about="#CombinationCarrierShip">
    <SUMO:disjoint rdf:resource="#ContainerShip"/>
    <rdf:type rdf:resource="&owl;Thing"/>
    <rdfs:comment>CombinationCarrierShip 

is the subclass of CargoShips that are designed to carry two 

different types of cargoes.</rdfs:comment>
    <rdfs:label>combination carrier</rdfs:label>
    <rdfs:label>dual purpose ship</rdfs:label>
    <rdfs:subClassOf rdf:resource="#CargoShip"/>
  </owl:Class>

  <owl:Class rdf:about="#CombinationOreAndOilCarrierShip">
    <rdfs:subClassOf rdf:resource="#CombinationCarrierShip"/>
  </owl:Class>

  <owl:Class rdf:about="#CommercialAirport">
    <rdfs:comment>CommercialAirport is the subclass of 

Airports where commerical air service is offered.</rdfs:comment>
    <rdfs:subClassOf rdf:resource="&Mid-level-ontology;Airport"/>
    <rdfs:subClassOf rdf:resource="&SUMO;CommercialAgent"/>
    <owl:disjointWith rdf:resource="#InternationalAirport"/>
  </owl:Class>

  <owl:Class rdf:about="#CommercialCarrier">
    <rdfs:comment>CommercialCarrier is the subclass of 

TransportationCompany whose instances provide transportation services 

for payment, with the intention of making a profit.</rdfs:comment>
    <rdfs:subClassOf rdf:resource="&Mid-level-ontology;TransportationCompany"/>
  </owl:Class>

  <owl:Class rdf:about="#CommercialShipping">
    <rdfs:comment>CommercialShipping is the subclass of 

Transportation events in which a commercial agent provides transportation 

of goods for remuneration.</rdfs:comment>
    <rdfs:subClassOf rdf:resource="#Shipping"/>
    <rdfs:subClassOf rdf:resource="&SUMO;CommercialService"/>
  </owl:Class>

  <owl:Class rdf:about="#ContainerAndRoRoCargoShip">
    <rdfs:comment>ContainerAndRoRoCargoShip is a 

subclass of CargoShips that are designed for a combination of containers 

and roll-on, roll-off cargo.</rdfs:comment>
    <rdfs:subClassOf rdf:resource="#PartialContainerShip"/>
    <rdfs:subClassOf rdf:resource="#RollOnRollOffCargoShip"/>
  </owl:Class>

  <owl:Class rdf:about="#ContainerHandlingEquipment">
    <rdfs:comment>ContainerHandlingEquipment 

is a class of Devices that are equipment used for loading and 

unloading CargoContainers on ContainerShips or other transportation 

devices.</rdfs:comment>
    <rdfs:subClassOf rdf:resource="&Mid-level-ontology;MaterialHandlingEquipment"/>
  </owl:Class>

  <owl:Class rdf:about="#ContainerShip">
    <rdf:type rdf:resource="&owl;Thing"/>
    <rdfs:comment>ContainerShip is the subclass of 

CargoShips that are designed for transporting CargoContainers.</rdfs:comment>
    <rdfs:subClassOf rdf:resource="#CargoShip"/>
    <rdfs:subClassOf rdf:resource="#Freighter"/>
  </owl:Class>

  <owl:Class rdf:about="#ContainerTerminal">
    <SUMO:relatedInternalConcept rdf:resource="#ContainerShip"/>
    <rdf:type rdf:resource="&owl;Thing"/>
    <rdfs:comment>ContainerTerminal is the subclass 

of PortFacility whose instances have terminals for large 

ContainerShips that transport cargo in containers.  Such facilities 

require equipment to load, unload, and move CargoContainers, as well 

as a waterside location with sufficient waterDepth to be navigable by 

ContainerShips.</rdfs:comment>
    <rdfs:subClassOf rdf:resource="&Mid-level-ontology;PortFacility"/>
  </owl:Class>

  <owl:Class rdf:about="#Containerization">
    <rdfs:comment>Containerization is the subclass of 

end-to-end Transportation processes in which cargo is transported 

from a source to a recipient by means of CargoContainers.</rdfs:comment>
    <rdfs:subClassOf rdf:resource="&SUMO;Transportation"/>
  </owl:Class>

  <owl:Class rdf:about="#CraneShip">
    <rdfs:subClassOf rdf:resource="&Mid-level-ontology;Ship"/>
    <owl:disjointWith rdf:resource="#CableShip"/>
    <owl:disjointWith rdf:resource="#CargoShip"/>
    <owl:disjointWith rdf:resource="#Dredger"/>
    <owl:disjointWith rdf:resource="#DrillingShip"/>
    <owl:disjointWith rdf:resource="#IceBreakerShip"/>
    <owl:disjointWith rdf:resource="#MerchantMarineShip"/>
    <owl:disjointWith rdf:resource="#MotorHopper"/>
    <owl:disjointWith rdf:resource="#OffshoreSupplyShip"/>
    <owl:disjointWith rdf:resource="#OffshoreSupportShip"/>
    <owl:disjointWith rdf:resource="#OffshoreWellProductionShip"/>
    <owl:disjointWith rdf:resource="#PassengerShip"/>
    <owl:disjointWith rdf:resource="#ResearchShip"/>
    <owl:disjointWith rdf:resource="#SludgeDisposalVessel"/>
  </owl:Class>

  <owl:Class rdf:about="#CrewDormCar">
    <rdfs:comment>CrewDormCar is the subclass of Railcars 

that are used for housing the employee staff on long-distance trains.</rdfs:comment>
    <rdfs:subClassOf rdf:resource="#PassengerRailwayCar"/>
    <rdfs:subClassOf rdf:resource="#Railcar"/>
  </owl:Class>

  <owl:Class rdf:about="#CrewList">
    <rdfs:comment>CrewList is the class of ContentBearingObjects 

that contain the name, position, and other information about members of 

a VehicleCrew.</rdfs:comment>
    <rdfs:subClassOf rdf:resource="&SUMO;ContentBearingObject"/>
    <owl:disjointWith rdf:resource="#AidToNavigation"/>
    <owl:disjointWith rdf:resource="#BillOfLading"/>
    <owl:disjointWith rdf:resource="#CargoManifest"/>
    <owl:disjointWith rdf:resource="#CertificateOfRegistry"/>
    <owl:disjointWith rdf:resource="#VehicleRegistration"/>
  </owl:Class>

  <owl:Class rdf:about="#CruiseShip">
    <rdfs:comment>CruiseShip is the subclass of 

PassengerShips designed for the purpose of carrying passengers 

on extended trips and operated by a TransportationCompany.</rdfs:comment>
    <rdfs:subClassOf rdf:resource="#PassengerShip"/>
  </owl:Class>

  <owl:Class rdf:about="#Cycle-TransportationDevice">
    <rdfs:comment>Cycle-TransportationDevice 

is a class of wheeled, pedal-driven UserPoweredVehicles that are 

designed to be ridden on roads or trails.</rdfs:comment>
    <rdfs:subClassOf rdf:resource="&Mid-level-ontology;LandVehicle"/>
    <rdfs:subClassOf rdf:resource="&Mid-level-ontology;UserPoweredDevice"/>
  </owl:Class>

  <owl:Class rdf:about="#DangerousGoods">
    <rdfs:comment>DangerousGoods is a subclass of Object, 

representing hazardous goods that require special handling during 

Transportation.</rdfs:comment>
    <rdfs:subClassOf rdf:resource="&SUMO;Object"/>
  </owl:Class>

  <owl:Class rdf:about="#DeckCargo">
    <rdfs:comment>DeckCargo is a subclass of Object consisting 

of goods that are carried on the deck of a Ship rather than in a cargo 

hold.</rdfs:comment>
    <rdfs:subClassOf rdf:resource="&SUMO;Object"/>
  </owl:Class>

  <owl:Class rdf:about="#DeckCargoShip">
    <rdfs:subClassOf rdf:resource="#GeneralCargoShip"/>
  </owl:Class>

  <owl:Class rdf:about="#DeckCrane">
    <rdfs:comment>DeckCrane is a subclass of Devices that 

are cranes designed and fitted for use on the deck of a Ship.  Deck 

cranes are used for lift-on and lift-off of cargo (LO-LO).</rdfs:comment>
    <rdfs:subClassOf rdf:resource="&Mid-level-ontology;Crane"/>
  </owl:Class>

  <owl:Class rdf:about="#DeepDraftPortCity">
    <rdfs:comment>DeepDraftPortCity is the subclass of 

PortCity that represents any port city having a DeepDraftWaterArea.</rdfs:comment>
    <rdfs:subClassOf rdf:resource="#PortCity"/>
    <owl:disjointWith rdf:resource="#RiverPort"/>
    <owl:disjointWith rdf:resource="#SeaPort"/>
  </owl:Class>

  <owl:Class rdf:about="#DeepDraftWaterArea">
    <rdfs:comment>DeepDraftWaterArea is the subclass 

of WaterAreas that have a waterDepth sufficient to accommodate 

vessels having a draft of at least 45 feet (13.7 meters).  For the 

concept of a deep-water ship terminal located offshore (but on the 

continental shelf), see DeepwaterPort.</rdfs:comment>
    <rdfs:subClassOf rdf:resource="&SUMO;WaterArea"/>
    <owl:disjointWith rdf:resource="#Anchorage"/>
    <owl:disjointWith rdf:resource="#Harbor"/>
    <owl:disjointWith rdf:resource="#ShipBerth"/>
    <owl:disjointWith rdf:resource="&Mid-level-ontology;Waterway"/>
  </owl:Class>

  <owl:Class rdf:about="#DeepwaterPort">
    <rdfs:comment>DeepwaterPort is the subclass of 

PortFacility representing ship terminals meeting the criteria defined in 

33 U.S.C. section 1502(1) as 'any fixed or floating man-made structures 

other than a vessel, or any group of such structures, located beyond the 

territorial sea and off the coast of the United States and which are used 

or intended for use as a port or terminal for the loading or unloading 

and further handling of oil for transportation to any State.... The term 

includes all associated components and equipment including pipelines, 

pumping stations, service platforms, mooring buoys, and similar 

appurtenances to the extent they are located seaward of the high water 

mark.'  Cf. DeepDraftPort and DeepDraftHarbor.</rdfs:comment>
    <rdfs:subClassOf rdf:resource="&Mid-level-ontology;PortFacility"/>
  </owl:Class>

  <owl:Class rdf:about="#DepartmentOfTransportation">
    <rdfs:comment>DepartmentOfTransportation 

is a subclass of GovernmentOrganization that includes national or 

subnational level departments concerned with transportation in the region 

where they operate or have jurisdiction.  Also called, Ministry of 

Transportation.</rdfs:comment>
    <rdfs:subClassOf rdf:resource="&SUMO;GovernmentOrganization"/>
  </owl:Class>

  <owl:Class rdf:about="#DiningCar">
    <rdfs:comment>DiningCar is the subclass of PassengerRailcars that are equipped 

with dining tables and food preparation areas, where meals are served 

to passengers.</rdfs:comment>
    <rdfs:subClassOf rdf:resource="#PassengerRailwayCar"/>
    <rdfs:subClassOf rdf:resource="#Railcar"/>
  </owl:Class>

  <owl:Class rdf:about="#DirectingTraffic">
    <rdfs:comment>DirectingTraffic is the subclass of 

actions in which a person uses hand gestures to regulate the movement 

of vehicles.</rdfs:comment>
    <rdfs:subClassOf rdf:resource="&SUMO;BodyMotion"/>
    <rdfs:subClassOf rdf:resource="&SUMO;Communication"/>
  </owl:Class>

  <owl:Class rdf:about="#DisplacementHullWatercraft">
    <rdfs:comment>DisplacementHullWatercraft is 

a subclass of Watercraft with hulls designed to move water aside as they 

move through the water.  Contrast with PlaningHullWatercraft.</rdfs:comment>
    <rdfs:subClassOf rdf:resource="&Mid-level-ontology;Watercraft"/>
  </owl:Class>

  <owl:Class rdf:about="#Drawbridge">
    <rdfs:comment>Drawbridge is the subclass of FixedBridges 

that have moveable parts allowing objects taller than the bridge 

clearance to pass beneath the bridge, as on a Waterway.</rdfs:comment>
    <rdfs:subClassOf rdf:resource="#FixedBridge"/>
    <rdfs:subClassOf rdf:resource="&SUMO;Device"/>
    <owl:disjointWith rdf:resource="#Axle"/>
    <owl:disjointWith rdf:resource="#CanalLockGate"/>
    <owl:disjointWith rdf:resource="&Mid-level-ontology;AnimalPoweredDevice"/>
  </owl:Class>

  <owl:Class rdf:about="#Dredger">
    <rdfs:subClassOf rdf:resource="&Mid-level-ontology;Ship"/>
    <owl:disjointWith rdf:resource="#CableShip"/>
    <owl:disjointWith rdf:resource="#CargoShip"/>
    <owl:disjointWith rdf:resource="#CraneShip"/>
    <owl:disjointWith rdf:resource="#DrillingShip"/>
    <owl:disjointWith rdf:resource="#IceBreakerShip"/>
    <owl:disjointWith rdf:resource="#MerchantMarineShip"/>
    <owl:disjointWith rdf:resource="#MotorHopper"/>
    <owl:disjointWith rdf:resource="#OffshoreSupplyShip"/>
    <owl:disjointWith rdf:resource="#OffshoreSupportShip"/>
    <owl:disjointWith rdf:resource="#OffshoreWellProductionShip"/>
    <owl:disjointWith rdf:resource="#PassengerShip"/>
    <owl:disjointWith rdf:resource="#ResearchShip"/>
    <owl:disjointWith rdf:resource="#SludgeDisposalVessel"/>
  </owl:Class>

  <owl:Class rdf:about="#DrillingShip">
    <rdfs:subClassOf rdf:resource="&Mid-level-ontology;Ship"/>
    <owl:disjointWith rdf:resource="#CableShip"/>
    <owl:disjointWith rdf:resource="#CargoShip"/>
    <owl:disjointWith rdf:resource="#CraneShip"/>
    <owl:disjointWith rdf:resource="#Dredger"/>
    <owl:disjointWith rdf:resource="#IceBreakerShip"/>
    <owl:disjointWith rdf:resource="#MerchantMarineShip"/>
    <owl:disjointWith rdf:resource="#MotorHopper"/>
    <owl:disjointWith rdf:resource="#OffshoreSupplyShip"/>
    <owl:disjointWith rdf:resource="#OffshoreSupportShip"/>
    <owl:disjointWith rdf:resource="#OffshoreWellProductionShip"/>
    <owl:disjointWith rdf:resource="#PassengerShip"/>
    <owl:disjointWith rdf:resource="#ResearchShip"/>
    <owl:disjointWith rdf:resource="#SludgeDisposalVessel"/>
  </owl:Class>

  <owl:Class rdf:about="#DromedaryContainer">
    <rdfs:comment>DromedaryContainer is the subclass 

of CargoContainers that can be mounted on TruckTrailers.</rdfs:comment>
    <rdfs:subClassOf rdf:resource="#CargoContainer"/>
    <owl:disjointWith rdf:resource="#FlatRackContainer"/>
    <owl:disjointWith rdf:resource="#HalfHeightContainer"/>
    <owl:disjointWith rdf:resource="#MilitaryVan"/>
    <owl:disjointWith rdf:resource="#Seavan"/>
  </owl:Class>

  <owl:Class rdf:about="#DryBulkCargo">
    <rdfs:comment>DryBulkCargo is the subclass of BulkCargo 

that represents dry bulk cargo.</rdfs:comment>
    <rdfs:subClassOf rdf:resource="#BulkCargo"/>
  </owl:Class>

  <owl:Class rdf:about="#DryBulkCarrierShip">
    <SUMO:disjoint rdf:resource="#ContainerShip"/>
    <rdf:type rdf:resource="&owl;Thing"/>
    <rdfs:comment>DryBulkCarrierShip is the subclass 

of CargoShips that carry dry, loose (uncontainerized), homogeneous 

BulkCargo loaded directly into their holds.</rdfs:comment>
    <rdfs:subClassOf rdf:resource="#CargoShip"/>
  </owl:Class>

  <owl:Class rdf:about="#DualGaugeRailway">
    <rdfs:comment>DualGaugeRailway is the class of 

Railway that has three tracks, enabling trains of two different gauges 

to run on it.</rdfs:comment>
    <rdfs:subClassOf rdf:resource="&Mid-level-ontology;Railway"/>
  </owl:Class>

  <owl:Class rdf:about="#ElectrifiedRailway">
    <rdfs:comment>ElectrifiedRailway is the subclass 

of Railway representing electrified railways.</rdfs:comment>
    <rdfs:subClassOf rdf:resource="&Mid-level-ontology;Railway"/>
  </owl:Class>

  <owl:Class rdf:about="#ElectrifiedRailwayCar">
    <rdfs:comment>ElectrifiedRailwayCar is the 

subclass of railway cars that are powered by electricity, which is 

provided to the car through an overhead link or electrified third rail.</rdfs:comment>
    <rdfs:subClassOf rdf:resource="#RollingStock"/>
    <rdfs:subClassOf rdf:resource="#SelfPoweredVehicle"/>
    <rdfs:subClassOf rdf:resource="&Mid-level-ontology;ElectricDevice"/>
    <owl:disjointWith rdf:resource="#CabCar"/>
    <owl:disjointWith rdf:resource="#EmergencyVehicle"/>
    <owl:disjointWith rdf:resource="#Locomotive"/>
    <owl:disjointWith rdf:resource="#MotorizedRailwayCar"/>
    <owl:disjointWith rdf:resource="#PersonalWatercraft"/>
    <owl:disjointWith rdf:resource="#SelfPoweredRoadVehicle"/>
    <owl:disjointWith rdf:resource="#Tugboat"/>
    <owl:disjointWith rdf:resource="&Mid-level-ontology;Airplane"/>
    <owl:disjointWith rdf:resource="&Mid-level-ontology;ElectricMotor"/>
    <owl:disjointWith rdf:resource="&Mid-level-ontology;Train"/>
  </owl:Class>

  <owl:Class rdf:about="#EmergencyRoadVehicle">
    <rdfs:comment>EmergencyRoadVehicle is the 

subclass of EmergencyVehicle that includes RoadVehicles designed 

for special use in emergencies, e.g., Ambulances, FireEngines.</rdfs:comment>
    <rdfs:subClassOf rdf:resource="#EmergencyVehicle"/>
    <rdfs:subClassOf rdf:resource="#SelfPoweredRoadVehicle"/>
    <owl:disjointWith rdf:resource="&Mid-level-ontology;Automobile"/>
  </owl:Class>

  <owl:Class rdf:about="#EmergencyVehicle">
    <rdfs:comment>EmergencyVehicle is the subclass of 

Vehicles that are used for special-purpose emergency response.</rdfs:comment>
    <rdfs:subClassOf rdf:resource="#SelfPoweredVehicle"/>
    <owl:disjointWith rdf:resource="#ElectrifiedRailwayCar"/>
    <owl:disjointWith rdf:resource="#Locomotive"/>
    <owl:disjointWith rdf:resource="&Mid-level-ontology;Airplane"/>
  </owl:Class>

  <owl:Class rdf:about="#EtiologicAgent">
    <rdfs:comment>EtiologicAgent is a subclass of 

OrganicObjects identified in the Hazardous Materials Regulations (49 CR) 

as viable microorganisms, or their toxins, which may cause human disease.</rdfs:comment>
    <rdfs:subClassOf rdf:resource="&SUMO;OrganicObject"/>
  </owl:Class>

  <Transportation:VehicleClassForFHWA rdf:about="#FHWAVehicleClass1">
    <rdf:type rdf:resource="&owl;Class"/>
  </Transportation:VehicleClassForFHWA>

  <Transportation:VehicleClassForFHWA rdf:about="#FHWAVehicleClass10">
    <rdf:type rdf:resource="&owl;Class"/>
    <rdfs:subClassOf rdf:resource="#TractorTrailer"/>
  </Transportation:VehicleClassForFHWA>

  <Transportation:VehicleClassForFHWA rdf:about="#FHWAVehicleClass11">
    <rdf:type rdf:resource="&owl;Class"/>
    <rdfs:subClassOf rdf:resource="#TractorTrailer"/>
  </Transportation:VehicleClassForFHWA>

  <Transportation:VehicleClassForFHWA rdf:about="#FHWAVehicleClass12">
    <rdf:type rdf:resource="&owl;Class"/>
    <rdfs:subClassOf rdf:resource="#TractorTrailer"/>
  </Transportation:VehicleClassForFHWA>

  <Transportation:VehicleClassForFHWA rdf:about="#FHWAVehicleClass13">
    <rdf:type rdf:resource="&owl;Class"/>
    <rdfs:subClassOf rdf:resource="#TractorTrailer"/>
  </Transportation:VehicleClassForFHWA>

  <Transportation:VehicleClassForFHWA rdf:about="#FHWAVehicleClass2">
    <rdf:type rdf:resource="&owl;Class"/>
  </Transportation:VehicleClassForFHWA>

  <Transportation:VehicleClassForFHWA rdf:about="#FHWAVehicleClass4">
    <rdf:type rdf:resource="&owl;Class"/>
  </Transportation:VehicleClassForFHWA>

  <Transportation:VehicleClassForFHWA rdf:about="#FHWAVehicleClass5">
    <rdf:type rdf:resource="&owl;Class"/>
    <rdfs:subClassOf rdf:resource="&Mid-level-ontology;Truck"/>
  </Transportation:VehicleClassForFHWA>

  <Transportation:VehicleClassForFHWA rdf:about="#FHWAVehicleClass6">
    <rdf:type rdf:resource="&owl;Class"/>
    <rdfs:subClassOf rdf:resource="&Mid-level-ontology;Truck"/>
  </Transportation:VehicleClassForFHWA>

  <Transportation:VehicleClassForFHWA rdf:about="#FHWAVehicleClass7">
    <rdf:type rdf:resource="&owl;Class"/>
    <rdfs:subClassOf rdf:resource="&Mid-level-ontology;Truck"/>
  </Transportation:VehicleClassForFHWA>

  <Transportation:VehicleClassForFHWA rdf:about="#FHWAVehicleClass8">
    <rdf:type rdf:resource="&owl;Class"/>
    <rdfs:subClassOf rdf:resource="#TractorTrailer"/>
  </Transportation:VehicleClassForFHWA>

  <Transportation:VehicleClassForFHWA rdf:about="#FHWAVehicleClass9">
    <rdf:type rdf:resource="&owl;Class"/>
    <rdfs:subClassOf rdf:resource="#TractorTrailer"/>
  </Transportation:VehicleClassForFHWA>

  <owl:Class rdf:about="#FireBoat">
    <rdfs:comment>FireBoat is the subclass of EmergencyVehicles 

that are boats capable of spraying water to fight fires on ships or on the 

waterfront.</rdfs:comment>
    <rdfs:subClassOf rdf:resource="#EmergencyVehicle"/>
    <rdfs:subClassOf rdf:resource="&Mid-level-ontology;Watercraft"/>
  </owl:Class>

  <owl:Class rdf:about="#FireEngine">
    <rdfs:comment>FireEngine is the subclass of 

EmergencyRoadVehicles that represents fire engines.</rdfs:comment>
    <rdfs:subClassOf rdf:resource="#EmergencyRoadVehicle"/>
  </owl:Class>

  <owl:Class rdf:about="#FishCarrierShip">
    <rdfs:subClassOf rdf:resource="#FishingVessel"/>
  </owl:Class>

  <owl:Class rdf:about="#FishFactoryShip">
    <rdfs:subClassOf rdf:resource="#FishingVessel"/>
  </owl:Class>

  <owl:Class rdf:about="#FishingBoat">
    <rdfs:subClassOf rdf:resource="#FishingVessel"/>
  </owl:Class>

  <owl:Class rdf:about="#FishingTrawler">
    <rdfs:subClassOf rdf:resource="#FishingVessel"/>
  </owl:Class>

  <owl:Class rdf:about="#FishingVessel">
    <rdf:type rdf:resource="&owl;Thing"/>
    <rdfs:comment>FishingVessel is a broad subclass of boats 

and ships that are used in FishingProcesses.</rdfs:comment>
    <rdfs:subClassOf rdf:resource="&Mid-level-ontology;Watercraft"/>
  </owl:Class>

  <owl:Class rdf:about="#FiveWellStackCar"
             rdfs:label="stack car">
    <rdfs:comment>FiveWellStackCar is the subclass of 

FreightCars that are five-unit cars that carry double-stacked 

CargoContainers.</rdfs:comment>
    <rdfs:subClassOf rdf:resource="#OpenTopRailcar"/>
  </owl:Class>

  <owl:Class rdf:about="#FixedBridge">
    <rdfs:comment>FixedBridge is the subclass of Bridges 

that are permanently installed at their location.  This includes 

Drawbridges; although drawbridges have moveable parts, their location 

is fixed.</rdfs:comment>
    <rdfs:subClassOf rdf:resource="&Mid-level-ontology;Bridge"/>
    <rdfs:subClassOf rdf:resource="&SUMO;StationaryArtifact"/>
  </owl:Class>

  <owl:Class rdf:about="#FlagOfConvenienceRegister">
    <rdfs:comment>FlagOfConvenienceRegister is the subclass of ShipRegisters 

in which most of the registered ships are owned outside of the 

GeopoliticalArea to which the registry belongs.  

InternalShipRegisters and OffshoreShipRegisters both may act as 

FlagOfConvenienceRegisters, if permitted by the maritime 

regulations of the registry owner.</rdfs:comment>
    <rdfs:label>flag of convenience</rdfs:label>
    <rdfs:label>open register</rdfs:label>
    <rdfs:subClassOf rdf:resource="#ShipRegister"/>
    <owl:disjointWith rdf:resource="#InternalShipRegister"/>
    <owl:disjointWith rdf:resource="#NationalShipRegister"/>
    <owl:disjointWith rdf:resource="#OffshoreShipRegister"/>
  </owl:Class>

  <owl:Class rdf:about="#FlatRackContainer">
    <rdfs:comment>FlatRackContainer is the subclass of 

CargoContainers that have open sides and top, with two adjustable or 

removable ends.  FlatRackContainers meet International Standards 

Organization (ISO) standards.</rdfs:comment>
    <rdfs:subClassOf rdf:resource="#CargoContainer"/>
    <owl:disjointWith rdf:resource="#DromedaryContainer"/>
  </owl:Class>

  <owl:Class rdf:about="#Flatcar">
    <rdfs:comment>Flatcar is the subclass of FreightCars that do 

not have sides or roofs.</rdfs:comment>
    <rdfs:subClassOf rdf:resource="#FreightCar"/>
    <rdfs:subClassOf rdf:resource="#OpenTopRailcar"/>
  </owl:Class>

  <owl:Class rdf:about="#FlightDeck">
    <rdfs:comment>FlightDeck is the subclass of ShipDecks 

where aircraft take off and land.</rdfs:comment>
    <rdfs:subClassOf rdf:resource="#ShipDeck"/>
  </owl:Class>

  <owl:Class rdf:about="#FlightSchedule">
    <rdfs:comment>FlightSchedule is the subclass of 

TransportationSchedules that contain flight information.</rdfs:comment>
    <rdfs:subClassOf rdf:resource="#TransportationSchedule"/>
  </owl:Class>

  <owl:Class rdf:about="#FreightCar">
    <rdfs:comment>FreightCar is the subclass of Railcars that 

are used for hauling freight: bulk materials, manufactured goods, and other 

commodities.</rdfs:comment>
    <rdfs:subClassOf rdf:resource="#Railcar"/>
  </owl:Class>

  <owl:Class rdf:about="#Freighter"
             rdfs:label="freighter">
    <rdfs:comment>Freighter is the subclass of CargoShip 

that includes breakbulk vessels (refrigerated and non-), container ships, 

partial containerships, roll-on roll-off vessels, and barge carriers.</rdfs:comment>
    <rdfs:subClassOf rdf:resource="#CargoShip"/>
  </owl:Class>

  <owl:Class rdf:about="#FuelTank">
    <rdfs:comment>FuelTank is the subclass of Containers that 

are designed as reservoirs for Fuel.  FuelTank includes both 

stand-alone fuel tanks and fuel tanks that are attached to Engines 

and SelfPoweredDevices.</rdfs:comment>
    <rdfs:subClassOf rdf:resource="&Mid-level-ontology;Container"/>
    <owl:disjointWith rdf:resource="#CargoContainer"/>
  </owl:Class>

  <owl:Class rdf:about="#FullSizeVan">
    <rdfs:subClassOf rdf:resource="&Mid-level-ontology;Automobile"/>
  </owl:Class>

  <owl:Class rdf:about="#GalleryCar">
    <rdfs:comment>GalleryCar is the subclass of PassengerRailcars that are double-decked 

passenger cars with a glassed-in viewing area on the second floor.</rdfs:comment>
    <rdfs:subClassOf rdf:resource="#PassengerRailwayCar"/>
    <rdfs:subClassOf rdf:resource="#Railcar"/>
  </owl:Class>

  <owl:Class rdf:about="#GeneralCargoShip">
    <rdfs:comment>GeneralCargoShip is the subclass of 

CargoShips that carry heterogeneous cargo in various kinds of 

packaging.</rdfs:comment>
    <rdfs:subClassOf rdf:resource="#CargoShip"/>
  </owl:Class>

  <owl:Class rdf:about="#GliderAirplane">
    <rdfs:comment>GliderAirplane is the subclass of 

fixed-wing Aircraft that fly by gliding, without using an engine.</rdfs:comment>
    <rdfs:subClassOf rdf:resource="#WindPoweredDevice"/>
    <rdfs:subClassOf rdf:resource="&Mid-level-ontology;Aircraft"/>
    <owl:disjointWith rdf:resource="&Mid-level-ontology;Airplane"/>
  </owl:Class>

  <owl:Class rdf:about="#GondolaRailcar">
    <rdfs:comment>GondolaRailcar is the subclass of 

OpenTopRailcars that have fixed sides, generally used for hauling 

BulkCargo such as Coal.</rdfs:comment>
    <rdfs:subClassOf rdf:resource="#OpenTopRailcar"/>
  </owl:Class>

  <owl:Class rdf:about="#GreatLakesShip"
             rdfs:label="laker">
    <rdfs:comment>GreatLakesShip is the subclass of 

CargoShips that are built especially for use on the Great Lakes of 

North America.  Typically they carry bulk cargo of grain, iron ore, 

or coal.</rdfs:comment>
    <rdfs:subClassOf rdf:resource="#CargoShip"/>
  </owl:Class>

  <owl:Class rdf:about="#HalfHeightContainer">
    <rdfs:comment>HalfHeightContainer is the subclass 

of CargoContainers that have one end door and an open top.  Half-height 

containers meet International Standards Organization (ISO) standards.</rdfs:comment>
    <rdfs:subClassOf rdf:resource="#CargoContainer"/>
    <owl:disjointWith rdf:resource="#DromedaryContainer"/>
  </owl:Class>

  <owl:Class rdf:about="#HangarBay">
    <rdfs:comment>HangarBay is the subclass of 

ShipCompartments where Aircraft are stored aboard ship.</rdfs:comment>
    <rdfs:subClassOf rdf:resource="#ShipCompartment"/>
  </owl:Class>

  <owl:Class rdf:about="#Harbor">
    <rdfs:comment>Harbor is the subclass of WaterAreas that 

provide shelter and anchorage for Watercraft.  Every PortCity has 

a Harbor.</rdfs:comment>
    <rdfs:subClassOf rdf:resource="&SUMO;WaterArea"/>
    <owl:disjointWith rdf:resource="#Anchorage"/>
    <owl:disjointWith rdf:resource="#DeepDraftWaterArea"/>
    <owl:disjointWith rdf:resource="#ShipBerth"/>
    <owl:disjointWith rdf:resource="&Mid-level-ontology;Waterway"/>
  </owl:Class>

  <owl:Class rdf:about="#HeadEndCar">
    <rdfs:comment>HeadEndCar is the subclass of Railcars that 

are typically placed near the front of a train, including mail cars and 

baggage cars.</rdfs:comment>
    <rdfs:subClassOf rdf:resource="#Railcar"/>
  </owl:Class>

  <owl:Class rdf:about="#Heliport">
    <rdfs:comment>Heliport is the class of TransitTerminals 

designed for the takeoff and landing of Helicopters.</rdfs:comment>
    <rdfs:label>helipad</rdfs:label>
    <rdfs:label>heliport</rdfs:label>
    <rdfs:subClassOf rdf:resource="#AirTransitway"/>
    <rdfs:subClassOf rdf:resource="&Mid-level-ontology;TransitTerminal"/>
    <owl:disjointWith rdf:resource="#AirRoute"/>
    <owl:disjointWith rdf:resource="&Mid-level-ontology;Airplane"/>
    <owl:disjointWith rdf:resource="&Mid-level-ontology;Airport"/>
  </owl:Class>

  <owl:Class rdf:about="#HopperDredger">
    <rdfs:subClassOf rdf:resource="#Dredger"/>
  </owl:Class>

  <owl:Class rdf:about="#HumanHabitationArtifact">
    <rdfs:comment>HumanHabitationArtifact is the 

subclass of HumanHabitationSpaces that are also Artifacts.</rdfs:comment>
    <rdfs:subClassOf rdf:resource="#HumanHabitationSpace"/>
    <rdfs:subClassOf rdf:resource="&SUMO;Artifact"/>
    <owl:disjointWith rdf:resource="#ShipCompartment"/>
    <owl:disjointWith rdf:resource="#ShipDeck"/>
    <owl:disjointWith rdf:resource="#ShipHull"/>
  </owl:Class>

  <owl:Class rdf:about="#HumanHabitationSpace">
    <rdfs:comment>HumanHabitationSpace is the subclass 

of Regions that are created as or reserved for, and suited to, occupation 

by Human beings.</rdfs:comment>
    <rdfs:subClassOf rdf:resource="&SUMO;Region"/>
  </owl:Class>

  <owl:Class rdf:about="#HumanPoweredDevice">
    <rdfs:comment>HumanPoweredDevice is the 

subclass of Devices that are moved by human exertion, including 

Canoes, Bicycles, and hand saws.</rdfs:comment>
    <rdfs:subClassOf rdf:resource="&SUMO;Device"/>
    <owl:disjointWith rdf:resource="#Axle"/>
    <owl:disjointWith rdf:resource="#CanalLockGate"/>
    <owl:disjointWith rdf:resource="&Mid-level-ontology;AnimalPoweredDevice"/>
  </owl:Class>

  <owl:Class rdf:about="#HydraCushionFreightCar">
    <rdfs:comment>HydraCushionFreightCars is the 

subclass of FreightCars that have hydraulic underframes to cushion 

their loads.</rdfs:comment>
    <rdfs:subClassOf rdf:resource="#FreightCar"/>
  </owl:Class>

  <owl:Class rdf:about="#IceBreakerShip">
    <rdfs:subClassOf rdf:resource="&Mid-level-ontology;Ship"/>
    <owl:disjointWith rdf:resource="#CableShip"/>
    <owl:disjointWith rdf:resource="#CargoShip"/>
    <owl:disjointWith rdf:resource="#CraneShip"/>
    <owl:disjointWith rdf:resource="#Dredger"/>
    <owl:disjointWith rdf:resource="#DrillingShip"/>
    <owl:disjointWith rdf:resource="#MerchantMarineShip"/>
    <owl:disjointWith rdf:resource="#MotorHopper"/>
    <owl:disjointWith rdf:resource="#OffshoreSupplyShip"/>
    <owl:disjointWith rdf:resource="#OffshoreSupportShip"/>
    <owl:disjointWith rdf:resource="#OffshoreWellProductionShip"/>
    <owl:disjointWith rdf:resource="#PassengerShip"/>
    <owl:disjointWith rdf:resource="#ResearchShip"/>
    <owl:disjointWith rdf:resource="#SludgeDisposalVessel"/>
  </owl:Class>

  <owl:Class rdf:about="#IntermodalTransportation">
    <rdfs:comment>IntermodalTransportation is 

the subclass of Transportation events in which more than one kind of 

Transitway (road, rail, sea, or air) is used.  That is, there are at 

least two subProcesses of the motion that use different types of 

Transitway.</rdfs:comment>
    <rdfs:subClassOf rdf:resource="&SUMO;Transportation"/>
  </owl:Class>

  <owl:Class rdf:about="#IntermodalTransportationSystem">
    <rdfs:comment>IntermodalTransportationSystem is the class of TransportationSystems 

that include more than one type of Transitway and can accommodate more 

than one type of TransportationDevice.</rdfs:comment>
    <rdfs:subClassOf rdf:resource="#TransportationSystem"/>
  </owl:Class>

  <owl:Class rdf:about="#InternalShipRegister">
    <rdfs:subClassOf rdf:resource="#ShipRegister"/>
    <owl:disjointWith rdf:resource="#FlagOfConvenienceRegister"/>
  </owl:Class>

  <owl:Class rdf:about="#InternationalAirport">
    <rdfs:comment>InternationalAirport is the subclass 

of Airports that are the origin or destination for flights outside of 

the Nation where the airport is located.</rdfs:comment>
    <rdfs:subClassOf rdf:resource="#CommercialAirport"/>
    <rdfs:subClassOf rdf:resource="&Mid-level-ontology;Airport"/>
    <owl:disjointWith rdf:resource="#CommercialAirport"/>
  </owl:Class>

  <owl:Class rdf:about="#JetAirplane">
    <rdfs:comment>JetAirplane is the subclass of Aircraft 

that are powered by JetEngines.</rdfs:comment>
    <rdfs:subClassOf rdf:resource="&Mid-level-ontology;Airplane"/>
    <owl:disjointWith rdf:resource="#PropellerAirplane"/>
    <owl:disjointWith rdf:resource="#TurbopropAirplane"/>
  </owl:Class>

  <owl:Class rdf:about="#JetEngine">
    <rdfs:subClassOf rdf:resource="&Mid-level-ontology;InternalCombustionEngine"/>
  </owl:Class>

  <owl:Class rdf:about="#Kayak">
    <rdfs:subClassOf rdf:resource="#HumanPoweredDevice"/>
    <rdfs:subClassOf rdf:resource="&Mid-level-ontology;Watercraft"/>
    <owl:disjointWith rdf:resource="#Canoe"/>
  </owl:Class>

  <owl:Class rdf:about="#LightTruck">
    <rdfs:comment>LightTruck is the subclass of Automobiles 

that are built on truck chassis and have a gross vehicle weight rating 

(GVWR) of 8,500 pounds or less and a vehicle curb weight (VCW) of 6,000 

pounds or less. (49 CFR 523)  As a classification for fuel emissions, 

LightTrucks may include SUVs and mini-vans that meet the weight 

requirements.</rdfs:comment>
    <rdfs:subClassOf rdf:resource="&Mid-level-ontology;Automobile"/>
    <rdfs:subClassOf rdf:resource="&Mid-level-ontology;Truck"/>
  </owl:Class>

  <owl:Class rdf:about="#Lighter">
    <rdfs:comment>Lighter is the subclass of Barges that are 

used for short-haul transport, as for moving goods between shore and a 

CargoShip.</rdfs:comment>
    <rdfs:subClassOf rdf:resource="#Barge"/>
  </owl:Class>

  <owl:Class rdf:about="#LinerService">
    <rdfs:comment>LinerService is the subclass of 

Transportation events that are regularly scheduled Ship passages 

offered by a TransportationCompany.</rdfs:comment>
    <rdfs:subClassOf rdf:resource="&SUMO;Transportation"/>
  </owl:Class>

  <owl:Class rdf:about="#LiquefiedGasAndChemicalTankerShip">
    <rdfs:comment>LiquefiedGasAndChemicalTankerShip is the subclass of ships that can 

carry liquefied gas or ChemicalProducts.</rdfs:comment>
    <rdfs:subClassOf rdf:resource="#ChemicalTankerShip"/>
    <rdfs:subClassOf rdf:resource="#LiquefiedGasTankerShip"/>
  </owl:Class>

  <owl:Class rdf:about="#LiquefiedGasTankerShip"
             rdfs:label="liquefied gas carrier">
    <rdfs:comment>LiquefiedGasTankerShip is the 

subclass of ships that carry liquefied gas products.</rdfs:comment>
    <rdfs:subClassOf rdf:resource="#CargoShip"/>
  </owl:Class>

  <owl:Class rdf:about="#LivestockCarrierShip">
    <rdfs:comment>LivestockCarrierShip is a subclass 

of CargoShips that are used for carrying cattle and other livestock.</rdfs:comment>
    <rdfs:subClassOf rdf:resource="#CargoShip"/>
  </owl:Class>

  <owl:Class rdf:about="#LocalTransitSystem">
    <rdfs:comment>LocalTransitSystem is the subclass 

of TransportationSystems that are located in a regional area, under a 

single or unified TransitAuthority.</rdfs:comment>
    <rdfs:subClassOf rdf:resource="#TransportationSystem"/>
  </owl:Class>

  <owl:Class rdf:about="#Locomotive">
    <rdfs:comment>Locomotive is the subclass of RollingStock

that represents train locomotives, including those with DieselEngines 

and with SteamEngines.</rdfs:comment>
    <rdfs:subClassOf rdf:resource="#RollingStock"/>
    <rdfs:subClassOf rdf:resource="#SelfPoweredVehicle"/>
    <owl:disjointWith rdf:resource="#ElectrifiedRailwayCar"/>
    <owl:disjointWith rdf:resource="#EmergencyVehicle"/>
    <owl:disjointWith rdf:resource="#MotorizedRailwayCar"/>
    <owl:disjointWith rdf:resource="#PersonalWatercraft"/>
    <owl:disjointWith rdf:resource="#SelfPoweredRoadVehicle"/>
    <owl:disjointWith rdf:resource="#Tugboat"/>
    <owl:disjointWith rdf:resource="&Mid-level-ontology;Airplane"/>
    <owl:disjointWith rdf:resource="&Mid-level-ontology;Train"/>
  </owl:Class>

  <owl:Class rdf:about="#LocomotiveCoalCar">
    <rdfs:comment>LocomotiveCoalCar is the subclass  

of Railcars used for transporting fuel Coal for coal-powered steam 

locomotives.  In a train, they are placed directly behind the Locomotive 

for ready accessibility.</rdfs:comment>
    <rdfs:subClassOf rdf:resource="#Railcar"/>
  </owl:Class>

  <SUMO:UnitOfMeasure rdf:about="#LongTon">
    <rdf:type rdf:resource="&owl;Class"/>
    <rdfs:comment>LongTon is the UnitOfMeasure, 

equal to 2,240 PoundMass, which is used to measure Dead Weight 

Tonnage capacity of Ships.</rdfs:comment>
    <rdfs:subClassOf rdf:resource="&SUMO;MassMeasure"/>
  </SUMO:UnitOfMeasure>

  <owl:Class rdf:about="#MajorAirCarrier">
    <rdfs:comment>MajorAirCarrier is a certified  

commercial air carrier with annual revenues of one billion dollars (U.S.) 

or more.</rdfs:comment>
    <rdfs:subClassOf rdf:resource="&Mid-level-ontology;TransportationCompany"/>
  </owl:Class>

  <owl:Class rdf:about="#MaritimeBlockade">
    <rdfs:comment>MaritimeBlockade is the subclass of 

IntentionalProcesses in which access to and egress from a PortCity 

is prevented by physical obstacles or threats.</rdfs:comment>
    <rdfs:subClassOf rdf:resource="&SUMO;IntentionalProcess"/>
  </owl:Class>

  <owl:Class rdf:about="#MerchantMarine">
    <rdfs:comment>MerchantMarine is a class of 

Collections of Ships, each collection belonging to a particular 

Nation or GeopoliticalArea, in whose ShipRegister the member 

ships are enrolled.  For example, the merchant marine ships of France.</rdfs:comment>
    <rdfs:subClassOf rdf:resource="&SUMO;Collection"/>
  </owl:Class>

  <owl:Class rdf:about="#MerchantMarineShip">
    <SUMO:disjoint rdf:resource="#FishingVessel"/>
    <SUMO:disjoint rdf:resource="&Mid-level-ontology;MilitaryWatercraft"/>
    <rdf:type rdf:resource="&owl;Thing"/>
    <rdfs:comment>MerchantMarineShip is the class 

of Ships that carry goods or passengers in exchange for payment.  

This excludes military ships, as well as working ships such as tugboats 

and fishing vessels.  Merchant Marine ships belong to the 

MerchantMarine of some country and are registered in its related 

ShipRegister.</rdfs:comment>
    <rdfs:label>commercial vessel</rdfs:label>
    <rdfs:label>merchant ship</rdfs:label>
    <rdfs:subClassOf rdf:resource="&Mid-level-ontology;Ship"/>
    <owl:disjointWith rdf:resource="#CableShip"/>
    <owl:disjointWith rdf:resource="#CargoShip"/>
    <owl:disjointWith rdf:resource="#CraneShip"/>
    <owl:disjointWith rdf:resource="#Dredger"/>
    <owl:disjointWith rdf:resource="#DrillingShip"/>
    <owl:disjointWith rdf:resource="#IceBreakerShip"/>
    <owl:disjointWith rdf:resource="#MotorHopper"/>
    <owl:disjointWith rdf:resource="#OffshoreSupplyShip"/>
    <owl:disjointWith rdf:resource="#OffshoreSupportShip"/>
    <owl:disjointWith rdf:resource="#OffshoreWellProductionShip"/>
    <owl:disjointWith rdf:resource="#PassengerShip"/>
    <owl:disjointWith rdf:resource="#ResearchShip"/>
    <owl:disjointWith rdf:resource="#SludgeDisposalVessel"/>
  </owl:Class>

  <owl:Class rdf:about="#MilitaryVan">
    <rdfs:comment>MilitaryVan is the subclass of 

CargoContainers that are owned by the U.S. military and are used within 

a military-controlled transportation system to ship military cargo.  These 

containers meet both U.S. and international (ISO) standards.</rdfs:comment>
    <rdfs:subClassOf rdf:resource="#CargoContainer"/>
    <owl:disjointWith rdf:resource="#DromedaryContainer"/>
  </owl:Class>

  <owl:Class rdf:about="#Minivan">
    <rdfs:subClassOf rdf:resource="&Mid-level-ontology;Automobile"/>
  </owl:Class>

  <owl:Class rdf:about="#ModeOfTransit">
    <rdfs:comment>ModeOfTransit is the class of generic 

types of Transitways, e.g., road, rail, water, air.</rdfs:comment>
    <rdfs:subClassOf rdf:resource="&SUMO;SetOrClass"/>
    <owl:disjointWith rdf:resource="#VehicleClassForFHWA"/>
  </owl:Class>

  <owl:Class rdf:about="#MotorHopper">
    <rdfs:subClassOf rdf:resource="&Mid-level-ontology;Ship"/>
    <owl:disjointWith rdf:resource="#CableShip"/>
    <owl:disjointWith rdf:resource="#CraneShip"/>
    <owl:disjointWith rdf:resource="#Dredger"/>
    <owl:disjointWith rdf:resource="#DrillingShip"/>
    <owl:disjointWith rdf:resource="#IceBreakerShip"/>
    <owl:disjointWith rdf:resource="#MerchantMarineShip"/>
    <owl:disjointWith rdf:resource="#OffshoreSupplyShip"/>
    <owl:disjointWith rdf:resource="#OffshoreSupportShip"/>
    <owl:disjointWith rdf:resource="#OffshoreWellProductionShip"/>
    <owl:disjointWith rdf:resource="#PassengerShip"/>
    <owl:disjointWith rdf:resource="#ResearchShip"/>
    <owl:disjointWith rdf:resource="#SludgeDisposalVessel"/>
  </owl:Class>

  <owl:Class rdf:about="#MotorScooter">
    <rdfs:comment>MotorScooter is the subclass of 

RoadVehicles that have two or three wheels, with one of the wheels 

in front.  MotorScooters generally have less powerful engines than 

Motorcycles and more comfortable, chairlike seats.</rdfs:comment>
    <rdfs:subClassOf rdf:resource="#SelfPoweredRoadVehicle"/>
    <owl:disjointWith rdf:resource="&Mid-level-ontology;Automobile"/>
  </owl:Class>

  <owl:Class rdf:about="#Motorboat">
    <rdfs:subClassOf rdf:resource="&Mid-level-ontology;Watercraft"/>
  </owl:Class>

  <owl:Class rdf:about="#Motorcycle">
    <rdfs:comment>Motorcycle is the subclass of RoadVehicles 

that have two wheels one behind the other in the frame, upon which the rider 

sits on a seat above the engine.</rdfs:comment>
    <rdfs:subClassOf rdf:resource="#FHWAVehicleClass1"/>
    <rdfs:subClassOf rdf:resource="#SelfPoweredRoadVehicle"/>
    <rdfs:subClassOf rdf:resource="&Mid-level-ontology;RoadVehicle"/>
    <owl:disjointWith rdf:resource="&Mid-level-ontology;Automobile"/>
  </owl:Class>

  <owl:Class rdf:about="#MotorizedRailwayCar">
    <rdfs:comment>MotorizedRailwayCar is the subclass 

of railway cars that carry their own power source.</rdfs:comment>
    <rdfs:subClassOf rdf:resource="#RollingStock"/>
    <rdfs:subClassOf rdf:resource="#SelfPoweredVehicle"/>
    <owl:disjointWith rdf:resource="#ElectrifiedRailwayCar"/>
    <owl:disjointWith rdf:resource="#Locomotive"/>
    <owl:disjointWith rdf:resource="&Mid-level-ontology;Airplane"/>
  </owl:Class>

  <owl:Class rdf:about="#MovingViolation">
    <rdfs:comment>MovingViolation is the class of 

Attributes that characterize Translocation events that are  

performed in some illegal manner.</rdfs:comment>
    <rdfs:subClassOf rdf:resource="&SUMO;RelationalAttribute"/>
  </owl:Class>

  <owl:Class rdf:about="#MultifunctionalLargeLoadCarrierShip">
    <rdfs:comment>MultifunctionalLargeLoadCarrierShip is a subclass of CargoShips that 

are designed to carry large or heavy cargos, and which are equipped with 

on-board cranes or other devices for moving the loads on and off.</rdfs:comment>
    <rdfs:label>heavy cargo carrier</rdfs:label>
    <rdfs:label>heavy lift carrier</rdfs:label>
    <rdfs:subClassOf rdf:resource="#CargoShip"/>
  </owl:Class>

  <owl:Class rdf:about="#MultipleTrackRailway">
    <rdfs:comment>MultipleTrackRailway is the 

subclass of Railway whose instances consists of two or more sets of 

tracks running in parallel, allowing motion in both directions along 

a route without the need for sidings and delays.</rdfs:comment>
    <rdfs:subClassOf rdf:resource="&Mid-level-ontology;Railway"/>
  </owl:Class>

  <owl:Class rdf:about="#NarrowGaugeRailway">
    <rdfs:comment>NarrowGaugeRailway is the class of 

Railway that has a distance less than 1.44 Meters between its 

rails.</rdfs:comment>
    <rdfs:subClassOf rdf:resource="&Mid-level-ontology;Railway"/>
  </owl:Class>

  <owl:Class rdf:about="#NationalShipRegister">
    <SUMO:disjoint rdf:resource="#OffshoreShipRegister"/>
    <rdf:type rdf:resource="&owl;Thing"/>
    <rdfs:comment>NationalShipRegister is the 

subclass of ShipRegisters that belong to Nations.</rdfs:comment>
    <rdfs:subClassOf rdf:resource="#ShipRegister"/>
    <owl:disjointWith rdf:resource="#FlagOfConvenienceRegister"/>
  </owl:Class>

  <owl:Class rdf:about="#NaturalGasPipeline">
    <rdfs:comment>NaturalGasPipeline is the subclass 

of Pipelines that are used to carry NaturalGas.</rdfs:comment>
    <rdfs:subClassOf rdf:resource="&Mid-level-ontology;Pipeline"/>
  </owl:Class>

  <owl:Class rdf:about="#Navigation">
    <rdfs:comment>Navigation is the subclass of Guiding 

for processes that involve plotting a course, determining a position, or 

determining a heading for a Transportation device, especially an 

Aircraft or Ship.  Contrast with Steering, which is physically 

guiding a vehicle, while Navigation is the determination of course 

or position.  The course to be executed by the helm in Steering may be 

the result of a process of Navigation.</rdfs:comment>
    <rdfs:subClassOf rdf:resource="&SUMO;Guiding"/>
  </owl:Class>

  <owl:Class rdf:about="#NavigationBuoy">
    <rdfs:subClassOf rdf:resource="#AidToNavigation"/>
    <owl:disjointWith rdf:resource="#NavigationLight"/>
    <owl:disjointWith rdf:resource="#RadioNavigationBeacon"/>
  </owl:Class>

  <owl:Class rdf:about="#NavigationLight">
    <rdfs:subClassOf rdf:resource="#AidToNavigation"/>
    <rdfs:subClassOf rdf:resource="&Mid-level-ontology;ElectricDevice"/>
    <rdfs:subClassOf rdf:resource="&Mid-level-ontology;LightFixture"/>
    <owl:disjointWith rdf:resource="#NavigationBuoy"/>
    <owl:disjointWith rdf:resource="&Mid-level-ontology;ElectricMotor"/>
  </owl:Class>

  <owl:Class rdf:about="#OceanLiner">
    <rdfs:comment>OceanLiner is the subclass of Ships 

that make regularly scheduled voyages to transport people and goods 

from one place to another.</rdfs:comment>
    <rdfs:subClassOf rdf:resource="#CargoShip"/>
    <rdfs:subClassOf rdf:resource="#PassengerShip"/>
  </owl:Class>

  <owl:Class rdf:about="#OffshoreAnchorage">
    <rdfs:comment>OffshoreAnchorage is the subclass 

of Anchorages that are located offshore and not within a Harbor.</rdfs:comment>
    <rdfs:subClassOf rdf:resource="#Anchorage"/>
  </owl:Class>

  <owl:Class rdf:about="#OffshoreShipRegister">
    <rdf:type rdf:resource="&owl;Thing"/>
    <rdfs:comment>OffshoreShipRegister is 

the class of ShipRegisters maintained by a colony, territory, or 

possession (OffshoreArea) of a Nation.  Typically such a register 

has more lenient maritime regulations with respect to taxation and 

crewing of ships than does the national register associated with the 

country of which the offshore area is a dependency.</rdfs:comment>
    <rdfs:label>captive register</rdfs:label>
    <rdfs:label>offshore ship register</rdfs:label>
    <rdfs:subClassOf rdf:resource="#ShipRegister"/>
    <owl:disjointWith rdf:resource="#FlagOfConvenienceRegister"/>
  </owl:Class>

  <owl:Class rdf:about="#OffshoreSupplyShip">
    <rdfs:subClassOf rdf:resource="&Mid-level-ontology;Ship"/>
    <owl:disjointWith rdf:resource="#CableShip"/>
    <owl:disjointWith rdf:resource="#CargoShip"/>
    <owl:disjointWith rdf:resource="#CraneShip"/>
    <owl:disjointWith rdf:resource="#Dredger"/>
    <owl:disjointWith rdf:resource="#DrillingShip"/>
    <owl:disjointWith rdf:resource="#IceBreakerShip"/>
    <owl:disjointWith rdf:resource="#MerchantMarineShip"/>
    <owl:disjointWith rdf:resource="#MotorHopper"/>
    <owl:disjointWith rdf:resource="#OffshoreSupportShip"/>
    <owl:disjointWith rdf:resource="#OffshoreWellProductionShip"/>
    <owl:disjointWith rdf:resource="#PassengerShip"/>
    <owl:disjointWith rdf:resource="#ResearchShip"/>
    <owl:disjointWith rdf:resource="#SludgeDisposalVessel"/>
  </owl:Class>

  <owl:Class rdf:about="#OffshoreSupportShip">
    <rdfs:subClassOf rdf:resource="&Mid-level-ontology;Ship"/>
    <owl:disjointWith rdf:resource="#CableShip"/>
    <owl:disjointWith rdf:resource="#CargoShip"/>
    <owl:disjointWith rdf:resource="#CraneShip"/>
    <owl:disjointWith rdf:resource="#Dredger"/>
    <owl:disjointWith rdf:resource="#DrillingShip"/>
    <owl:disjointWith rdf:resource="#IceBreakerShip"/>
    <owl:disjointWith rdf:resource="#MerchantMarineShip"/>
    <owl:disjointWith rdf:resource="#MotorHopper"/>
    <owl:disjointWith rdf:resource="#OffshoreSupplyShip"/>
    <owl:disjointWith rdf:resource="#OffshoreWellProductionShip"/>
    <owl:disjointWith rdf:resource="#PassengerShip"/>
    <owl:disjointWith rdf:resource="#ResearchShip"/>
    <owl:disjointWith rdf:resource="#SludgeDisposalVessel"/>
  </owl:Class>

  <owl:Class rdf:about="#OffshoreWellProductionShip">
    <rdfs:subClassOf rdf:resource="&Mid-level-ontology;Ship"/>
    <owl:disjointWith rdf:resource="#CableShip"/>
    <owl:disjointWith rdf:resource="#CargoShip"/>
    <owl:disjointWith rdf:resource="#CraneShip"/>
    <owl:disjointWith rdf:resource="#Dredger"/>
    <owl:disjointWith rdf:resource="#DrillingShip"/>
    <owl:disjointWith rdf:resource="#IceBreakerShip"/>
    <owl:disjointWith rdf:resource="#MerchantMarineShip"/>
    <owl:disjointWith rdf:resource="#MotorHopper"/>
    <owl:disjointWith rdf:resource="#OffshoreSupplyShip"/>
    <owl:disjointWith rdf:resource="#OffshoreSupportShip"/>
    <owl:disjointWith rdf:resource="#PassengerShip"/>
    <owl:disjointWith rdf:resource="#ResearchShip"/>
    <owl:disjointWith rdf:resource="#SludgeDisposalVessel"/>
  </owl:Class>

  <owl:Class rdf:about="#OneWayTransitway">
    <rdfs:comment>OneWayTransitway is the subclass of 

Transitways that are intended for travel in only one direction.</rdfs:comment>
    <rdfs:subClassOf rdf:resource="&SUMO;Transitway"/>
    <owl:disjointWith rdf:resource="#AirTransitway"/>
    <owl:disjointWith rdf:resource="#SingleTrafficLane"/>
    <owl:disjointWith rdf:resource="#TransitRoute"/>
    <owl:disjointWith rdf:resource="&Mid-level-ontology;Pipeline"/>
    <owl:disjointWith rdf:resource="&Mid-level-ontology;TransitwayJunction"/>
    <owl:disjointWith rdf:resource="&Mid-level-ontology;Tunnel"/>
    <owl:disjointWith rdf:resource="&Mid-level-ontology;Waterway"/>
    <owl:disjointWith rdf:resource="&SUMO;LandTransitway"/>
  </owl:Class>

  <owl:Class rdf:about="#OpenTopRailcar">
    <rdfs:comment>OpenTopRailcar is the subset of 

FreightCars that have no roof.  They may have sides or not.</rdfs:comment>
    <rdfs:subClassOf rdf:resource="#FreightCar"/>
  </owl:Class>

  <owl:Class rdf:about="#OreCarrierShip">
    <rdfs:comment>OreCarrierShip is the subclass of 

CargoShips that carry Mineral ores.</rdfs:comment>
    <rdfs:subClassOf rdf:resource="#DryBulkCarrierShip"/>
  </owl:Class>

  <owl:Class rdf:about="#OutfitCar">
    <rdfs:comment>OutfitCar is the subclass of Railcars that 

are used for housing railway construction or maintenance workers in the 

field.  Also called 'camp cars'.</rdfs:comment>
    <rdfs:subClassOf rdf:resource="#PassengerRailwayCar"/>
    <rdfs:subClassOf rdf:resource="#Railcar"/>
  </owl:Class>

  <owl:Class rdf:about="#PalletizedCargoShip">
    <rdfs:subClassOf rdf:resource="#GeneralCargoShip"/>
  </owl:Class>

  <owl:Class rdf:about="#ParkingGarage">
    <rdfs:comment>ParkingGarage is the class of areas where 

Automobiles may be stored when not in use.</rdfs:comment>
    <rdfs:subClassOf rdf:resource="&SUMO;Building"/>
    <owl:disjointWith rdf:resource="&Mid-level-ontology;TerminalBuilding"/>
  </owl:Class>

  <owl:Class rdf:about="#PartialContainerShip">
    <rdfs:comment>PartialContainerShip is the 

subclass of CargoShips that have some portion of their hold designated 

for carrying CargoContainers.</rdfs:comment>
    <rdfs:subClassOf rdf:resource="#CargoShip"/>
    <rdfs:subClassOf rdf:resource="#Freighter"/>
    <owl:disjointWith rdf:resource="#RollOnRollOffCargoShip"/>
  </owl:Class>

  <owl:Class rdf:about="#PassengerAndCargoShip">
    <rdfs:subClassOf rdf:resource="#CargoShip"/>
    <rdfs:subClassOf rdf:resource="#PassengerShip"/>
  </owl:Class>

  <owl:Class rdf:about="#PassengerAndLandingCraft">
    <rdfs:comment>PassengerAndLandingCraft is a 

subclass of Ship representing vessels designed for landing people and 

vehicles on a shore.</rdfs:comment>
    <rdfs:subClassOf rdf:resource="#PassengerAndCargoShip"/>
    <rdfs:subClassOf rdf:resource="#RollOnRollOffCargoShip"/>
  </owl:Class>

  <owl:Class rdf:about="#PassengerCar">
    <rdfs:comment>PassengerCar is the subclass of 

Automobile that includes Economy, Compact, Convertible, Midsize, 

Full Size, Premium, and Luxury cars.</rdfs:comment>
    <rdfs:subClassOf rdf:resource="#FHWAVehicleClass2"/>
    <rdfs:subClassOf rdf:resource="&Mid-level-ontology;Automobile"/>
  </owl:Class>

  <owl:Class rdf:about="#PassengerRailwayCar">
    <rdfs:comment>PassengerRailwayCar is the subclass 

of RollingStock that is designed for transportation of Human beings.  

PassengerRailwayCar includes self-powered vehicles such as CabCars and 

motorized Streetcars, as well as the various kinds of unpowered 

passenger Railcars that are parts of Trains.</rdfs:comment>
    <rdfs:subClassOf rdf:resource="#HumanHabitationArtifact"/>
    <rdfs:subClassOf rdf:resource="#RollingStock"/>
  </owl:Class>

  <owl:Class rdf:about="#PassengerShip">
    <rdfs:comment>PassengerShip is the subclass of 

Watercraft designed for the purpose of carrying passengers and 

capable of carrying at least thirteen passengers.</rdfs:comment>
    <rdfs:subClassOf rdf:resource="&Mid-level-ontology;Ship"/>
    <owl:disjointWith rdf:resource="#CableShip"/>
    <owl:disjointWith rdf:resource="#CargoShip"/>
    <owl:disjointWith rdf:resource="#CraneShip"/>
    <owl:disjointWith rdf:resource="#Dredger"/>
    <owl:disjointWith rdf:resource="#DrillingShip"/>
    <owl:disjointWith rdf:resource="#IceBreakerShip"/>
    <owl:disjointWith rdf:resource="#MerchantMarineShip"/>
    <owl:disjointWith rdf:resource="#MotorHopper"/>
    <owl:disjointWith rdf:resource="#OffshoreSupplyShip"/>
    <owl:disjointWith rdf:resource="#OffshoreSupportShip"/>
    <owl:disjointWith rdf:resource="#OffshoreWellProductionShip"/>
    <owl:disjointWith rdf:resource="#ResearchShip"/>
    <owl:disjointWith rdf:resource="#SludgeDisposalVessel"/>
  </owl:Class>

  <owl:Class rdf:about="#Passport"/>
  <SUMO:GovernmentOrganization rdf:about="#PassportControl">
    <rdf:type rdf:resource="&owl;Class"/>
    <rdfs:comment>PassportControl is the subclass of 

Organizations that are concerned with examining Passports being used 

for travel.  PassportControl may be a government agency or authorized 

by a government organization to conduct its activities.</rdfs:comment>
  </SUMO:GovernmentOrganization>

  <owl:Class rdf:about="#PavedRunway">
    <SUMO:disjoint rdf:resource="#UnpavedRunway"/>
    <rdf:type rdf:resource="&owl;Thing"/>
    <rdfs:comment>PavedRunway is the subclass of Runways 

that are surfaced with concrete or asphalt.</rdfs:comment>
    <rdfs:subClassOf rdf:resource="&Mid-level-ontology;Runway"/>
  </owl:Class>

  <owl:Class rdf:about="#PersonalWatercraft"
             rdfs:label="Jet Ski">
    <rdfs:comment>PersonalWatercraft is the class 

of motor-driven watercraft ridden by one or more passengers, e.g., 

a JetSki.</rdfs:comment>
    <rdfs:subClassOf rdf:resource="#SelfPoweredVehicle"/>
    <rdfs:subClassOf rdf:resource="&Mid-level-ontology;Watercraft"/>
    <owl:disjointWith rdf:resource="#ElectrifiedRailwayCar"/>
    <owl:disjointWith rdf:resource="#Locomotive"/>
    <owl:disjointWith rdf:resource="&Mid-level-ontology;Airplane"/>
  </owl:Class>

  <owl:Class rdf:about="#PetroleumPipeline">
    <rdfs:comment>PetroleumPipeline is the subclass of 

Pipelines that are used to carry Petroleum.</rdfs:comment>
    <rdfs:subClassOf rdf:resource="&Mid-level-ontology;Pipeline"/>
  </owl:Class>

  <owl:Class rdf:about="#PetroleumProductPipeline">
    <rdfs:comment>PetroleumProductPipeline is the subclass of Pipelines that are 

used to carry PetroleumProducts.</rdfs:comment>
    <rdfs:subClassOf rdf:resource="&Mid-level-ontology;Pipeline"/>
  </owl:Class>

  <owl:Class rdf:about="#PetroleumTankerShip">
    <rdfs:comment>PetroleumTankerShip is the 

subclass of ships that carry PetroleumProducts.</rdfs:comment>
    <rdfs:label>oil tanker</rdfs:label>
    <rdfs:label>petroleum tanker</rdfs:label>
    <rdfs:subClassOf rdf:resource="#CargoShip"/>
    <owl:disjointWith rdf:resource="#RollOnRollOffCargoShip"/>
  </owl:Class>

  <owl:Class rdf:about="#Pier">
    <rdfs:comment>Pier is the subclass of StationaryArtifacts that 

are built along a waterfront to provide a landing place for ships or 

boats.</rdfs:comment>
    <rdfs:subClassOf rdf:resource="&SUMO;StationaryArtifact"/>
    <owl:disjointWith rdf:resource="#Bulkhead"/>
    <owl:disjointWith rdf:resource="#CanalLock"/>
    <owl:disjointWith rdf:resource="#CanalStructure"/>
    <owl:disjointWith rdf:resource="&Mid-level-ontology;Bridge"/>
    <owl:disjointWith rdf:resource="&Mid-level-ontology;RailroadTrack"/>
    <owl:disjointWith rdf:resource="&Mid-level-ontology;Railway"/>
    <owl:disjointWith rdf:resource="&Mid-level-ontology;TransitTerminal"/>
    <owl:disjointWith rdf:resource="&Mid-level-ontology;Tunnel"/>
  </owl:Class>

  <owl:Class rdf:about="#PlaningHullWatercraft">
    <rdfs:comment>PlaningHullWatercraft is a subclass 

of Watercraft with hulls designed for a position partially on or above 

the water surface when they are in motion, in order to reduce drag.  See 

also DisplacementHullWatercraft.</rdfs:comment>
    <rdfs:subClassOf rdf:resource="&Mid-level-ontology;Watercraft"/>
  </owl:Class>

  <owl:Class rdf:about="#PontoonBridge">
    <rdfs:comment>PontoonBridge is the subclass of 

PortableBridges that transit a WaterArea, supported on pontoons.</rdfs:comment>
    <rdfs:subClassOf rdf:resource="#PortableBridge"/>
  </owl:Class>

  <owl:Class rdf:about="#PortCity">
    <rdfs:comment>PortCity is the subclass of City whose 

instances are cities or towns located adjacent to a Harbor which is 

included in the administrative area of the city.</rdfs:comment>
    <rdfs:subClassOf rdf:resource="&SUMO;City"/>
  </owl:Class>

  <owl:Class rdf:about="#PortCrane">
    <rdfs:comment>PortCrane is a subclass of Devices that are 

cranes installed in a PortFacility and used for loading and unloading 

ships, especially ContainerShips.</rdfs:comment>
    <rdfs:subClassOf rdf:resource="&Mid-level-ontology;Crane"/>
  </owl:Class>

  <owl:Class rdf:about="#PortDetention">
    <rdfs:comment>PortDetention is the subclass of 

RegulatoryProcesses in which a Ship is kept in PortCity by the 

relevant port authority or other law enforcement agency, on the 

basis that the crew or owners of the ship have infringed on some 

regulation.</rdfs:comment>
    <rdfs:subClassOf rdf:resource="&SUMO;Keeping"/>
    <rdfs:subClassOf rdf:resource="&SUMO;RegulatoryProcess"/>
  </owl:Class>

  <owl:Class rdf:about="#PortEmbargo">
    <rdfs:comment>PortEmbargo is the subclass of 

OrganizationalProcesses in which a Nation forbids commercial 

vessels from leaving its ports.</rdfs:comment>
    <rdfs:subClassOf rdf:resource="&SUMO;OrganizationalProcess"/>
  </owl:Class>

  <owl:Class rdf:about="#PortableBridge">
    <rdfs:comment>(PortableBridge is the subclass of 

Bridges that can be moved from one location to another; for example, 

various types of military bridges.  PortableBridges are designed 

for RoadVehicles.</rdfs:comment>
    <rdfs:subClassOf rdf:resource="&Mid-level-ontology;Bridge"/>
    <rdfs:subClassOf rdf:resource="&SUMO;Roadway"/>
  </owl:Class>

  <owl:Class rdf:about="#PrivateRailcar">
    <rdfs:comment>PrivateRailcar is the subclass of all 

Railcars that are owned and used by private individuals rather than 

by a common carrier transit service.</rdfs:comment>
    <rdfs:subClassOf rdf:resource="#Railcar"/>
  </owl:Class>

  <owl:Class rdf:about="#PropellerAirplane">
    <rdfs:comment>PropellerAirplane is a subclass of 

Airplanes whose driving force is provided by propellers.</rdfs:comment>
    <rdfs:subClassOf rdf:resource="&Mid-level-ontology;Airplane"/>
    <owl:disjointWith rdf:resource="#JetAirplane"/>
  </owl:Class>

  <owl:Class rdf:about="#PusherTug">
    <rdfs:subClassOf rdf:resource="#Tugboat"/>
  </owl:Class>

  <owl:Class rdf:about="#Radar">
    <rdfs:comment>Radar is the subclass of ElectronicDevices 

consisting of a synchronized emitter and receiver, used to locate 

airborne objects or objects on earth's surface.</rdfs:comment>
    <rdfs:subClassOf rdf:resource="http://reliant.teknowledge.com/DAML/Communications.owl#ElectronicDevice"/>
    <rdfs:subClassOf rdf:resource="&Mid-level-ontology;RadarOrSonar"/>
  </owl:Class>

  <owl:Class rdf:about="#RadarFacility">
    <rdfs:comment>RadarFacility is the subclass of 

Organizations that are equipped for monitoring and reporting activity 

using Radar.</rdfs:comment>
    <rdfs:subClassOf rdf:resource="&SUMO;Organization"/>
  </owl:Class>

  <owl:Class rdf:about="#RadioNavigationBeacon">
    <rdfs:subClassOf rdf:resource="#AidToNavigation"/>
    <rdfs:subClassOf rdf:resource="&Mid-level-ontology;ElectricDevice"/>
    <owl:disjointWith rdf:resource="#NavigationBuoy"/>
    <owl:disjointWith rdf:resource="&Mid-level-ontology;ElectricMotor"/>
  </owl:Class>

  <owl:Class rdf:about="#RailCarrierControl">
    <rdfs:comment>RailCarrierControl is the process of 

controlling the speed or direction of a Train by sending high or 

low frequency currents on the rails.</rdfs:comment>
    <rdfs:subClassOf rdf:resource="&Mid-level-ontology;ElectricalSignalling"/>
  </owl:Class>

  <owl:Class rdf:about="#RailTransportationSystem">
    <rdfs:comment>RailTransportationSystem 

is the subclass of TransportationSystems whose routes are Railways.</rdfs:comment>
    <rdfs:subClassOf rdf:resource="#TransportationSystem"/>
  </owl:Class>

  <owl:Class rdf:about="#Railcar">
    <SUMO:disjoint rdf:resource="#SelfPoweredVehicle"/>
    <rdf:type rdf:resource="&owl;Thing"/>
    <rdfs:comment>Railcar is the subclass of RollingStock that 

includes all non-locomotive, non-self-powered RailwayVehicles.</rdfs:comment>
    <rdfs:subClassOf rdf:resource="#RollingStock"/>
  </owl:Class>

  <owl:Class rdf:about="#RailcarCarrierShip">
    <rdfs:comment>RailcarCarrierShip is a subclass of 

CargoShips that are designed to carry railroad cars which are rolled on 

and off.</rdfs:comment>
    <rdfs:subClassOf rdf:resource="#RollOnRollOffCargoShip"/>
  </owl:Class>

  <owl:Class rdf:about="#RailroadBridge">
    <rdfs:comment>RailroadBridge is the subclass of 

Bridges that carry RailroadTracks over a land gap, WaterArea, or 

other obstacle.</rdfs:comment>
    <rdfs:subClassOf rdf:resource="#FixedBridge"/>
    <rdfs:subClassOf rdf:resource="&Mid-level-ontology;Railway"/>
  </owl:Class>

  <owl:Class rdf:about="#RailwayJunction">
    <rdfs:comment>RailwayJunction is the subclass of 

TransitwayJunctions where two or more Railway lines come together.</rdfs:comment>
    <rdfs:subClassOf rdf:resource="&Mid-level-ontology;Railway"/>
    <rdfs:subClassOf rdf:resource="&Mid-level-ontology;TransitwayJunction"/>
    <owl:disjointWith rdf:resource="#WaterwayJunction"/>
    <owl:disjointWith rdf:resource="&Mid-level-ontology;RoadJunction"/>
  </owl:Class>

  <owl:Class rdf:about="#RailwayTerminal">
    <rdfs:comment>RailwayTerminal is the subclass of 

TransitTerminals designed for Trains.  A RailwayTerminal includes 

all the RailroadTrack and any outbuildings or other related structure 

in the terminal, as well as the TrainStation (if there is one).</rdfs:comment>
    <rdfs:subClassOf rdf:resource="&Mid-level-ontology;TransitTerminal"/>
  </owl:Class>

  <owl:Class rdf:about="#RailwayVehicle">
    <rdfs:comment>RailwayVehicle is the subclass of 

Vehicles that are designed to run on Railways, including both Trains 

and individual cars (RollingStock).</rdfs:comment>
    <rdfs:subClassOf rdf:resource="&Mid-level-ontology;LandVehicle"/>
  </owl:Class>

  <owl:Class rdf:about="#RefrigeratedCargoShip"
             rdfs:label="refrigerated carrier">
    <rdfs:comment>RefrigeratedCargoShip is the 

subclass of CargoShips that are designed to carry goods which require 

refrigeration, such as meat or vegetables.  A Cooling system is used 

to refrigerate the ShipHold.</rdfs:comment>
    <rdfs:subClassOf rdf:resource="#CargoShip"/>
    <rdfs:subClassOf rdf:resource="#Freighter"/>
    <owl:disjointWith rdf:resource="#RollOnRollOffCargoShip"/>
  </owl:Class>

  <SUMO:UnitOfMeasure rdf:about="#RegistryTon">
    <rdf:type rdf:resource="&owl;Class"/>
    <rdfs:comment>RegistryTon is a unit of measure used to 

represent the Gross Registered Tonnage (GRT) capacity of Ships.  

GRT is based on a volume measure, with one RegistryTon equal to a 

volume of 100 cubic feet.</rdfs:comment>
    <rdfs:label>Gross Ton</rdfs:label>
    <rdfs:label>Registry Ton</rdfs:label>
    <rdfs:subClassOf rdf:resource="&SUMO;MassMeasure"/>
  </SUMO:UnitOfMeasure>

  <owl:Class rdf:about="#ResearchShip">
    <rdfs:subClassOf rdf:resource="&Mid-level-ontology;Ship"/>
    <owl:disjointWith rdf:resource="#CableShip"/>
    <owl:disjointWith rdf:resource="#CargoShip"/>
    <owl:disjointWith rdf:resource="#CraneShip"/>
    <owl:disjointWith rdf:resource="#Dredger"/>
    <owl:disjointWith rdf:resource="#DrillingShip"/>
    <owl:disjointWith rdf:resource="#IceBreakerShip"/>
    <owl:disjointWith rdf:resource="#MerchantMarineShip"/>
    <owl:disjointWith rdf:resource="#MotorHopper"/>
    <owl:disjointWith rdf:resource="#OffshoreSupplyShip"/>
    <owl:disjointWith rdf:resource="#OffshoreSupportShip"/>
    <owl:disjointWith rdf:resource="#OffshoreWellProductionShip"/>
    <owl:disjointWith rdf:resource="#PassengerShip"/>
    <owl:disjointWith rdf:resource="#SludgeDisposalVessel"/>
  </owl:Class>

  <owl:Class rdf:about="#RiverPort">
    <rdfs:comment>RiverPort is the subclass of PortCity 

whose instances are port cities Adjacent to a navigable River.</rdfs:comment>
    <rdfs:subClassOf rdf:resource="#PortCity"/>
    <owl:disjointWith rdf:resource="#DeepDraftPortCity"/>
  </owl:Class>

  <owl:Class rdf:about="#RoadTransportationSystem">
    <rdfs:comment>RoadTransportationSystem 

is the subclass of TransportationSystems whose routes are Roadways.</rdfs:comment>
    <rdfs:subClassOf rdf:resource="#TransportationSystem"/>
  </owl:Class>

  <owl:Class rdf:about="#RocketEngine">
    <rdfs:subClassOf rdf:resource="&Mid-level-ontology;Engine"/>
  </owl:Class>

  <owl:Class rdf:about="#RollOnRollOffCargoShip">
    <rdfs:comment>RollOnRollOffCargoShip is a 

subclass of CargoShips that carry goods which can be driven or 

'rolled' on and off the ship, such as trucks or trailers.</rdfs:comment>
    <rdfs:label>Ro-Ro</rdfs:label>
    <rdfs:label>roll-on roll-off</rdfs:label>
    <rdfs:subClassOf rdf:resource="#CargoShip"/>
    <rdfs:subClassOf rdf:resource="#Freighter"/>
    <owl:disjointWith rdf:resource="#PartialContainerShip"/>
    <owl:disjointWith rdf:resource="#PetroleumTankerShip"/>
    <owl:disjointWith rdf:resource="#RefrigeratedCargoShip"/>
  </owl:Class>

  <owl:Class rdf:about="#RollingStock">
    <rdfs:comment>RollingStock is the subclass of 

RailwayVehicles that individual railway cars.  RollingStock includes 

locomotives, motorized transit cars, trolleys, and all kinds of railcars.</rdfs:comment>
    <rdfs:subClassOf rdf:resource="#RailwayVehicle"/>
  </owl:Class>

  <owl:Class rdf:about="#RotaryDumpCar">
    <rdfs:comment>RotaryDumpCar is a subclass of open-top 

freight cars that have a rotating coupler allowing them to be emptied 

by dumping while still coupled.</rdfs:comment>
    <rdfs:subClassOf rdf:resource="#GondolaRailcar"/>
  </owl:Class>

  <owl:Class rdf:about="#Sailboat">
    <rdfs:subClassOf rdf:resource="#WindPoweredDevice"/>
    <rdfs:subClassOf rdf:resource="&Mid-level-ontology;Watercraft"/>
  </owl:Class>

  <owl:Class rdf:about="#ScaleTestCar">
    <rdfs:comment>ScaleTestCar is a subclass of Railcars 

that have a known weight and are used to test or calibrate track scales 

used for weighing freight.</rdfs:comment>
    <rdfs:subClassOf rdf:resource="#Railcar"/>
  </owl:Class>

  <owl:Class rdf:about="#SeaLane">
    <rdfs:subClassOf rdf:resource="&Mid-level-ontology;Waterway"/>
    <owl:disjointWith rdf:resource="&Mid-level-ontology;Canal"/>
  </owl:Class>

  <owl:Class rdf:about="#SeaPort">
    <rdfs:comment>SeaPort is the subclass of PortCity 

whose instances are port cities on a Sea or Ocean.</rdfs:comment>
    <rdfs:subClassOf rdf:resource="#PortCity"/>
    <owl:disjointWith rdf:resource="#DeepDraftPortCity"/>
  </owl:Class>

  <owl:Class rdf:about="#Seavan">
    <rdfs:comment>Seavan is the subclass of CargoContainers that 

are moved via ocean transport and have no wheels attached.</rdfs:comment>
    <rdfs:subClassOf rdf:resource="#CargoContainer"/>
    <owl:disjointWith rdf:resource="#DromedaryContainer"/>
  </owl:Class>

  <owl:Class rdf:about="#SelfDischargingBulkCarrierShip">
    <rdfs:comment>OreCSelfDischargingBulkCarrierShip arrierShip is the subclass of 

CargoShips that are equipped to unload their own cargo, e.g., via 

a crane or snorkel.</rdfs:comment>
    <rdfs:subClassOf rdf:resource="#DryBulkCarrierShip"/>
  </owl:Class>

  <owl:Class rdf:about="#SelfPoweredRoadVehicle">
    <rdfs:comment>SelfPoweredRoadVehicle is the 

class of RoadVehicles that are also SelfPoweredVehicles.  

SelfPoweredRoadVehicle covers motorcycles, semi-trailers, RVs, etc., 

as well as Automobiles.  This class includes vehicles powered by 

electricity, gasoline, diesel, and other fuels.</rdfs:comment>
    <rdfs:subClassOf rdf:resource="#SelfPoweredVehicle"/>
    <rdfs:subClassOf rdf:resource="&Mid-level-ontology;RoadVehicle"/>
    <owl:disjointWith rdf:resource="#ElectrifiedRailwayCar"/>
    <owl:disjointWith rdf:resource="#Locomotive"/>
    <owl:disjointWith rdf:resource="&Mid-level-ontology;Airplane"/>
  </owl:Class>

  <owl:Class rdf:about="#SelfPoweredVehicle">
    <rdf:type rdf:resource="&owl;Thing"/>
    <rdfs:comment>SelfPoweredVehicle is the subclass 

of Vehicles whose motion is powered by some kind of on-board 

powerPlant.  Contrast with UserPoweredVehicle and 

AnimalPoweredVehicle.</rdfs:comment>
    <rdfs:subClassOf rdf:resource="&Mid-level-ontology;SelfPoweredDevice"/>
    <rdfs:subClassOf rdf:resource="&SUMO;Vehicle"/>
  </owl:Class>

  <owl:Class rdf:about="#ShipAgent">
    <rdfs:comment>ShipAgent is the subclass of agents, who 

may be persons or companies, that transact business in a specified port 

for a ship's owners or charterers.  A ship's agent is not a member of 

the crew that travels with the Ship.</rdfs:comment>
    <rdfs:subClassOf rdf:resource="&SUMO;Agent"/>
  </owl:Class>

  <owl:Class rdf:about="#ShipBerth">
    <rdfs:comment>ShipBerth is the class of areas where a 

single Ship may be moored, either at an Anchorage, Pier, or dock.</rdfs:comment>
    <rdfs:subClassOf rdf:resource="&SUMO;WaterArea"/>
    <owl:disjointWith rdf:resource="#Anchorage"/>
    <owl:disjointWith rdf:resource="#DeepDraftWaterArea"/>
    <owl:disjointWith rdf:resource="#Harbor"/>
    <owl:disjointWith rdf:resource="&Mid-level-ontology;Waterway"/>
  </owl:Class>

  <owl:Class rdf:about="#ShipBerthing">
    <rdfs:comment>ShipBerthing is the class of 

Translocation processes in which a vessel is brought to a 

mooring, at dockside or anchorage.</rdfs:comment>
    <rdfs:subClassOf rdf:resource="&Mid-level-ontology;Arriving"/>
  </owl:Class>

  <owl:Class rdf:about="#ShipCabin">
    <rdfs:comment>ShipCabin is the subclass of all 

ShipCompartments for accommodating Humans aboard a ship.</rdfs:comment>
    <rdfs:subClassOf rdf:resource="#HumanHabitationArtifact"/>
    <rdfs:subClassOf rdf:resource="#ShipCompartment"/>
  </owl:Class>

  <owl:Class rdf:about="#ShipCompartment">
    <rdfs:comment>ShipCompartment is the subclass of 

Artifacts that includes any fully or partly bounded section of a 

Ship.</rdfs:comment>
    <rdfs:subClassOf rdf:resource="&SUMO;Artifact"/>
    <owl:disjointWith rdf:resource="#HumanHabitationArtifact"/>
  </owl:Class>

  <owl:Class rdf:about="#ShipDeck">
    <rdfs:comment>ShipDeck is the class of decks on a ship, 

considered as spaces or Regions in which passengers and crew work, 

live, or ride, or in which machinery and cargo are stored on a 

Ship.</rdfs:comment>
    <rdfs:subClassOf rdf:resource="&SUMO;Artifact"/>
    <owl:disjointWith rdf:resource="#HumanHabitationArtifact"/>
  </owl:Class>

  <owl:Class rdf:about="#ShipHatch">
    <rdfs:comment>ShipHatch is a subclass of Holes that are 

made by openings through the deck of a ship into a ShipCompartment.</rdfs:comment>
    <rdfs:subClassOf rdf:resource="&SUMO;Hole"/>
  </owl:Class>

  <owl:Class rdf:about="#ShipHold">
    <rdfs:comment>ShipHold is the subclass of ShipCompartments 

that are intended for the stowage of general cargo.</rdfs:comment>
    <rdfs:subClassOf rdf:resource="#ShipCompartment"/>
  </owl:Class>

  <owl:Class rdf:about="#ShipHull">
    <rdfs:comment>ShipHull is the class of hulls of Ships or 

other Watercraft.</rdfs:comment>
    <rdfs:subClassOf rdf:resource="&SUMO;Artifact"/>
    <owl:disjointWith rdf:resource="#HumanHabitationArtifact"/>
  </owl:Class>

  <owl:Class rdf:about="#ShipRegister">
    <rdfs:comment>ShipRegister is the class of ContentBearingObjects that contain an 

record of each Ship and owner registered with the maritime authorities 

of the Nation or OverseasArea to which the register belongs.  Ships 

entered in the ShipRegister of a given GeopoliticalArea fly the flag 

of that area and are subject to its maritime regulations and rules of 

taxation.</rdfs:comment>
    <rdfs:subClassOf rdf:resource="&SUMO;ContentBearingObject"/>
    <owl:disjointWith rdf:resource="#AidToNavigation"/>
    <owl:disjointWith rdf:resource="#BillOfLading"/>
    <owl:disjointWith rdf:resource="#CargoManifest"/>
    <owl:disjointWith rdf:resource="#CertificateOfRegistry"/>
  </owl:Class>

  <owl:Class rdf:about="#Shipping">
    <rdfs:comment>Shipping is the subclass of Transportation 

events in which goods are transported from one place to another by an 

agent who is entrusted with the goods temporarily just in order to move 

them.  Shipping may be done within an organization or it may be done 

by an outside commercial agent.  See CommercialShipping.</rdfs:comment>
    <rdfs:subClassOf rdf:resource="&SUMO;Transportation"/>
  </owl:Class>

  <owl:Class rdf:about="#ShippingChannel">
    <rdfs:subClassOf rdf:resource="&Mid-level-ontology;Waterway"/>
    <owl:disjointWith rdf:resource="&Mid-level-ontology;Canal"/>
  </owl:Class>

  <owl:Class rdf:about="#ShippingLane">
    <rdfs:subClassOf rdf:resource="&Mid-level-ontology;Waterway"/>
    <owl:disjointWith rdf:resource="&Mid-level-ontology;Canal"/>
  </owl:Class>

  <owl:Class rdf:about="#ShortSeaPassengerShip">
    <rdfs:comment>ShortSeaPassengerShip is the 

subclass of PassengerShips that are used for short trips; passenger 

ferries.</rdfs:comment>
    <rdfs:label>ferry</rdfs:label>
    <rdfs:label>short sea passenger ship</rdfs:label>
    <rdfs:subClassOf rdf:resource="#PassengerShip"/>
  </owl:Class>

  <owl:Class rdf:about="#SingleTrafficLane">
    <rdfs:comment>SingleTrafficLane is the subclass of 

Transitways that are wide enough for passage of only one Vehicle 

at a time.  Note that a SingleTrafficLane may be part of a larger 

Transitway.</rdfs:comment>
    <rdfs:subClassOf rdf:resource="&SUMO;Transitway"/>
    <owl:disjointWith rdf:resource="#AirTransitway"/>
    <owl:disjointWith rdf:resource="#OneWayTransitway"/>
    <owl:disjointWith rdf:resource="#TransitRoute"/>
    <owl:disjointWith rdf:resource="&Mid-level-ontology;Pipeline"/>
    <owl:disjointWith rdf:resource="&Mid-level-ontology;TransitwayJunction"/>
    <owl:disjointWith rdf:resource="&Mid-level-ontology;Tunnel"/>
    <owl:disjointWith rdf:resource="&Mid-level-ontology;Waterway"/>
    <owl:disjointWith rdf:resource="&SUMO;LandTransitway"/>
  </owl:Class>

  <owl:Class rdf:about="#SleeperRailcar">
    <rdfs:comment>SleeperRailcar is the subclass of 

Railcars that are designed with sleeping accommodations for 

passengers.</rdfs:comment>
    <rdfs:subClassOf rdf:resource="#PassengerRailwayCar"/>
    <rdfs:subClassOf rdf:resource="#Railcar"/>
  </owl:Class>

  <owl:Class rdf:about="#SludgeDisposalVessel">
    <rdfs:subClassOf rdf:resource="&Mid-level-ontology;Ship"/>
    <owl:disjointWith rdf:resource="#CableShip"/>
    <owl:disjointWith rdf:resource="#CargoShip"/>
    <owl:disjointWith rdf:resource="#CraneShip"/>
    <owl:disjointWith rdf:resource="#Dredger"/>
    <owl:disjointWith rdf:resource="#DrillingShip"/>
    <owl:disjointWith rdf:resource="#IceBreakerShip"/>
    <owl:disjointWith rdf:resource="#MerchantMarineShip"/>
    <owl:disjointWith rdf:resource="#MotorHopper"/>
    <owl:disjointWith rdf:resource="#OffshoreSupplyShip"/>
    <owl:disjointWith rdf:resource="#OffshoreSupportShip"/>
    <owl:disjointWith rdf:resource="#OffshoreWellProductionShip"/>
    <owl:disjointWith rdf:resource="#PassengerShip"/>
    <owl:disjointWith rdf:resource="#ResearchShip"/>
  </owl:Class>

  <owl:Class rdf:about="#SpecializedTankerShip">
    <rdfs:comment>SpecializedTankerShip is the 

subclass of CargoShips that are tankers designed for some special 

cargo other than gas or oil.</rdfs:comment>
    <rdfs:subClassOf rdf:resource="#CargoShip"/>
  </owl:Class>

  <owl:Class rdf:about="#SpineCar">
    <rdfs:comment>SpineCar is a subset of articulated Flatcars 

used to carry truck trailers or containers.</rdfs:comment>
    <rdfs:subClassOf rdf:resource="#Flatcar"/>
  </owl:Class>

  <owl:Class rdf:about="#SportUtilityVehicle">
    <rdfs:subClassOf rdf:resource="&Mid-level-ontology;Automobile"/>
  </owl:Class>

  <owl:Class rdf:about="#StandardGaugeRailway">
    <rdfs:comment>StandardGaugeRailway is the class of 

Railway that has a distance of 1.44 Meters between its rails.</rdfs:comment>
    <rdfs:subClassOf rdf:resource="&Mid-level-ontology;Railway"/>
  </owl:Class>

  <owl:Class rdf:about="#Street">
    <rdfs:comment>Street is the subclass of Roadways that are 

located in a City and have numbered addresses assigned to them.</rdfs:comment>
    <rdfs:subClassOf rdf:resource="&SUMO;Roadway"/>
  </owl:Class>

  <owl:Class rdf:about="#Streetcar">
    <rdfs:comment>Streetcar is the subclass of 

ElectrifiedRailwayCars that run on tracks laid into, along, or 

beside city Streets.</rdfs:comment>
    <rdfs:subClassOf rdf:resource="#ElectrifiedRailwayCar"/>
  </owl:Class>

  <owl:Class rdf:about="#TankCar">
    <rdfs:comment>TankCar is the subclass of enclosed FreightCars 

that are Containers used to carry fluids.</rdfs:comment>
    <rdfs:subClassOf rdf:resource="#FreightCar"/>
    <rdfs:subClassOf rdf:resource="&Mid-level-ontology;Container"/>
    <owl:disjointWith rdf:resource="#CargoContainer"/>
  </owl:Class>

  <owl:Class rdf:about="#TrackGauge">
    <rdfs:comment>TrackGauge is the collection of width 

attributes that characterize Railways, based on the regular distance 

maintained between the two rails of the RailroadTrack.  Precisely, the 

measurement of track gauge is the distance between the inner vertical 

surfaces of the heads of the rails.  Track gauge attributes include 

BroadGauge, DualGauge, StandardGauge, and NarrowGauge.  

TrackGauge may be attributed both to a Railway and to the 

RailroadTrack that is its main component.</rdfs:comment>
    <rdfs:subClassOf rdf:resource="&SUMO;InternalAttribute"/>
  </owl:Class>

  <owl:Class rdf:about="#TractorTrailer">
    <rdfs:comment>TractorTrailer is the subclass of 

RoadVehicles that are truck tractor- truck trailer combinations.</rdfs:comment>
    <rdfs:label>semi-trailer</rdfs:label>
    <rdfs:label>tractor-trailer</rdfs:label>
    <rdfs:subClassOf rdf:resource="#SelfPoweredRoadVehicle"/>
    <rdfs:subClassOf rdf:resource="&Mid-level-ontology;RoadVehicle"/>
    <owl:disjointWith rdf:resource="&Mid-level-ontology;Automobile"/>
  </owl:Class>

  <owl:Class rdf:about="#TradeEmbargo">
    <rdfs:comment>TradeEmbargo is the subclass of 

OrganizationalProcesses in which commerce and transportation of goods 

is forbidden by a Nation or Organization that has some means of 

enforcing such a ban.  A TradeEmbargo may be against a specified class 

of goods (e.g., weapons of mass destruction) or against a particular 

Nation or Nations.  See embargoedTradeType and embargoedArea.</rdfs:comment>
    <rdfs:subClassOf rdf:resource="&SUMO;OrganizationalProcess"/>
  </owl:Class>

  <owl:Class rdf:about="#TrafficControlProcess">
    <rdfs:comment>TrafficControlProcess is a  

subclass of Guiding, representing events in which an Agent directly  

or indirectly guides the Motion of traffic in a Region.</rdfs:comment>
    <rdfs:subClassOf rdf:resource="&SUMO;Guiding"/>
  </owl:Class>

  <owl:Class rdf:about="#TrafficLight">
    <rdfs:comment>TrafficLight is the subclass of 

TrafficSignal representing traffic lights whose function is to signal 

traffic to stop (or go), including blinkers or three-way stop lights.</rdfs:comment>
    <rdfs:subClassOf rdf:resource="#TrafficSignal"/>
    <rdfs:subClassOf rdf:resource="&Mid-level-ontology;ElectricDevice"/>
    <owl:disjointWith rdf:resource="&Mid-level-ontology;ElectricMotor"/>
  </owl:Class>

  <owl:Class rdf:about="#TrafficSignal">
    <rdfs:comment>TrafficSignal is the subclass of 

TransportationControlDevices that are designed to control the flow 

of Roadway traffic.  TrafficSignals perform some signalling process, 

typically using light or sound.</rdfs:comment>
    <rdfs:subClassOf rdf:resource="#TransportationControlDevice"/>
  </owl:Class>

  <owl:Class rdf:about="#Trail">
    <SUMO:disjoint rdf:resource="&Mid-level-ontology;Railway"/>
    <rdf:type rdf:resource="&owl;Thing"/>
    <rdfs:comment>Trail is the subclass of LandTransitways that are 

walkable, skateable, bikeable paths.  In general, Trails are not 

intended for use by motor Vehicles.</rdfs:comment>
    <rdfs:subClassOf rdf:resource="&SUMO;LandTransitway"/>
  </owl:Class>

  <owl:Class rdf:about="#TrainAssembly">
    <rdfs:comment>TrainAssembly is the process of putting 

together a single Train from one or more Locomotives and Railcars.</rdfs:comment>
    <rdfs:subClassOf rdf:resource="&SUMO;Attaching"/>
    <rdfs:subClassOf rdf:resource="&SUMO;Making"/>
  </owl:Class>

  <owl:Class rdf:about="#TrainStation">
    <rdfs:comment>TrainStation is the subclass of 

Buildings that are located at a RailwayTerminal and used in support  

of its functions, especially for the handling of passengers and freight.</rdfs:comment>
    <rdfs:subClassOf rdf:resource="&Mid-level-ontology;TerminalBuilding"/>
    <rdfs:subClassOf rdf:resource="&Mid-level-ontology;TransitTerminal"/>
  </owl:Class>

  <owl:Class rdf:about="#TransitRoute">
    <rdfs:comment>TransitRoute is the subclass of established 

Transitways that are routes officially recognized by some authority, 

civilian or military, and which are formally designated by name, headings, 

boundaries, or waypoints; for example, Bus routes or AirRoutes followed 

by Vehicles belonging to a CommercialCarrier.</rdfs:comment>
    <rdfs:subClassOf rdf:resource="&SUMO;Transitway"/>
    <owl:disjointWith rdf:resource="#AirTransitway"/>
    <owl:disjointWith rdf:resource="#OneWayTransitway"/>
    <owl:disjointWith rdf:resource="#SingleTrafficLane"/>
    <owl:disjointWith rdf:resource="&Mid-level-ontology;Pipeline"/>
    <owl:disjointWith rdf:resource="&Mid-level-ontology;TransitwayJunction"/>
    <owl:disjointWith rdf:resource="&Mid-level-ontology;Tunnel"/>
    <owl:disjointWith rdf:resource="&Mid-level-ontology;Waterway"/>
    <owl:disjointWith rdf:resource="&SUMO;LandTransitway"/>
  </owl:Class>

  <owl:Class rdf:about="#TransitShelter">
    <rdfs:comment>TransitShelter is the class of 

structures that provide shelter for passengers waiting at a 

TransitStop.</rdfs:comment>
    <rdfs:subClassOf rdf:resource="#HumanHabitationArtifact"/>
  </owl:Class>

  <owl:Class rdf:about="#TransitStop">
    <rdfs:comment>TransitStop is the subclass of places 

where a vehicle of a scheduled or common carrier makes a stop to 

discharge or take on passengers or goods.</rdfs:comment>
    <rdfs:subClassOf rdf:resource="&SUMO;Region"/>
  </owl:Class>

  <owl:Class rdf:about="#TransitwayObstacle">
    <rdfs:comment>TransitwayObstacle is the general 

class of Objects that can act as obstacles to Motion along a 

Transitway.</rdfs:comment>
    <rdfs:subClassOf rdf:resource="&SUMO;Object"/>
  </owl:Class>

  <owl:Class rdf:about="#TransitwayState">
    <rdfs:comment>TransitwayState is the class of 

RelationalAttributes used to describe the state of a Transitway.  

This could include traffic congestion, limited visibility, or being 

ClosedForAllTraffic.</rdfs:comment>
    <rdfs:subClassOf rdf:resource="&SUMO;RelationalAttribute"/>
  </owl:Class>

  <owl:Class rdf:about="#TransportationAuthority">
    <rdfs:comment>TransportationAuthority is the class of Organizations that are 

responsible for one or more systems of transportation, usually within 

a particular GeopoliticalArea.</rdfs:comment>
    <rdfs:subClassOf rdf:resource="&SUMO;Organization"/>
  </owl:Class>

  <owl:Class rdf:about="#TransportationControlDevice">
    <rdfs:comment>TransportationControlDevice 

is a subclass of Devices that are used to direct, regulate, or control 

the flow of traffic or movement along a Transitway.</rdfs:comment>
    <rdfs:subClassOf rdf:resource="&SUMO;Device"/>
    <owl:disjointWith rdf:resource="#Axle"/>
    <owl:disjointWith rdf:resource="#CanalLockGate"/>
    <owl:disjointWith rdf:resource="&Mid-level-ontology;AnimalPoweredDevice"/>
  </owl:Class>

  <owl:Class rdf:about="#TransportationSchedule">
    <rdfs:comment>TransportationSchedule is the 

subclass of ContentBearingObjects that contain the schedule of trips 

planned by a transportation organization.</rdfs:comment>
    <rdfs:subClassOf rdf:resource="&SUMO;ContentBearingObject"/>
    <owl:disjointWith rdf:resource="#AidToNavigation"/>
    <owl:disjointWith rdf:resource="#BillOfLading"/>
    <owl:disjointWith rdf:resource="#CargoManifest"/>
    <owl:disjointWith rdf:resource="#CertificateOfRegistry"/>
  </owl:Class>

  <owl:Class rdf:about="#TransportationSystem">
    <rdfs:comment>TransportationSystem is the 

subclass of complex Objects consisting of networks of Transitways 

and TransitJunctions that link together a number of GeographicRegions 

or TransitTerminals.  TransportationSystem covers worldwide 

networks, such as internationally recognized shipping lanes or air 

corridors, also route systems such as those flown by a single airline, 

as well as LocalTransitSystems such as BART (Bay Area Rapid Transit).</rdfs:comment>
    <rdfs:subClassOf rdf:resource="&SUMO;Object"/>
  </owl:Class>

  <owl:Class rdf:about="#Trip">
    <rdfs:comment>Trip is the subclass of Translocations that 

are complete motions along a TransitRoute or Transitway from one 

place to another.</rdfs:comment>
    <rdfs:subClassOf rdf:resource="&SUMO;Translocation"/>
  </owl:Class>

  <owl:Class rdf:about="#TruckTractor">
    <rdfs:comment>TruckTractor is the subclass of Trucks 

that are used to tow truck trailers.  Truck tractors are the cab portions 

of tractor-trailers.  See also TruckTrailer.</rdfs:comment>
    <rdfs:subClassOf rdf:resource="&Mid-level-ontology;Truck"/>
  </owl:Class>

  <owl:Class rdf:about="#TruckTrailer">
    <rdfs:comment>TruckTrailer is the subclass of Trailers 

that are towed by TruckTractors.  These are the trailers used in 

tractor-trailer (semi-trailer) rigs.</rdfs:comment>
    <rdfs:subClassOf rdf:resource="&Mid-level-ontology;Trailer"/>
  </owl:Class>

  <owl:Class rdf:about="#Tugboat">
    <rdfs:comment>Tugboat is the subclass of diesel-powered 

boats that are used for moving Barges, barge trains, and oil platforms, 

or for rescue and salvage at sea.</rdfs:comment>
    <rdfs:subClassOf rdf:resource="#DisplacementHullWatercraft"/>
    <rdfs:subClassOf rdf:resource="#SelfPoweredVehicle"/>
    <owl:disjointWith rdf:resource="#ElectrifiedRailwayCar"/>
    <owl:disjointWith rdf:resource="#Locomotive"/>
    <owl:disjointWith rdf:resource="&Mid-level-ontology;Airplane"/>
  </owl:Class>

  <owl:Class rdf:about="#TurbojetEngine">
    <rdfs:subClassOf rdf:resource="&Mid-level-ontology;InternalCombustionEngine"/>
  </owl:Class>

  <owl:Class rdf:about="#TurbopropAirplane">
    <rdfs:comment>TurbopropAirplane is the subclass of 

Aircraft whose engines use a combination of propellers and jet power.</rdfs:comment>
    <rdfs:label>propjet</rdfs:label>
    <rdfs:label>turboprop</rdfs:label>
    <rdfs:subClassOf rdf:resource="&Mid-level-ontology;Airplane"/>
    <owl:disjointWith rdf:resource="#JetAirplane"/>
  </owl:Class>

  <owl:Class rdf:about="#UnimodalTransportationSystem">
    <rdfs:comment>UnimodalTransportationSystem is the class of TransportationSystems 

that include only one type of Transitway or accommodate a single type of 

TransportationDevice.</rdfs:comment>
    <rdfs:subClassOf rdf:resource="#TransportationSystem"/>
  </owl:Class>

  <owl:Class rdf:about="#UnpavedRunway">
    <rdf:type rdf:resource="&owl;Thing"/>
    <rdfs:comment>UnpavedRunways include Runways with 

grass, dirt, sand, or gravel surfaces.  Contrast with PavedRunway.</rdfs:comment>
    <rdfs:subClassOf rdf:resource="&Mid-level-ontology;Runway"/>
  </owl:Class>

  <owl:Class rdf:about="#UreaCarrierShip">
    <rdfs:comment>UreaCarrierShip is the 

subclass of CargoShips that carry Urea.</rdfs:comment>
    <rdfs:subClassOf rdf:resource="#DryBulkCarrierShip"/>
  </owl:Class>

  <owl:Class rdf:about="#UserPoweredVehicle">
    <rdf:type rdf:resource="&owl;Thing"/>
    <rdfs:comment>UserPoweredVehicle is the subclass of 

Vehicles whose power source is the rider or user.  Examples: Bicycles, 

Canoes, grocery carts.</rdfs:comment>
    <rdfs:subClassOf rdf:resource="&Mid-level-ontology;UserPoweredDevice"/>
    <rdfs:subClassOf rdf:resource="&SUMO;Vehicle"/>
  </owl:Class>

  <owl:Class rdf:about="#VehicleCarrierShip">
    <rdfs:subClassOf rdf:resource="#RollOnRollOffCargoShip"/>
  </owl:Class>

  <owl:Class rdf:about="#VehicleClassForFHWA">
    <rdfs:comment>VehicleClassForFHWA is a subclass 

of SetOrClass that contains thirteen subclasses used by the 

UnitedStatesFederalHighwayAdministration (and also many U.S. states) 

as a basis for vehicle fees and usage statistics.</rdfs:comment>
    <rdfs:subClassOf rdf:resource="&SUMO;SetOrClass"/>
    <owl:disjointWith rdf:resource="#ModeOfTransit"/>
  </owl:Class>

  <owl:Class rdf:about="#VehicleCrew">
    <rdfs:comment>A VehicleCrew is an Organization of 

people who perform various functions aboard a Ship, Aircraft, 

Train, or other transportation vehicle.</rdfs:comment>
    <rdfs:subClassOf rdf:resource="&SUMO;Organization"/>
  </owl:Class>

  <owl:Class rdf:about="#VehicleRegistration">
    <rdfs:comment>VehicleRegistration is the class 

of official documents containing information about a vehicle's ownership 

and identifying characteristics, as required by the appropriate authority 

for the type and location of individual vehicles.</rdfs:comment>
    <rdfs:subClassOf rdf:resource="&SUMO;ContentBearingObject"/>
    <owl:disjointWith rdf:resource="#AidToNavigation"/>
    <owl:disjointWith rdf:resource="#BillOfLading"/>
    <owl:disjointWith rdf:resource="#CargoManifest"/>
    <owl:disjointWith rdf:resource="#CertificateOfRegistry"/>
    <owl:disjointWith rdf:resource="#CrewList"/>
  </owl:Class>

  <owl:Class rdf:about="#VehicleWheel">
    <rdfs:comment>VehicleWheel is a class of cylindrical 

Devices used to move a RoadVehicle along a road, running either  

directly on the wheel rims or on tires attached to the wheel rims.</rdfs:comment>
    <rdfs:subClassOf rdf:resource="&Mid-level-ontology;Wheel"/>
    <rdfs:subClassOf rdf:resource="&SUMO;Device"/>
    <owl:disjointWith rdf:resource="#Axle"/>
    <owl:disjointWith rdf:resource="#CanalLockGate"/>
    <owl:disjointWith rdf:resource="&Mid-level-ontology;AnimalPoweredDevice"/>
  </owl:Class>

  <owl:Class rdf:about="#WaterTransportationSystem">
    <rdfs:comment>WaterTransportationSystem 

is the subclass of TransportationSystems whose routes are Waterways.</rdfs:comment>
    <rdfs:subClassOf rdf:resource="#TransportationSystem"/>
  </owl:Class>

  <owl:Class rdf:about="#WaterwayJunction">
    <rdfs:comment>WaterwayJunction is the subclass of 

TransitwayJunctions where two or more Waterways come together.</rdfs:comment>
    <rdfs:subClassOf rdf:resource="&Mid-level-ontology;TransitwayJunction"/>
    <rdfs:subClassOf rdf:resource="&Mid-level-ontology;Waterway"/>
    <owl:disjointWith rdf:resource="#RailwayJunction"/>
    <owl:disjointWith rdf:resource="&Mid-level-ontology;Canal"/>
  </owl:Class>

  <owl:Class rdf:about="#WhalingShip">
    <rdfs:subClassOf rdf:resource="#FishingVessel"/>
  </owl:Class>

  <owl:Class rdf:about="#WindPoweredDevice">
    <rdfs:comment>WindPoweredDevice is the 

subclass of Devices that are moved by wind power, including 

Sailboats, GliderAirplanes, and windmills.</rdfs:comment>
    <rdfs:subClassOf rdf:resource="&SUMO;Device"/>
    <owl:disjointWith rdf:resource="#Axle"/>
    <owl:disjointWith rdf:resource="#CanalLockGate"/>
    <owl:disjointWith rdf:resource="&Mid-level-ontology;AnimalPoweredDevice"/>
  </owl:Class>

  <owl:Class rdf:about="#WoodChipsCarrierShip">
    <rdfs:comment>WoodChipsCarrierShip is the 

subclass of CargoShips that carry wood chips.</rdfs:comment>
    <rdfs:subClassOf rdf:resource="#DryBulkCarrierShip"/>
  </owl:Class>

  <owl:Class rdf:about="http://reliant.teknowledge.com/DAML/Communications.owl#ElectronicDevice"/>
  <owl:Class rdf:about="http://reliant.teknowledge.com/DAML/Economy.owl#PetroleumProduct"/>
  <owl:Class rdf:about="http://reliant.teknowledge.com/DAML/Geography.owl#Coal"
             rdfs:label="coal">
    <rdfs:subClassOf rdf:resource="&Mid-level-ontology;FossilFuel"/>
  </owl:Class>

  <owl:Class rdf:about="http://reliant.teknowledge.com/DAML/Geography.owl#Dam">
    <rdfs:subClassOf rdf:resource="#TransitwayObstacle"/>
  </owl:Class>

  <owl:Class rdf:about="&Government;InternationalOrganization"/>
  <owl:Class rdf:about="&Mid-level-ontology;Address"/>
  <owl:Class rdf:about="&Mid-level-ontology;Aircraft">
    <rdfs:comment>Aircraft is the subclass of TransportationDevices that travel 

through air.  Aircraft are intermodal transportation devices, since 

they must take off and land either on land or in water.</rdfs:comment>
    <rdfs:subClassOf rdf:resource="&SUMO;TransportationDevice"/>
    <owl:disjointWith rdf:resource="#CargoContainer"/>
    <owl:disjointWith rdf:resource="&Mid-level-ontology;Crane"/>
    <owl:disjointWith rdf:resource="&Mid-level-ontology;SelfPoweredDevice"/>
    <owl:disjointWith rdf:resource="&Mid-level-ontology;Watercraft"/>
    <owl:disjointWith rdf:resource="&SUMO;Vehicle"/>
  </owl:Class>

  <owl:Class rdf:about="&Mid-level-ontology;Airplane">
    <rdfs:comment>Airplane is the subclass of Aircraft that 

are fixed-wing aircraft which carry their own power sources.  Airplane 

includes jet airplanes and propeller planes, but not GliderAirplanes.</rdfs:comment>
    <rdfs:subClassOf rdf:resource="#SelfPoweredVehicle"/>
    <rdfs:subClassOf rdf:resource="&Mid-level-ontology;Aircraft"/>
    <owl:disjointWith rdf:resource="#CabCar"/>
    <owl:disjointWith rdf:resource="#ElectrifiedRailwayCar"/>
    <owl:disjointWith rdf:resource="#EmergencyVehicle"/>
    <owl:disjointWith rdf:resource="#GliderAirplane"/>
    <owl:disjointWith rdf:resource="#Heliport"/>
    <owl:disjointWith rdf:resource="#Locomotive"/>
    <owl:disjointWith rdf:resource="#MotorizedRailwayCar"/>
    <owl:disjointWith rdf:resource="#PersonalWatercraft"/>
    <owl:disjointWith rdf:resource="#SelfPoweredRoadVehicle"/>
    <owl:disjointWith rdf:resource="#Tugboat"/>
    <owl:disjointWith rdf:resource="&Mid-level-ontology;Helicopter"/>
    <owl:disjointWith rdf:resource="&Mid-level-ontology;Train"/>
  </owl:Class>

  <owl:Class rdf:about="&Mid-level-ontology;Airport">
    <rdfs:comment>Airport is the subclass of TransitTerminals 

designed for Airplanes (fixed-wing Aircraft).</rdfs:comment>
    <rdfs:subClassOf rdf:resource="#AirTransitway"/>
    <rdfs:subClassOf rdf:resource="&Mid-level-ontology;TransitTerminal"/>
    <rdfs:subClassOf rdf:resource="&SUMO;LandTransitway"/>
    <owl:disjointWith rdf:resource="#AirRoute"/>
    <owl:disjointWith rdf:resource="#Heliport"/>
  </owl:Class>

  <owl:Class rdf:about="&Mid-level-ontology;AnimalPoweredDevice">
    <rdfs:comment>AnimalPoweredDevice is the subclass 

of Devices that function with power supplied by animals.  Examples: 

oxcarts, horse-drawn plows, mule-driven mills.</rdfs:comment>
    <rdfs:subClassOf rdf:resource="&SUMO;Device"/>
    <owl:disjointWith rdf:resource="#Axle"/>
    <owl:disjointWith rdf:resource="#CanalLockGate"/>
    <owl:disjointWith rdf:resource="#Drawbridge"/>
    <owl:disjointWith rdf:resource="#HumanPoweredDevice"/>
    <owl:disjointWith rdf:resource="#TransportationControlDevice"/>
    <owl:disjointWith rdf:resource="#VehicleWheel"/>
    <owl:disjointWith rdf:resource="#WindPoweredDevice"/>
    <owl:disjointWith rdf:resource="&Mid-level-ontology;Battery"/>
    <owl:disjointWith rdf:resource="&Mid-level-ontology;HoistingDevice"/>
    <owl:disjointWith rdf:resource="&Mid-level-ontology;MaterialHandlingEquipment"/>
    <owl:disjointWith rdf:resource="&Mid-level-ontology;UserPoweredDevice"/>
  </owl:Class>

  <owl:Class rdf:about="&Mid-level-ontology;Arriving"/>
  <owl:Class rdf:about="&Mid-level-ontology;AtmosphericRegion"/>
  <owl:Class rdf:about="&Mid-level-ontology;Automobile">
    <rdfs:comment>Automobile is a subclass of SelfPoweredRoadVehicles including 

PassengerCars, FamilyVans, LightTrucks, and SportUtilityVehicles.  

In general, this class covers four-wheeled passenger road vehicles.</rdfs:comment>
    <rdfs:subClassOf rdf:resource="#SelfPoweredRoadVehicle"/>
    <owl:disjointWith rdf:resource="#Bus"/>
    <owl:disjointWith rdf:resource="#EmergencyRoadVehicle"/>
    <owl:disjointWith rdf:resource="#MotorScooter"/>
    <owl:disjointWith rdf:resource="#Motorcycle"/>
    <owl:disjointWith rdf:resource="#TractorTrailer"/>
    <owl:disjointWith rdf:resource="&Mid-level-ontology;Truck"/>
  </owl:Class>

  <owl:Class rdf:about="&Mid-level-ontology;Battery">
    <rdfs:comment>Battery is a subclass of Device.  Batteries are 

devices that use chemical means to store or produce electrical power.</rdfs:comment>
    <rdfs:subClassOf rdf:resource="&SUMO;Device"/>
    <owl:disjointWith rdf:resource="#Axle"/>
    <owl:disjointWith rdf:resource="#CanalLockGate"/>
    <owl:disjointWith rdf:resource="&Mid-level-ontology;AnimalPoweredDevice"/>
  </owl:Class>

  <owl:Class rdf:about="&Mid-level-ontology;Bridge">
    <rdfs:comment>Bridge is the subclass of LandTransitways 

that are Artifacts crossing over water or other obstacles to motion, 

both positive (e.g., railroad tracks or a wall) or negative (a chasm). 

A Bridge provides a path for foot traffic, RoadVehicles, 

Trains, or other land vehicles.  Bridge includes FixedBridges and 

PortableBridges.</rdfs:comment>
    <rdfs:subClassOf rdf:resource="&SUMO;LandTransitway"/>
    <rdfs:subClassOf rdf:resource="&SUMO;StationaryArtifact"/>
    <owl:disjointWith rdf:resource="#Bulkhead"/>
    <owl:disjointWith rdf:resource="#CanalLock"/>
    <owl:disjointWith rdf:resource="#CanalStructure"/>
    <owl:disjointWith rdf:resource="#Pier"/>
    <owl:disjointWith rdf:resource="&Mid-level-ontology;RailroadTrack"/>
    <owl:disjointWith rdf:resource="&Mid-level-ontology;Railway"/>
    <owl:disjointWith rdf:resource="&Mid-level-ontology;TransitTerminal"/>
    <owl:disjointWith rdf:resource="&Mid-level-ontology;Tunnel"/>
  </owl:Class>

  <owl:Class rdf:about="&Mid-level-ontology;Canal">
    <rdfs:comment>Canal is the subclass of navigable Waterways 

flowing through an artificial course (CanalStructure) designed for 

the passage of Ships from one natural BodyOfWater to another.  In many 

cases, CanalLocks are used to compensate for the difference in water 

level between the linked bodies of water.</rdfs:comment>
    <rdfs:subClassOf rdf:resource="&Mid-level-ontology;Waterway"/>
    <owl:disjointWith rdf:resource="#SeaLane"/>
    <owl:disjointWith rdf:resource="#ShippingChannel"/>
    <owl:disjointWith rdf:resource="#ShippingLane"/>
    <owl:disjointWith rdf:resource="#WaterwayJunction"/>
  </owl:Class>

  <owl:Class rdf:about="&Mid-level-ontology;CommonCarrier">
    <rdfs:comment>CommonCarrier is the subclass of 

TransportationCompany whose instances offer services fairly to all 

customers, according to regular routes and schedules.  Contrast with 

ContractCarrier.</rdfs:comment>
    <rdfs:subClassOf rdf:resource="#CommercialCarrier"/>
  </owl:Class>

  <owl:Class rdf:about="&Mid-level-ontology;Container"/>
  <owl:Class rdf:about="&Mid-level-ontology;ContractCarrier">
    <rdfs:comment>ContractCarrier is the subclass of 

TransportationCompany whose instances offer services to individual 

customers, under contract.  Contrast with CommonCarrier.</rdfs:comment>
    <rdfs:subClassOf rdf:resource="#CommercialCarrier"/>
  </owl:Class>

  <owl:Class rdf:about="&Mid-level-ontology;Crane">
    <rdfs:comment>Crane is a subclass of mechanical Devices 

that consist of a HoistingDevice on a moveable boom, designed to 

assist in moving heavy loads.</rdfs:comment>
    <rdfs:subClassOf rdf:resource="&SUMO;TransportationDevice"/>
    <owl:disjointWith rdf:resource="#CargoContainer"/>
    <owl:disjointWith rdf:resource="&Mid-level-ontology;Aircraft"/>
    <owl:disjointWith rdf:resource="&Mid-level-ontology;SelfPoweredDevice"/>
    <owl:disjointWith rdf:resource="&Mid-level-ontology;Watercraft"/>
    <owl:disjointWith rdf:resource="&SUMO;Vehicle"/>
  </owl:Class>

  <SUMO:UnitOfMeasure rdf:about="&Mid-level-ontology;CubicFoot">
    <rdf:type rdf:resource="&owl;Class"/>
    <rdfs:comment>CubicFoot is a unit for measuring volume, 

equal to a volume of one foot length in each dimension of length, width, 

and height.</rdfs:comment>
    <rdfs:subClassOf rdf:resource="&SUMO;VolumeMeasure"/>
  </SUMO:UnitOfMeasure>

  <owl:Class rdf:about="&Mid-level-ontology;Cycle"/>
  <owl:Class rdf:about="&Mid-level-ontology;DeviceStateAttribute">
    <rdfs:comment>DeviceStateAttribute is the class 

of attributes that represent different states that a Device may be in.  

Examples: DeviceOff and DeviceOn, DeviceOpen and DeviceClosed.</rdfs:comment>
    <rdfs:subClassOf rdf:resource="&SUMO;Attribute"/>
    <owl:disjointWith rdf:resource="#AirportClassification"/>
  </owl:Class>

  <owl:Class rdf:about="&Mid-level-ontology;DieselEngine">
    <rdfs:comment>DieselEngine is the subclass of 

InternalCombustionEngines that use DieselFuel as their resource.</rdfs:comment>
    <rdfs:subClassOf rdf:resource="&Mid-level-ontology;InternalCombustionEngine"/>
  </owl:Class>

  <owl:Class rdf:about="&Mid-level-ontology;DieselFuel">
    <rdfs:comment>DieselFuel is the subclass of FossilFuel 

that represents the kind of heavy fuel oils used in DieselEngines.</rdfs:comment>
    <rdfs:subClassOf rdf:resource="&Mid-level-ontology;FossilFuel"/>
  </owl:Class>

  <owl:Class rdf:about="&Mid-level-ontology;ElectricDevice"/>
  <owl:Class rdf:about="&Mid-level-ontology;ElectricMotor">
    <rdfs:comment>ElectricMotor is the subclass of Engines 

that produce mechanical power from electricity.</rdfs:comment>
    <rdfs:subClassOf rdf:resource="&Mid-level-ontology;ElectricDevice"/>
    <rdfs:subClassOf rdf:resource="&Mid-level-ontology;Engine"/>
    <owl:disjointWith rdf:resource="#ElectrifiedRailwayCar"/>
    <owl:disjointWith rdf:resource="#NavigationLight"/>
    <owl:disjointWith rdf:resource="#RadioNavigationBeacon"/>
    <owl:disjointWith rdf:resource="#TrafficLight"/>
  </owl:Class>

  <owl:Class rdf:about="&Mid-level-ontology;ElectricalSignalling">
    <rdfs:comment>ElectricalSignalling is the 

subclass of Signalling processes that involve control of an electrical 

current.  Cf. ElectronicSignalling.</rdfs:comment>
    <rdfs:subClassOf rdf:resource="&Mid-level-ontology;Signalling"/>
  </owl:Class>

  <owl:Class rdf:about="&Mid-level-ontology;ElectronicSignalling">
    <rdfs:comment>ElectronicSignalling is the 

subclass of Signalling processes that involve a signal generated or 

controlled by a computer or other electronic device.</rdfs:comment>
    <rdfs:subClassOf rdf:resource="&Mid-level-ontology;ElectricalSignalling"/>
  </owl:Class>

  <owl:Class rdf:about="&Mid-level-ontology;Engine">
    <rdfs:comment>Engine is a subclass of Machine.  Engines 

are devices for converting some form of energy resource into mechanical 

power.</rdfs:comment>
    <rdfs:subClassOf rdf:resource="&SUMO;Machine"/>
  </owl:Class>

  <owl:Class rdf:about="&Mid-level-ontology;Expressway">
    <rdfs:comment>Expressway is the subclass of 

SurfacedRoadways that are multiple-lane, limited-access highways 

designed for rapid travel by self-powered motor vehicles.</rdfs:comment>
    <rdfs:subClassOf rdf:resource="&Mid-level-ontology;SurfacedRoadway"/>
  </owl:Class>

  <owl:Class rdf:about="&Mid-level-ontology;FossilFuel">
    <rdfs:comment>FossilFuel is the subclass of Fuel whose 

instances are derived from fossilized organic deposits, such as Coal 

and Petroleum.</rdfs:comment>
    <rdfs:subClassOf rdf:resource="&Mid-level-ontology;Fuel"/>
    <rdfs:subClassOf rdf:resource="&Mid-level-ontology;OrganicCompound"/>
  </owl:Class>

  <owl:Class rdf:about="&Mid-level-ontology;Fuel">
    <rdfs:comment>Fuel is the class of Substances that can be 

used as resources in Combustion processes in order to produce heat.  

Mechanical energy can be produced by burning fuel in an Engine.</rdfs:comment>
    <rdfs:subClassOf rdf:resource="&SUMO;Substance"/>
  </owl:Class>

  <owl:Class rdf:about="&Mid-level-ontology;Gasoline">
    <rdfs:comment>Gasoline is the subclass of FossilFuel that 

represents the light, volatile fuels used in GasolineEngines.</rdfs:comment>
    <rdfs:subClassOf rdf:resource="&Mid-level-ontology;FossilFuel"/>
  </owl:Class>

  <owl:Class rdf:about="&Mid-level-ontology;GasolineEngine">
    <rdfs:comment>GasolineEngine is the subclass of 

InternalCombustionEngines that use Gasoline as their resource.</rdfs:comment>
    <rdfs:subClassOf rdf:resource="&Mid-level-ontology;InternalCombustionEngine"/>
  </owl:Class>

  <owl:Class rdf:about="&Mid-level-ontology;Helicopter">
    <rdfs:comment>Helicopter is the subclass of Aircraft 

that have rotary wings.</rdfs:comment>
    <rdfs:subClassOf rdf:resource="#SelfPoweredVehicle"/>
    <rdfs:subClassOf rdf:resource="&Mid-level-ontology;Aircraft"/>
    <owl:disjointWith rdf:resource="&Mid-level-ontology;Airplane"/>
  </owl:Class>

  <owl:Class rdf:about="&Mid-level-ontology;HoistingDevice">
    <rdfs:comment>HoistingDevice is a subclass of 

mechanical Devices that provide a mechanical advantage in lifting 

and lowering, e.g., by use of a block and tackle.</rdfs:comment>
    <rdfs:subClassOf rdf:resource="&SUMO;Device"/>
    <owl:disjointWith rdf:resource="#Axle"/>
    <owl:disjointWith rdf:resource="#CanalLockGate"/>
    <owl:disjointWith rdf:resource="&Mid-level-ontology;AnimalPoweredDevice"/>
  </owl:Class>

  <owl:Class rdf:about="&Mid-level-ontology;InternalCombustionEngine">
    <rdfs:comment>InternalCombustionEngine is 

the subclass of Engines in which a heat reaction that occurs inside 

the engine is transformed into mechanical energy.</rdfs:comment>
    <rdfs:subClassOf rdf:resource="&Mid-level-ontology;Engine"/>
  </owl:Class>

  <owl:Class rdf:about="&Mid-level-ontology;InternationalLaw"/>
  <owl:Class rdf:about="&Mid-level-ontology;LandVehicle">
    <rdfs:comment>LandVehicle is the class of TransportationDevices that travel on 

LandTransitways.  The two main types of LandVehicle are RoadVehicle 

and RailwayVehicle, distinguished by their different types of interface 

with the land surface.</rdfs:comment>
    <rdfs:subClassOf rdf:resource="&SUMO;Vehicle"/>
  </owl:Class>

  <owl:Class rdf:about="&Mid-level-ontology;LegalCharge">
    <rdfs:subClassOf rdf:resource="&SUMO;RegulatoryProcess"/>
  </owl:Class>

  <owl:Class rdf:about="&Mid-level-ontology;License">
    <rdfs:comment>License is the subclass of Certificates that 

are official documents granted by a GovernmentOrganization and which 

authorize the performance of certain kinds of actions, e.g., driving or 

exporting.</rdfs:comment>
    <rdfs:subClassOf rdf:resource="&SUMO;Certificate"/>
  </owl:Class>

  <owl:Class rdf:about="&Mid-level-ontology;LightFixture"/>
  <owl:Class rdf:about="&Mid-level-ontology;LiquefiedPetroleumGas">
    <rdfs:comment>LiquefiedPetroleumGas is a 

compressed hydrocarbon gas.</rdfs:comment>
    <rdfs:subClassOf rdf:resource="http://reliant.teknowledge.com/DAML/Economy.owl#PetroleumProduct"/>
  </owl:Class>

  <owl:Class rdf:about="&Mid-level-ontology;MaterialHandlingEquipment">
    <rdfs:comment>MaterialHandlingEquipment 

is a class of Devices that are equipment used for handling goods and 

supplies more efficiently or safely.  Examples are cranes, hoists, 

forklifts, conveyors, racks, etc.</rdfs:comment>
    <rdfs:subClassOf rdf:resource="&SUMO;Device"/>
    <owl:disjointWith rdf:resource="#Axle"/>
    <owl:disjointWith rdf:resource="#CanalLockGate"/>
    <owl:disjointWith rdf:resource="&Mid-level-ontology;AnimalPoweredDevice"/>
  </owl:Class>

  <SUMO:UnitOfMeasure rdf:about="&Mid-level-ontology;MetricTon">
    <rdf:type rdf:resource="&owl;Class"/>
    <rdfs:comment>MetricTon is a UnitOfMeasure that represents 

a weight of 2,205 PoundMass.</rdfs:comment>
    <rdfs:subClassOf rdf:resource="&SUMO;MassMeasure"/>
  </SUMO:UnitOfMeasure>

  <owl:Class rdf:about="&Mid-level-ontology;MilitaryWatercraft">
    <rdf:type rdf:resource="&owl;Thing"/>
    <rdfs:comment>MilitaryWatercraft is the class of 

all Watercraft owned or leased for use by some MilitaryOrganization.</rdfs:comment>
    <rdfs:subClassOf rdf:resource="&Mid-level-ontology;Watercraft"/>
  </owl:Class>

  <owl:Class rdf:about="&Mid-level-ontology;OrganicCompound"/>
  <owl:Class rdf:about="&Mid-level-ontology;Pipeline">
    <rdfs:comment>Pipeline is the class of pipelines used 

to transport various kinds of fluids.</rdfs:comment>
    <rdfs:subClassOf rdf:resource="&SUMO;Transitway"/>
    <owl:disjointWith rdf:resource="#AirTransitway"/>
    <owl:disjointWith rdf:resource="#OneWayTransitway"/>
    <owl:disjointWith rdf:resource="#SingleTrafficLane"/>
    <owl:disjointWith rdf:resource="#TransitRoute"/>
    <owl:disjointWith rdf:resource="&Mid-level-ontology;TransitwayJunction"/>
    <owl:disjointWith rdf:resource="&Mid-level-ontology;Tunnel"/>
    <owl:disjointWith rdf:resource="&Mid-level-ontology;Waterway"/>
    <owl:disjointWith rdf:resource="&SUMO;LandTransitway"/>
  </owl:Class>

  <owl:Class rdf:about="&Mid-level-ontology;PortFacility">
    <rdfs:comment>PortFacility is the class of port 

complexes, including piers and docking space, moorings, cargo-handling 

and other support facilities for marine traffic.  A PortFacility is 

a TransitTerminal.  Ships are loaded and unloaded at a large 

PortFacility.</rdfs:comment>
    <rdfs:subClassOf rdf:resource="&Mid-level-ontology;TransitTerminal"/>
  </owl:Class>

  <owl:Class rdf:about="&Mid-level-ontology;Profession"/>
  <owl:Class rdf:about="&Mid-level-ontology;RadarOrSonar"/>
  <owl:Class rdf:about="&Mid-level-ontology;RailroadCompany"/>
  <owl:Class rdf:about="&Mid-level-ontology;RailroadTrack">
    <rdfs:comment>RailroadTrack is the class of 

StationaryArtifacts consisting of rails laid on supports to form 

a track for railway vehicles.  RailroadTrack is the basic component 

of a Railway, while the latter also includes any signalling devices, 

crossing markers, switches, and other artifacts along the tracks.</rdfs:comment>
    <rdfs:subClassOf rdf:resource="&SUMO;StationaryArtifact"/>
    <owl:disjointWith rdf:resource="#Bulkhead"/>
    <owl:disjointWith rdf:resource="#CanalLock"/>
    <owl:disjointWith rdf:resource="#CanalStructure"/>
    <owl:disjointWith rdf:resource="#Pier"/>
    <owl:disjointWith rdf:resource="&Mid-level-ontology;Bridge"/>
    <owl:disjointWith rdf:resource="&Mid-level-ontology;Railway"/>
    <owl:disjointWith rdf:resource="&Mid-level-ontology;TransitTerminal"/>
    <owl:disjointWith rdf:resource="&Mid-level-ontology;Tunnel"/>
  </owl:Class>

  <Transportation:ModeOfTransit rdf:about="&Mid-level-ontology;Railway">
    <rdf:type rdf:resource="&owl;Class"/>
    <rdfs:comment>Railway is the subclass of 

LandTransitways that have rails along which Trains may travel.  

A railway consists of the rail bed, sleepers, tracks, electric 

rails, switches, sensors, lights, crossing grades, and any other 

integral machinery or parts of a section of railway.</rdfs:comment>
    <rdfs:subClassOf rdf:resource="&SUMO;LandTransitway"/>
    <rdfs:subClassOf rdf:resource="&SUMO;StationaryArtifact"/>
    <owl:disjointWith rdf:resource="#Bulkhead"/>
    <owl:disjointWith rdf:resource="#CanalLock"/>
    <owl:disjointWith rdf:resource="#CanalStructure"/>
    <owl:disjointWith rdf:resource="#Pier"/>
    <owl:disjointWith rdf:resource="&Mid-level-ontology;Bridge"/>
    <owl:disjointWith rdf:resource="&Mid-level-ontology;RailroadTrack"/>
    <owl:disjointWith rdf:resource="&Mid-level-ontology;TransitTerminal"/>
    <owl:disjointWith rdf:resource="&Mid-level-ontology;Tunnel"/>
  </Transportation:ModeOfTransit>

  <owl:Class rdf:about="&Mid-level-ontology;Ramp">
    <rdfs:comment>Ramp is the class of Objects that are 

inclined planes used for moving objects from one level to another, 

especially used for wheeled vehicles and people who cannot climb stairs.</rdfs:comment>
    <rdfs:subClassOf rdf:resource="&SUMO;Object"/>
  </owl:Class>

  <owl:Class rdf:about="&Mid-level-ontology;RefrigeratedCompartment">
    <rdfs:comment>RefrigeratedCompartment is 

the subclass of Containers in which the temperature is reduced from 

that of the outside air, by some Cooling process.</rdfs:comment>
    <rdfs:subClassOf rdf:resource="&Mid-level-ontology;Container"/>
    <owl:disjointWith rdf:resource="#CargoContainer"/>
  </owl:Class>

  <owl:Class rdf:about="&Mid-level-ontology;RoadJunction">
    <rdfs:comment>RoadJunction is the subclass of 

TransitwayJunctions where two or more Roadways come together.</rdfs:comment>
    <rdfs:subClassOf rdf:resource="&Mid-level-ontology;TransitwayJunction"/>
    <rdfs:subClassOf rdf:resource="&SUMO;Roadway"/>
    <owl:disjointWith rdf:resource="#RailwayJunction"/>
  </owl:Class>

  <owl:Class rdf:about="&Mid-level-ontology;RoadVehicle">
    <rdfs:comment>RoadVehicle is the subclass of wheeled 

LandVehicles designed to travel on Roadways.</rdfs:comment>
    <rdfs:subClassOf rdf:resource="&Mid-level-ontology;LandVehicle"/>
  </owl:Class>

  <owl:Class rdf:about="&Mid-level-ontology;Runway">
    <rdfs:comment>Runway is the class of Transitways that are 

used for the takeoff and landing of Airplanes.  Runways are 

Transitways for an intermodal transit, which begins with a land transit 

and ends with air transit, or vice versa.  The Airspace immediately 

above (and adjacent to) a Runway is an AirTransitway.</rdfs:comment>
    <rdfs:subClassOf rdf:resource="&SUMO;LandTransitway"/>
  </owl:Class>

  <owl:Class rdf:about="&Mid-level-ontology;SelfPoweredDevice">
    <rdfs:comment>SelfPoweredDevice is the subclass of Devices whose action is 

powered by some kind of on-board component or power source (not the user).</rdfs:comment>
    <rdfs:subClassOf rdf:resource="&SUMO;TransportationDevice"/>
    <owl:disjointWith rdf:resource="#CargoContainer"/>
    <owl:disjointWith rdf:resource="&Mid-level-ontology;Aircraft"/>
    <owl:disjointWith rdf:resource="&Mid-level-ontology;Crane"/>
    <owl:disjointWith rdf:resource="&Mid-level-ontology;Watercraft"/>
    <owl:disjointWith rdf:resource="&SUMO;Vehicle"/>
  </owl:Class>

  <owl:Class rdf:about="&Mid-level-ontology;Ship">
    <rdfs:comment>Ship is the class of large Watercraft used 

for travel on oceans, seas, or very large lakes.</rdfs:comment>
    <rdfs:subClassOf rdf:resource="#DisplacementHullWatercraft"/>
  </owl:Class>

  <owl:Class rdf:about="&Mid-level-ontology;Signalling">
    <rdfs:comment>Signalling is the subclass of Guiding 

processes in which an agent, animate or inanimate, sends a signal to 

another Object.  In many cases, this signal will be an electrical or 

electronic one.  Some signals may directly control the behavior of 

the object signalled, while others may merely cause information to be 

presented.  Instances of electrical Signalling are typically more 

complex than simply than operation of a DeviceSwitch, though in some 

cases, Signalling involves remote activation of such a switch by another 

device.</rdfs:comment>
    <rdfs:subClassOf rdf:resource="&SUMO;Guiding"/>
  </owl:Class>

  <owl:Class rdf:about="&Mid-level-ontology;SteamEngine">
    <rdfs:comment>SteamEngine is the subclass of Engines 

that produce mechanical power from heat and steam pressure.</rdfs:comment>
    <rdfs:subClassOf rdf:resource="&Mid-level-ontology;Engine"/>
  </owl:Class>

  <owl:Class rdf:about="&Mid-level-ontology;SurfacedRoadway">
    <SUMO:disjoint rdf:resource="&Mid-level-ontology;UnsurfacedRoadway"/>
    <rdf:type rdf:resource="&owl;Thing"/>
    <rdfs:comment>SurfacedRoadway is the subclass of 

Roadways that have been improved by covering them with a substance 

to increase the hardness and smoothness of the surface.  Covering 

materials include pavement, concrete, asphalt, macadam, and gravel.</rdfs:comment>
    <rdfs:subClassOf rdf:resource="&SUMO;Roadway"/>
  </owl:Class>

  <owl:Class rdf:about="&Mid-level-ontology;TakingOff">
    <rdfs:subClassOf rdf:resource="#IntermodalTransportation"/>
  </owl:Class>

  <owl:Class rdf:about="&Mid-level-ontology;TerminalBuilding">
    <rdfs:comment>TerminalBuilding is the subclass of 

Buildings that are located at a TransitTerminal and used in support  

of its functions, especially for the handling of passengers and freight.</rdfs:comment>
    <rdfs:subClassOf rdf:resource="&SUMO;Building"/>
    <owl:disjointWith rdf:resource="#ParkingGarage"/>
  </owl:Class>

  <owl:Class rdf:about="&Mid-level-ontology;Trailer">
    <SUMO:disjoint rdf:resource="#SelfPoweredVehicle"/>
    <SUMO:disjoint rdf:resource="#UserPoweredVehicle"/>
    <rdf:type rdf:resource="&owl;Thing"/>
    <rdfs:comment>Trailer is the class of RoadVehicles that 

are designed for towing with another RoadVehicle.</rdfs:comment>
    <rdfs:subClassOf rdf:resource="&Mid-level-ontology;RoadVehicle"/>
  </owl:Class>

  <owl:Class rdf:about="&Mid-level-ontology;Train">
    <rdfs:comment>Train is the subclass of TransportationDevice 

whose instances are linked sequences of RollingStock whose motion is 

driven by one or more Locomotives or MotorizedRailwayCars.</rdfs:comment>
    <rdfs:subClassOf rdf:resource="#RailwayVehicle"/>
    <rdfs:subClassOf rdf:resource="#SelfPoweredVehicle"/>
    <rdfs:subClassOf rdf:resource="&SUMO;Collection"/>
    <owl:disjointWith rdf:resource="#ElectrifiedRailwayCar"/>
    <owl:disjointWith rdf:resource="#Locomotive"/>
    <owl:disjointWith rdf:resource="&Mid-level-ontology;Airplane"/>
  </owl:Class>

  <owl:Class rdf:about="&Mid-level-ontology;TransitTerminal">
    <rdfs:comment>A TransitTerminal is a place where 

travellers or transportation devices begin or end their journeys, or 

where passengers or goods may be transferred.  At a terminal, 

TransportationDevices may be received, assigned, sent out, or 

stored.  Major TransitTerminals have one or more TerminalBuildings.</rdfs:comment>
    <rdfs:subClassOf rdf:resource="&SUMO;Region"/>
    <rdfs:subClassOf rdf:resource="&SUMO;StationaryArtifact"/>
    <owl:disjointWith rdf:resource="#Bulkhead"/>
    <owl:disjointWith rdf:resource="#CanalLock"/>
    <owl:disjointWith rdf:resource="#CanalStructure"/>
    <owl:disjointWith rdf:resource="#Pier"/>
    <owl:disjointWith rdf:resource="&Mid-level-ontology;Bridge"/>
    <owl:disjointWith rdf:resource="&Mid-level-ontology;RailroadTrack"/>
    <owl:disjointWith rdf:resource="&Mid-level-ontology;Railway"/>
    <owl:disjointWith rdf:resource="&Mid-level-ontology;Tunnel"/>
  </owl:Class>

  <owl:Class rdf:about="&Mid-level-ontology;TransitwayJunction">
    <rdfs:comment>TransitwayJunction is the class of 

regions where two or more Transitways meet and traffic may transfer 

from one transitway to another.</rdfs:comment>
    <rdfs:label>intersection</rdfs:label>
    <rdfs:label>junction</rdfs:label>
    <rdfs:subClassOf rdf:resource="&SUMO;Transitway"/>
    <owl:disjointWith rdf:resource="#AirTransitway"/>
    <owl:disjointWith rdf:resource="#OneWayTransitway"/>
    <owl:disjointWith rdf:resource="#SingleTrafficLane"/>
    <owl:disjointWith rdf:resource="#TransitRoute"/>
    <owl:disjointWith rdf:resource="&Mid-level-ontology;Pipeline"/>
    <owl:disjointWith rdf:resource="&Mid-level-ontology;Tunnel"/>
    <owl:disjointWith rdf:resource="&Mid-level-ontology;Waterway"/>
    <owl:disjointWith rdf:resource="&SUMO;LandTransitway"/>
  </owl:Class>

  <owl:Class rdf:about="&Mid-level-ontology;TransportationCompany"/>
  <owl:Class rdf:about="&Mid-level-ontology;Truck">
    <rdfs:comment>Truck is the subclass of RoadVehicles that 

are designed primarily for transporting various kinds of non-passenger 

loads.  Truck is the class of single-bodied trucks or TruckTractors.  

Note: TractorTrailer combinations are a distinct class.</rdfs:comment>
    <rdfs:subClassOf rdf:resource="#SelfPoweredRoadVehicle"/>
    <owl:disjointWith rdf:resource="&Mid-level-ontology;Automobile"/>
  </owl:Class>

  <owl:Class rdf:about="&Mid-level-ontology;Tunnel">
    <rdfs:comment>Tunnel is a subclass of Transitways that 

consist of a lengthwise enclosed Hole that allows for transit 

through a solid body, as through a mountain, through the seabed below a 

body of water, or through a Building.</rdfs:comment>
    <rdfs:subClassOf rdf:resource="&SUMO;StationaryArtifact"/>
    <rdfs:subClassOf rdf:resource="&SUMO;Transitway"/>
    <owl:disjointWith rdf:resource="#AirTransitway"/>
    <owl:disjointWith rdf:resource="#Bulkhead"/>
    <owl:disjointWith rdf:resource="#CanalLock"/>
    <owl:disjointWith rdf:resource="#CanalStructure"/>
    <owl:disjointWith rdf:resource="#OneWayTransitway"/>
    <owl:disjointWith rdf:resource="#Pier"/>
    <owl:disjointWith rdf:resource="#SingleTrafficLane"/>
    <owl:disjointWith rdf:resource="#TransitRoute"/>
    <owl:disjointWith rdf:resource="&Mid-level-ontology;Bridge"/>
    <owl:disjointWith rdf:resource="&Mid-level-ontology;Pipeline"/>
    <owl:disjointWith rdf:resource="&Mid-level-ontology;RailroadTrack"/>
    <owl:disjointWith rdf:resource="&Mid-level-ontology;Railway"/>
    <owl:disjointWith rdf:resource="&Mid-level-ontology;TransitTerminal"/>
    <owl:disjointWith rdf:resource="&Mid-level-ontology;TransitwayJunction"/>
    <owl:disjointWith rdf:resource="&Mid-level-ontology;Waterway"/>
    <owl:disjointWith rdf:resource="&SUMO;LandTransitway"/>
  </owl:Class>

  <owl:Class rdf:about="&Mid-level-ontology;UnsurfacedRoadway">
    <rdf:type rdf:resource="&owl;Thing"/>
    <rdfs:comment>UnsurfacedRoadway is the subclass 

of Roadways that have natural surfaces of dirt or sand.</rdfs:comment>
    <rdfs:subClassOf rdf:resource="&SUMO;Roadway"/>
  </owl:Class>

  <owl:Class rdf:about="&Mid-level-ontology;Urea">
    <rdfs:comment>Urea is a dry, soluble, nitrogenous substance 

that is the major solid component of the urine of mammals, and which 

may be synthesized from ammonia and carbon dioxide; it is useful in the 

production of plastic and in Fertilizers.</rdfs:comment>
    <rdfs:subClassOf rdf:resource="&Mid-level-ontology;OrganicCompound"/>
  </owl:Class>

  <owl:Class rdf:about="&Mid-level-ontology;UserPoweredDevice">
    <rdfs:comment>UserPoweredDevice is a subclass of 

Device representing devices that perform work when a power input is 

supplied by the user.</rdfs:comment>
    <rdfs:subClassOf rdf:resource="&SUMO;Device"/>
    <owl:disjointWith rdf:resource="#Axle"/>
    <owl:disjointWith rdf:resource="#CanalLockGate"/>
    <owl:disjointWith rdf:resource="&Mid-level-ontology;AnimalPoweredDevice"/>
  </owl:Class>

  <owl:Class rdf:about="&Mid-level-ontology;Watercraft">
    <rdfs:comment>Watercraft is the class of all 

TransportationDevices used to travel on or in water.</rdfs:comment>
    <rdfs:subClassOf rdf:resource="&SUMO;TransportationDevice"/>
    <owl:disjointWith rdf:resource="#CargoContainer"/>
    <owl:disjointWith rdf:resource="&Mid-level-ontology;Aircraft"/>
    <owl:disjointWith rdf:resource="&Mid-level-ontology;Crane"/>
    <owl:disjointWith rdf:resource="&Mid-level-ontology;SelfPoweredDevice"/>
    <owl:disjointWith rdf:resource="&SUMO;Vehicle"/>
  </owl:Class>

  <Transportation:ModeOfTransit rdf:about="&Mid-level-ontology;Waterway">
    <rdf:type rdf:resource="&owl;Class"/>
    <rdfs:comment>Waterway is the class of navigable waters, 

including Oceans, SeaLanes, Rivers, Canals, Lakes, and inland 

bodies of water.</rdfs:comment>
    <rdfs:subClassOf rdf:resource="&SUMO;Transitway"/>
    <rdfs:subClassOf rdf:resource="&SUMO;WaterArea"/>
    <owl:disjointWith rdf:resource="#AirTransitway"/>
    <owl:disjointWith rdf:resource="#Anchorage"/>
    <owl:disjointWith rdf:resource="#DeepDraftWaterArea"/>
    <owl:disjointWith rdf:resource="#Harbor"/>
    <owl:disjointWith rdf:resource="#OneWayTransitway"/>
    <owl:disjointWith rdf:resource="#ShipBerth"/>
    <owl:disjointWith rdf:resource="#SingleTrafficLane"/>
    <owl:disjointWith rdf:resource="#TransitRoute"/>
    <owl:disjointWith rdf:resource="&Mid-level-ontology;Pipeline"/>
    <owl:disjointWith rdf:resource="&Mid-level-ontology;TransitwayJunction"/>
    <owl:disjointWith rdf:resource="&Mid-level-ontology;Tunnel"/>
    <owl:disjointWith rdf:resource="&SUMO;LandTransitway"/>
  </Transportation:ModeOfTransit>

  <owl:Class rdf:about="&Mid-level-ontology;Wheel"/>
  <owl:Class rdf:about="&Mid-level-ontology;Windmill">
    <rdfs:comment>Windmill is the subclass of Engines that 

produce mechanical power from Wind energy.</rdfs:comment>
    <rdfs:subClassOf rdf:resource="&Mid-level-ontology;Engine"/>
  </owl:Class>

  <owl:Class rdf:about="&SUMO;Agent"/>
  <owl:Class rdf:about="&SUMO;Artifact"/>
  <owl:Class rdf:about="&SUMO;AsymmetricRelation"/>
  <owl:Class rdf:about="&SUMO;Attaching"/>
  <owl:Class rdf:about="&SUMO;Attribute"/>
  <owl:Class rdf:about="&SUMO;BinaryPredicate"/>
  <owl:Class rdf:about="&SUMO;BodyMotion"/>
  <owl:Class rdf:about="&SUMO;Building"/>
  <owl:Class rdf:about="&SUMO;CaseRole"/>
  <owl:Class rdf:about="&SUMO;Certificate"/>
  <owl:Class rdf:about="&SUMO;City"/>
  <owl:Class rdf:about="&SUMO;CognitiveAgent"/>
  <owl:Class rdf:about="&SUMO;Collection"/>
  <owl:Class rdf:about="&SUMO;CommercialAgent"/>
  <owl:Class rdf:about="&SUMO;CommercialService"/>
  <owl:Class rdf:about="&SUMO;Communication"/>
  <owl:Class rdf:about="&SUMO;ContentBearingObject"/>
  <owl:Class rdf:about="&SUMO;DeonticAttribute"/>
  <owl:Class rdf:about="&SUMO;Device"/>
  <owl:Class rdf:about="&SUMO;GeographicArea"/>
  <owl:Class rdf:about="&SUMO;GeopoliticalArea"/>
  <owl:Class rdf:about="&SUMO;GovernmentOrganization"/>
  <owl:Class rdf:about="&SUMO;Guiding"/>
  <owl:Class rdf:about="&SUMO;Hole"/>
  <owl:Class rdf:about="&SUMO;IntentionalProcess"/>
  <owl:Class rdf:about="&SUMO;InternalAttribute"/>
  <owl:Class rdf:about="&SUMO;IrreflexiveRelation"/>
  <owl:Class rdf:about="&SUMO;Keeping"/>
  <owl:Class rdf:about="&SUMO;LandArea"/>
  <owl:Class rdf:about="&SUMO;LandTransitway">
    <rdfs:comment>LandTransitway is the subclass of 

Transitways that are paths for motion over the ground.</rdfs:comment>
    <rdfs:subClassOf rdf:resource="&SUMO;LandArea"/>
    <rdfs:subClassOf rdf:resource="&SUMO;Transitway"/>
    <owl:disjointWith rdf:resource="#AirTransitway"/>
    <owl:disjointWith rdf:resource="#OneWayTransitway"/>
    <owl:disjointWith rdf:resource="#SingleTrafficLane"/>
    <owl:disjointWith rdf:resource="#TransitRoute"/>
    <owl:disjointWith rdf:resource="&Mid-level-ontology;Pipeline"/>
    <owl:disjointWith rdf:resource="&Mid-level-ontology;TransitwayJunction"/>
    <owl:disjointWith rdf:resource="&Mid-level-ontology;Tunnel"/>
    <owl:disjointWith rdf:resource="&Mid-level-ontology;Waterway"/>
    <owl:disjointWith rdf:resource="&SUMO;Roadway"/>
  </owl:Class>

  <owl:Class rdf:about="&SUMO;LengthMeasure"/>
  <owl:Class rdf:about="&SUMO;Machine"/>
  <owl:Class rdf:about="&SUMO;Making"/>
  <owl:Class rdf:about="&SUMO;Managing"/>
  <owl:Class rdf:about="&SUMO;MassMeasure"/>
  <owl:Class rdf:about="&SUMO;Motion"/>
  <owl:Class rdf:about="&SUMO;Object"/>
  <owl:Class rdf:about="&SUMO;Obligation"/>
  <owl:Class rdf:about="&SUMO;OrganicObject"/>
  <owl:Class rdf:about="&SUMO;Organization"/>
  <owl:Class rdf:about="&SUMO;OrganizationalProcess"/>
  <owl:Class rdf:about="&SUMO;Physical"/>
  <owl:Class rdf:about="&SUMO;PhysicalQuantity">
    <rdf:type rdf:resource="&owl;Thing"/>
  </owl:Class>

  <owl:Class rdf:about="&SUMO;Position"/>
  <owl:Class rdf:about="&SUMO;PositionalAttribute"/>
  <owl:Class rdf:about="&SUMO;Region"/>
  <owl:Class rdf:about="&SUMO;RegulatoryProcess"/>
  <owl:Class rdf:about="&SUMO;RelationalAttribute"/>
  <Transportation:ModeOfTransit rdf:about="&SUMO;Roadway">
    <rdf:type rdf:resource="&owl;Class"/>
    <rdfs:comment>Roadway is the subclass of LandTransitways 

that are areas intended for surface travel by wheeled vehicles, typically 

powered vehicles. (Roadways are not designed for tracked vehicles; 

though transitable by them, the surfaces may be damaged by tracks.)  

Roadways are areas that have been at least minimally improved 

to enable the passage of wheeled vehicles.  Roadway includes dirt and 

gravelled roads, paved streets, and expressways.</rdfs:comment>
    <rdfs:subClassOf rdf:resource="&SUMO;LandArea"/>
    <rdfs:subClassOf rdf:resource="&SUMO;LandTransitway"/>
    <owl:disjointWith rdf:resource="&SUMO;LandTransitway"/>
  </Transportation:ModeOfTransit>

  <owl:Class rdf:about="&SUMO;SelfConnectedObject"/>
  <owl:Class rdf:about="&SUMO;SetOrClass"/>
  <owl:Class rdf:about="&SUMO;SingleValuedRelation"/>
  <owl:Class rdf:about="&SUMO;StationaryArtifact"/>
  <owl:Class rdf:about="&SUMO;Substance"/>
  <owl:Class rdf:about="&SUMO;SymbolicString"/>
  <owl:Class rdf:about="&SUMO;Text"/>
  <owl:Class rdf:about="&SUMO;TextureAttribute"/>
  <owl:Class rdf:about="&SUMO;TimeInterval"/>
  <owl:Class rdf:about="&SUMO;Transitway">
    <rdfs:comment>Transitway is the broadest class 

of Regions which may be passed through as a path in some kind of  

of Translocation.  Transitway includes land, air, and sea 

regions, and it includes both natural and artificial transitways.</rdfs:comment>
    <rdfs:subClassOf rdf:resource="&SUMO;Region"/>
    <rdfs:subClassOf rdf:resource="&SUMO;SelfConnectedObject"/>
  </owl:Class>

  <owl:Class rdf:about="&SUMO;Translocation">
    <rdfs:comment>Translocation is that class of Motions 

in which an object moves from one place to another.  In the case of round 

trips, the origin and destination are the same, but the intervening 

motion passes through some other locations.  Translocation represents 

linear motion, in contrast to rotation or other movement in place.  Unlike 

in Transportation, with translocation the use of a vehicle is optional; 

e.g., walking is a kind of Translocation.</rdfs:comment>
    <rdfs:subClassOf rdf:resource="&SUMO;Motion"/>
  </owl:Class>

  <owl:Class rdf:about="&SUMO;Transportation">
    <rdf:type rdf:resource="&owl;Thing"/>
    <rdfs:subClassOf rdf:resource="&SUMO;Translocation"/>
  </owl:Class>

  <owl:Class rdf:about="&SUMO;TransportationDevice"/>
  <owl:Class rdf:about="&SUMO;UnaryFunction"/>
  <owl:Class rdf:about="&SUMO;UnitOfMeasure"/>
  <owl:Class rdf:about="&SUMO;Vehicle">
    <rdfs:comment>Vehicle is the subclass of 

TransportationDevices that transport passengers or goods from one place 

to another by moving themselves from the origin to the destination while 

carrying the transportedItem, e.g., cars, trucks, ferries, and airplanes.  

Contrast Vehicles with devices such as Escalators, people movers 

(moving walkways), and supermarket checkout belts, which carry items from 

one place to another by means of moving parts, without the device itself 

removing from the origin to the destination.</rdfs:comment>
    <rdfs:subClassOf rdf:resource="&SUMO;TransportationDevice"/>
    <owl:disjointWith rdf:resource="#CargoContainer"/>
    <owl:disjointWith rdf:resource="&Mid-level-ontology;Aircraft"/>
    <owl:disjointWith rdf:resource="&Mid-level-ontology;Crane"/>
    <owl:disjointWith rdf:resource="&Mid-level-ontology;SelfPoweredDevice"/>
    <owl:disjointWith rdf:resource="&Mid-level-ontology;Watercraft"/>
  </owl:Class>

  <owl:Class rdf:about="&SUMO;VolumeMeasure"/>
  <owl:Class rdf:about="&SUMO;WaterArea"/>

<!-- Datatypes -->
  <rdfs:Datatype rdf:about="&SUMO;NonnegativeInteger"/>

<!-- Datatype Properties -->
  <SUMO:BinaryPredicate rdf:about="#crewSize">
    <rdf:type rdf:resource="&owl;DatatypeProperty"/>
    <rdfs:comment>(crewSize ?TRANSPORT ?COUNT) means that the 

TransportationDevice ?TRANSPORT has a specified crew size of ?COUNT.</rdfs:comment>
    <rdfs:domain rdf:resource="&SUMO;TransportationDevice"/>
    <rdfs:range rdf:resource="&SUMO;NonnegativeInteger"/>
  </SUMO:BinaryPredicate>

  <SUMO:BinaryPredicate rdf:about="#passengerCapacityMaxCount">
    <rdf:type rdf:resource="&SUMO;SingleValuedRelation"/>
    <rdf:type rdf:resource="&owl;DatatypeProperty"/>
    <rdfs:comment>(passengerCapacityMaxCount ?TRANSPORT ?NUMBER) means that the 

TransportationDevice ?TRANSPORT has a safe or legal carrying capacity 

for a total ?NUMBER of passengers (not including crew).  See also 

totalPersonCapacityCount.</rdfs:comment>
    <rdfs:domain rdf:resource="&SUMO;TransportationDevice"/>
    <rdfs:range rdf:resource="&SUMO;NonnegativeInteger"/>
  </SUMO:BinaryPredicate>

  <SUMO:BinaryPredicate rdf:about="#totalPersonCapacityCount">
    <rdf:type rdf:resource="&SUMO;SingleValuedRelation"/>
    <rdf:type rdf:resource="&owl;DatatypeProperty"/>
    <rdfs:comment>(totalPersonCapacityCount ?THING ?COUNT) means that the Object ?THING 

can legally or safely accommodate a maximum number of people ?COUNT.</rdfs:comment>
    <rdfs:domain rdf:resource="&SUMO;Object"/>
    <rdfs:range rdf:resource="&SUMO;NonnegativeInteger"/>
  </SUMO:BinaryPredicate>

  <SUMO:BinaryPredicate rdf:about="#totalPersonsAboard">
    <rdf:type rdf:resource="&SUMO;SingleValuedRelation"/>
    <rdf:type rdf:resource="&owl;DatatypeProperty"/>
    <rdfs:comment>(totalPersonsAboard ?TRANSPORT ?NUMBER) means that there is a total 

?NUMBER of people aboard the TransportationDevice ?TRANSPORT, including 

both crew and passengers.</rdfs:comment>
    <rdfs:domain rdf:resource="&SUMO;TransportationDevice"/>
    <rdfs:range rdf:resource="&SUMO;NonnegativeInteger"/>
  </SUMO:BinaryPredicate>

<!-- Object Properties -->
  <SUMO:UnaryFunction rdf:about="#MerchantMarineFn">
    <rdf:type rdf:resource="&owl;ObjectProperty"/>
    <rdfs:comment>(MerchantMarineFn ?AREA) denotes 

the Collection of all commercial ships registered in the 

ShipRegister of the GeopoliticalArea ?AREA.</rdfs:comment>
    <rdfs:domain rdf:resource="&SUMO;GeopoliticalArea"/>
    <rdfs:range rdf:resource="#MerchantMarine"/>
  </SUMO:UnaryFunction>

  <SUMO:UnaryFunction rdf:about="#PassportControlFn">
    <rdf:type rdf:resource="&owl;ObjectProperty"/>
    <rdfs:comment>(PassportControlFn ?PLACE) denotes the 

PassportControl organization located at the Object ?PLACE.</rdfs:comment>
    <rdfs:domain rdf:resource="&SUMO;Object"/>
    <rdfs:range rdf:resource="#PassportControl"/>
  </SUMO:UnaryFunction>

  <SUMO:UnaryFunction rdf:about="#PortFacilityFn">
    <rdf:type rdf:resource="&owl;ObjectProperty"/>
    <rdfs:comment>(PortFacilityFn ?CITY) denotes the 

PortFacility of the PortCity ?CITY, including mooring areas, docking 

space, cargo handling equipment, and on-land support facilities for 

marine traffic.</rdfs:comment>
    <rdfs:domain rdf:resource="#PortCity"/>
    <rdfs:range rdf:resource="&Mid-level-ontology;PortFacility"/>
  </SUMO:UnaryFunction>

  <SUMO:UnaryFunction rdf:about="#ShipRegisterFn">
    <rdf:type rdf:resource="&owl;ObjectProperty"/>
    <rdfs:comment>(ShipRegisterFn ?AREA) 

denotes the ShipRegister of the Ships that fly the flag of 

the GeopoliticalArea ?AREA.</rdfs:comment>
    <rdfs:domain rdf:resource="&SUMO;GeopoliticalArea"/>
    <rdfs:range rdf:resource="#ShipRegister"/>
  </SUMO:UnaryFunction>

  <SUMO:UnaryFunction rdf:about="#TransportationByFn">
    <SUMO:rangeSubclass rdf:resource="&SUMO;Transportation"/>
    <rdf:type rdf:resource="&owl;ObjectProperty"/>
    <rdfs:comment>(TransportationByFn ?TYPE) denotes the subclass of Transportation 

events in which a TransportationDevice of ?TYPE is the carrier.</rdfs:comment>
    <rdfs:domain rdf:resource="&SUMO;TransportationDevice"/>
  </SUMO:UnaryFunction>

  <SUMO:UnaryFunction rdf:about="#VehicleCrewFn">
    <rdf:type rdf:resource="&owl;ObjectProperty"/>
    <rdfs:comment>(VehicleCrewFn ?VEHICLE) denotes the 

Organization of people charged with operating the Vehicle ?VEHICLE.</rdfs:comment>
    <rdfs:domain rdf:resource="&SUMO;Vehicle"/>
  </SUMO:UnaryFunction>

  <SUMO:UnaryFunction rdf:about="#VehicleTripFn">
    <SUMO:rangeSubclass rdf:resource="&SUMO;Transportation"/>
    <rdf:type rdf:resource="&owl;ObjectProperty"/>
    <rdfs:comment>(VehicleTripFn ?DEVICE) denotes the subclass of Transportation 

events in which the carrier is the individual TransportationDevice 

?VEHICLE. Contrast this function with TransportationByFn, which is used 

to denote transportation by a specific kind of vehicle.  Example: 

(VehicleTripFn HMSQueenMary) vs. (TransportationByFn CruiseShip). 

Also note that the former is an instance of the latter.</rdfs:comment>
    <rdfs:domain rdf:resource="&SUMO;TransportationDevice"/>
  </SUMO:UnaryFunction>

  <SUMO:BinaryPredicate rdf:about="#addressOfHolder">
    <rdf:type rdf:resource="&owl;ObjectProperty"/>
    <rdfs:comment>(addressOfHolder ?DOC ?ADDRESS) means 

that the address of the holder of the Certificate ?DOC is given as 

the Address ?ADDRESS.</rdfs:comment>
    <rdfs:domain rdf:resource="&SUMO;Certificate"/>
    <rdfs:range rdf:resource="&Mid-level-ontology;Address"/>
  </SUMO:BinaryPredicate>

  <SUMO:BinaryPredicate rdf:about="#addressOfLocation">
    <rdf:type rdf:resource="&owl;ObjectProperty"/>
    <rdfs:comment>(addressOfLocation ?ADDRESS ?PLACE) means that the SymbolicString 

?ADDRESS is the address of the Object ?PLACE.</rdfs:comment>
    <rdfs:domain rdf:resource="&SUMO;SymbolicString"/>
    <rdfs:range rdf:resource="&SUMO;Object"/>
  </SUMO:BinaryPredicate>

  <SUMO:BinaryPredicate rdf:about="#cargoType">
    <rdf:type rdf:resource="&owl;ObjectProperty"/>
    <rdfs:comment>(cargoType ?DEVICE ?TYPE) means that the 

TransportationDevice ?DEVICE can, and typically does, carry cargo of 

the kind ?TYPE.</rdfs:comment>
    <rdfs:domain rdf:resource="&SUMO;TransportationDevice"/>
    <rdfs:range rdf:resource="&SUMO;Object"/>
  </SUMO:BinaryPredicate>

  <SUMO:BinaryPredicate rdf:about="#carrier">
    <rdf:type rdf:resource="&SUMO;CaseRole"/>
    <rdf:type rdf:resource="&owl;ObjectProperty"/>
    <rdfs:comment>(carrier ?EVENT ?OBJECT) means that in the 

Transportation process ?EVENT, the TransportationDevice ?OBJECT is 

used to carry something from the origin to the destination.  If the 

carrier is a Vehicle, then it moves along with whatever is carried.</rdfs:comment>
    <rdfs:domain rdf:resource="&SUMO;Transportation"/>
    <rdfs:range rdf:resource="&SUMO;TransportationDevice"/>
  </SUMO:BinaryPredicate>

  <SUMO:BinaryPredicate rdf:about="#clearanceHeight">
    <SUMO:domain rdf:resource="&SUMO;PhysicalQuantity"/>
    <rdf:type rdf:resource="&owl;ObjectProperty"/>
    <rdfs:comment>(clearanceHeight ?OBJECT ?HEIGHT) means 

that the height of the free space below an Object ?OBJECT (such as a 

Bridge, Tunnel ceiling, or Door lintel) is ?HEIGHT.</rdfs:comment>
    <rdfs:domain rdf:resource="&SUMO;Object"/>
  </SUMO:BinaryPredicate>

  <SUMO:BinaryPredicate rdf:about="#consignee">
    <rdf:type rdf:resource="&owl;ObjectProperty"/>
    <rdfs:comment>(consignee ?BOL ?AGENT) means that the 

BillOfLading ?BOL names the Agent ?AGENT as the consignee, i.e., 

the agent to whom the goods described in the bill of lading are to be 

delivered.</rdfs:comment>
  </SUMO:BinaryPredicate>

  <SUMO:BinaryPredicate rdf:about="#consignor">
    <rdf:type rdf:resource="&owl;ObjectProperty"/>
    <rdfs:comment>(consignor ?BOL ?AGENT) means that the 

BillOfLading ?BOL names the Agent ?AGENT as the consignor, i.e., 

the agent who committed the goods described in the bill of lading to 

the ShipMaster named in the bill of lading, for shipment to the 

consignee.</rdfs:comment>
  </SUMO:BinaryPredicate>

  <SUMO:BinaryPredicate rdf:about="#cruisingRange">
    <rdf:type rdf:resource="&owl;ObjectProperty"/>
    <rdfs:comment>(cruisingRange ?VEHICLE ?RANGE) means 

that the Vehicle ?VEHICLE has a cruising range of LengthMeasure 

?RANGE, when it is fully loaded with fuel.</rdfs:comment>
    <rdfs:domain rdf:resource="&SUMO;Vehicle"/>
    <rdfs:range rdf:resource="&SUMO;LengthMeasure"/>
  </SUMO:BinaryPredicate>

  <SUMO:BinaryPredicate rdf:about="#dateOfIssue">
    <rdf:type rdf:resource="&owl;ObjectProperty"/>
    <rdfs:comment>(dateOfIssue ?DOC ?TIME) means that the 

Certificate ?DOC was issued on the date ?TIME.</rdfs:comment>
    <rdfs:domain rdf:resource="&SUMO;Certificate"/>
    <rdfs:range rdf:resource="&SUMO;TimeInterval"/>
  </SUMO:BinaryPredicate>

  <SUMO:BinaryPredicate rdf:about="#destinationInSchedule">
    <rdf:type rdf:resource="&owl;ObjectProperty"/>
    <rdfs:comment>(destinationInSchedule ?SCHED ?PLACE) means that the 

TransportationSchedule ?SCHED contains information 

about Trips that arrive at the Object ?PLACE.</rdfs:comment>
    <rdfs:domain rdf:resource="#TransportationSchedule"/>
    <rdfs:range rdf:resource="&SUMO;Object"/>
  </SUMO:BinaryPredicate>

  <SUMO:BinaryPredicate rdf:about="#destinationInSystem">
    <rdf:type rdf:resource="&owl;ObjectProperty"/>
    <rdfs:comment>(destinationInSystem ?PLACE ?SYSTEM) means that ?PLACE is a 

destination along some route in the TransportationSystem ?SYSTEM.</rdfs:comment>
    <rdfs:domain rdf:resource="&SUMO;Object"/>
    <rdfs:range rdf:resource="#TransportationSystem"/>
  </SUMO:BinaryPredicate>

  <SUMO:BinaryPredicate rdf:about="#documentNumber">
    <rdf:type rdf:resource="&owl;ObjectProperty"/>
    <rdfs:comment>(documentNumber ?DOC ?STRING) means that 

the ContentBearingObject ?DOC has the uniqueIdentifier ?STRING.</rdfs:comment>
    <rdfs:domain rdf:resource="&SUMO;ContentBearingObject"/>
    <rdfs:range rdf:resource="&SUMO;SymbolicString"/>
  </SUMO:BinaryPredicate>

  <SUMO:BinaryPredicate rdf:about="#embargoedArea">
    <rdf:type rdf:resource="&owl;ObjectProperty"/>
    <rdfs:comment>(embargoedArea ?EMBARGO ?AREA) means that 

the TradeEmbargo ?EMBARGO forbids trade with the GeographicArea 

?AREA.</rdfs:comment>
    <rdfs:domain rdf:resource="#TradeEmbargo"/>
    <rdfs:range rdf:resource="&SUMO;GeographicArea"/>
  </SUMO:BinaryPredicate>

  <SUMO:BinaryPredicate rdf:about="#embargoedTradeType">
    <rdf:type rdf:resource="&owl;ObjectProperty"/>
    <rdfs:comment>(embargoedTradeType ?EMBARGO ?TYPE) 

means that the TradeEmbargo ?EMBARGO forbids trade in the kinds of 

Object ?TYPE.</rdfs:comment>
    <rdfs:domain rdf:resource="#TradeEmbargo"/>
    <rdfs:range rdf:resource="&SUMO;Object"/>
  </SUMO:BinaryPredicate>

  <SUMO:BinaryPredicate rdf:about="#equipmentType">
    <rdf:type rdf:resource="&owl;ObjectProperty"/>
    <rdfs:comment>(equipmentType ?THING ?TYPE) means that 

the Artifact ?THING has a component or attachment of Device ?TYPE. 

See also equipmentTypeCount.</rdfs:comment>
    <rdfs:domain rdf:resource="&SUMO;Artifact"/>
    <rdfs:range rdf:resource="&SUMO;Device"/>
  </SUMO:BinaryPredicate>

  <SUMO:BinaryPredicate rdf:about="#flagState">
    <rdf:type rdf:resource="&owl;ObjectProperty"/>
    <rdfs:comment>(flagState ?SHIP ?AREA) means that 

the Ship ?SHIP is enrolled in the ShipRegister of the 

GeopoliticalArea ?AREA and is subject to its maritime laws, 

regulations for operation of the ship, and rules of taxation.</rdfs:comment>
    <rdfs:domain rdf:resource="&Mid-level-ontology;Watercraft"/>
    <rdfs:label>flag of registry</rdfs:label>
    <rdfs:label>flag state</rdfs:label>
    <rdfs:range rdf:resource="&SUMO;GeopoliticalArea"/>
  </SUMO:BinaryPredicate>

  <SUMO:BinaryPredicate rdf:about="#fleetDeadWeightTonnage">
    <rdf:type rdf:resource="&owl;ObjectProperty"/>
    <rdfs:comment>(fleetDeadWeightTonnage ?FLEET ?AMOUNT) means that the Collection 

of Ships ?FLEET has a total carrying capacity of ?AMOUNT in LongTons.  

This is the aggregate vesselDeadWeightTonnage of all the fleet vessels.  

Dead Weight Tonnage, or DWT, is the weight of cargo plus stores that a  

vessel can carry when immersed to the proper load line.</rdfs:comment>
    <rdfs:domain rdf:resource="&SUMO;Collection"/>
    <rdfs:range rdf:resource="&SUMO;MassMeasure"/>
  </SUMO:BinaryPredicate>

  <SUMO:BinaryPredicate rdf:about="#fleetGrossRegisteredTonnage">
    <rdf:type rdf:resource="&owl;ObjectProperty"/>
    <rdfs:comment>(fleetGrossRegisteredTonnage ?FLEET ?AMOUNT) means that the 

Collection of Ships ?FLEET has a total carrying capacity of ?AMOUNT 

in RegistryTons.  This is the aggregate vesselGrossRegisteredTonnage 

of all the fleet vessels.  Gross Registered Tonnage, or GRT, is the 

capacity of a vessel calculated on an equivalence of 100 cubic feet of 

sheltered area per ton.</rdfs:comment>
    <rdfs:domain rdf:resource="&SUMO;Collection"/>
    <rdfs:range rdf:resource="&SUMO;PhysicalQuantity"/>
  </SUMO:BinaryPredicate>

  <SUMO:BinaryPredicate rdf:about="#fuelCapacity">
    <rdf:type rdf:resource="&owl;ObjectProperty"/>
    <rdfs:comment>(fuelCapacity ?DEVICE ?AMOUNT) means that 

the Device ?DEVICE has the fuelCapacity ?AMOUNT.</rdfs:comment>
    <rdfs:domain rdf:resource="&SUMO;Device"/>
    <rdfs:range rdf:resource="&SUMO;VolumeMeasure"/>
  </SUMO:BinaryPredicate>

  <SUMO:BinaryPredicate rdf:about="#issuedTo">
    <rdf:type rdf:resource="&owl;ObjectProperty"/>
    <rdfs:comment>(issuedTo ?DOC ?AGENT) means that the 

Certificate ?DOC was issued to the CognitiveAgent ?AGENT.</rdfs:comment>
    <rdfs:domain rdf:resource="&SUMO;Certificate"/>
    <rdfs:range rdf:resource="&SUMO;CognitiveAgent"/>
  </SUMO:BinaryPredicate>

  <SUMO:BinaryPredicate rdf:about="#ladenDraft">
    <rdf:type rdf:resource="&owl;ObjectProperty"/>
    <rdfs:comment>(ladenDraft ?SHIP ?AMOUNT) means that 

the Watercraft ?SHIP requires a waterDepth greater than ?AMOUNT 

to sail without running aground, when she is loaded at capacity.  

It also means that the vertical height between the lowest part of 

the keel of the loaded vessel and the waterline is ?AMOUNT.</rdfs:comment>
    <rdfs:domain rdf:resource="&Mid-level-ontology;Watercraft"/>
    <rdfs:range rdf:resource="&SUMO;LengthMeasure"/>
  </SUMO:BinaryPredicate>

  <SUMO:BinaryPredicate rdf:about="#lengthOfBroadGaugeRailway">
    <rdf:type rdf:resource="&owl;ObjectProperty"/>
    <rdfs:comment>(lengthOfBroadGaugeRailway ?AREA ?LENGTH) means that the sum length 

of broad gauge railway routes in the GeographicArea ?AREA is the 

LengthMeasure ?LENGTH.</rdfs:comment>
    <rdfs:domain rdf:resource="&SUMO;GeographicArea"/>
    <rdfs:range rdf:resource="&SUMO;LengthMeasure"/>
  </SUMO:BinaryPredicate>

  <SUMO:BinaryPredicate rdf:about="#lengthOfDualGaugeRailway">
    <rdf:type rdf:resource="&owl;ObjectProperty"/>
    <rdfs:comment>(lengthOfDualGaugeRailway ?AREA ?LENGTH) means that the sum length 

of dual gauge railway routes in the GeographicArea ?AREA is the 

LengthMeasure ?LENGTH.</rdfs:comment>
    <rdfs:domain rdf:resource="&SUMO;GeographicArea"/>
    <rdfs:range rdf:resource="&SUMO;LengthMeasure"/>
  </SUMO:BinaryPredicate>

  <SUMO:BinaryPredicate rdf:about="#lengthOfElectrifiedRailway">
    <rdf:type rdf:resource="&owl;ObjectProperty"/>
    <rdfs:comment>(lengthOfElectrifiedRailway ?AREA ?LENGTH) means that the sum  

length of all ElectrifiedRailway routes in the GeographicArea 

?AREA is the LengthMeasure ?LENGTH.</rdfs:comment>
    <rdfs:domain rdf:resource="&SUMO;GeographicArea"/>
    <rdfs:range rdf:resource="&SUMO;LengthMeasure"/>
  </SUMO:BinaryPredicate>

  <SUMO:BinaryPredicate rdf:about="#lengthOfExpresswaySystem">
    <rdf:type rdf:resource="&owl;ObjectProperty"/>
    <rdfs:comment>(lengthOfExpresswaySystem ?AREA ?LENGTH) means that the total length 

of Expressway in the GeographicArea ?AREA is ?LENGTH.</rdfs:comment>
    <rdfs:domain rdf:resource="&SUMO;GeographicArea"/>
    <rdfs:range rdf:resource="&SUMO;LengthMeasure"/>
  </SUMO:BinaryPredicate>

  <SUMO:BinaryPredicate rdf:about="#lengthOfMultipleTrackRailway">
    <rdf:type rdf:resource="&owl;ObjectProperty"/>
    <rdfs:comment>(lengthOfMultipleTrackRailway ?AREA ?LENGTH) means that the sum  

length of all MultipleTrackRailway routes in the GeographicArea 

?AREA is the LengthMeasure ?LENGTH.</rdfs:comment>
    <rdfs:domain rdf:resource="&SUMO;GeographicArea"/>
    <rdfs:range rdf:resource="&SUMO;LengthMeasure"/>
  </SUMO:BinaryPredicate>

  <SUMO:BinaryPredicate rdf:about="#lengthOfNarrowGaugeRailway">
    <rdf:type rdf:resource="&owl;ObjectProperty"/>
    <rdfs:comment>(lengthOfNarrowGaugeRailway ?AREA ?LENGTH) means that the sum length 

of narrow gauge railway routes in the GeographicArea ?AREA is the 

LengthMeasure ?LENGTH.</rdfs:comment>
    <rdfs:domain rdf:resource="&SUMO;GeographicArea"/>
    <rdfs:range rdf:resource="&SUMO;LengthMeasure"/>
  </SUMO:BinaryPredicate>

  <SUMO:BinaryPredicate rdf:about="#lengthOfNaturalGasPipeline">
    <rdf:type rdf:resource="&owl;ObjectProperty"/>
    <rdfs:comment>(lengthOfNaturalGasPipeline ?AREA ?AMOUNT) means that in the 

GeograpicArea ?AREA there is the LengthMeasure ?AMOUNT of 

NaturalGasPipeline.</rdfs:comment>
    <rdfs:domain rdf:resource="&SUMO;GeographicArea"/>
    <rdfs:range rdf:resource="&SUMO;LengthMeasure"/>
  </SUMO:BinaryPredicate>

  <SUMO:BinaryPredicate rdf:about="#lengthOfPavedHighway">
    <rdf:type rdf:resource="&owl;ObjectProperty"/>
    <rdfs:comment>(lengthOfPavedHighway ?AREA ?LENGTH) means that the total length 

of SurfacedRoadway in the GeographicArea ?AREA is ?LENGTH.</rdfs:comment>
    <rdfs:domain rdf:resource="&SUMO;GeographicArea"/>
    <rdfs:range rdf:resource="&SUMO;LengthMeasure"/>
  </SUMO:BinaryPredicate>

  <SUMO:BinaryPredicate rdf:about="#lengthOfPetroleumPipeline">
    <rdf:type rdf:resource="&owl;ObjectProperty"/>
    <rdfs:comment>(lengthOfPetroleumPipeline ?AREA ?AMOUNT) means that in the 

GeograpicArea ?AREA there is the LengthMeasure ?AMOUNT of 

PetroleumPipeline.</rdfs:comment>
    <rdfs:domain rdf:resource="&SUMO;GeographicArea"/>
    <rdfs:range rdf:resource="&SUMO;LengthMeasure"/>
  </SUMO:BinaryPredicate>

  <SUMO:BinaryPredicate rdf:about="#lengthOfPetroleumProductPipeline">
    <rdf:type rdf:resource="&owl;ObjectProperty"/>
    <rdfs:comment>(lengthOfPetroleumProductPipeline ?AREA ?AMOUNT) means that in the 

GeograpicArea ?AREA there is the LengthMeasure ?AMOUNT of 

PetroleumProductPipeline.</rdfs:comment>
    <rdfs:domain rdf:resource="&SUMO;GeographicArea"/>
    <rdfs:range rdf:resource="&SUMO;LengthMeasure"/>
  </SUMO:BinaryPredicate>

  <SUMO:BinaryPredicate rdf:about="#lengthOfStandardGaugeRailway">
    <rdf:type rdf:resource="&owl;ObjectProperty"/>
    <rdfs:comment>(lengthOfStandardGaugeRailway ?AREA ?LENGTH) means that the sum length 

of standard gauge railway routes in the GeographicArea ?AREA is the 

LengthMeasure ?LENGTH.</rdfs:comment>
    <rdfs:domain rdf:resource="&SUMO;GeographicArea"/>
    <rdfs:range rdf:resource="&SUMO;LengthMeasure"/>
  </SUMO:BinaryPredicate>

  <SUMO:BinaryPredicate rdf:about="#lengthOfUnclassifiedGaugeRailway">
    <rdf:type rdf:resource="&owl;ObjectProperty"/>
    <rdfs:comment>(lengthOfUnclassifiedGaugeRailway ?AREA ?LENGTH) means that the sum length 

of railway routes in the GeographicArea ?AREA classified as something 

other than broad, dual, narrow, or standard gauge is the LengthMeasure 

?LENGTH.</rdfs:comment>
    <rdfs:domain rdf:resource="&SUMO;GeographicArea"/>
    <rdfs:range rdf:resource="&SUMO;LengthMeasure"/>
  </SUMO:BinaryPredicate>

  <SUMO:BinaryPredicate rdf:about="#lengthOfUnpavedHighway">
    <rdf:type rdf:resource="&owl;ObjectProperty"/>
    <rdfs:comment>(lengthOfUnpavedHighway ?AREA ?LENGTH) means that the total length 

of UnsurfacedRoadway in the GeographicArea ?AREA is ?LENGTH.</rdfs:comment>
    <rdfs:domain rdf:resource="&SUMO;GeographicArea"/>
    <rdfs:range rdf:resource="&SUMO;LengthMeasure"/>
  </SUMO:BinaryPredicate>

  <SUMO:BinaryPredicate rdf:about="#licenseNumber">
    <rdf:type rdf:resource="&owl;ObjectProperty"/>
    <rdfs:comment>(licenseNumber ?LIC ?STRING) means that 

the License ?LIC has the uniqueIdentifier ?STRING.</rdfs:comment>
    <rdfs:domain rdf:resource="&Mid-level-ontology;License"/>
    <rdfs:range rdf:resource="&SUMO;SymbolicString"/>
    <rdfs:subPropertyOf rdf:resource="#documentNumber"/>
  </SUMO:BinaryPredicate>

  <SUMO:BinaryPredicate rdf:about="#navigableForDraft">
    <rdf:type rdf:resource="&owl;ObjectProperty"/>
    <rdfs:comment>(navigableForDraft ?WATERWAY ?DRAFT) means that the Waterway 

?WATERWAY can be transited by vessels having a draft of ?DRAFT or 

less.  navigableForDraft does not indicate a positive limit.  To 

indicate a limit, state '(not (navigableForDraft ?WW ?MAX))', 

which implies no navigability for vessels of deeper draft than ?MAX.</rdfs:comment>
    <rdfs:domain rdf:resource="&SUMO;WaterArea"/>
    <rdfs:range rdf:resource="&SUMO;LengthMeasure"/>
  </SUMO:BinaryPredicate>

  <SUMO:BinaryPredicate rdf:about="#navigableForShippingTonnage">
    <rdf:type rdf:resource="&owl;ObjectProperty"/>
    <rdfs:comment>(navigableForShippingTonnage ?WATERWAY ?TONNAGE) means that the 

Waterway ?WATERWAY can accommodate vessels of the 

vesselDeadWeightTonnage ?TONNAGE.</rdfs:comment>
    <rdfs:domain rdf:resource="&SUMO;WaterArea"/>
    <rdfs:range rdf:resource="&SUMO;PhysicalQuantity"/>
  </SUMO:BinaryPredicate>

  <SUMO:BinaryPredicate rdf:about="#obstacleForMotionType">
    <rdf:type rdf:resource="&owl;ObjectProperty"/>
    <rdfs:comment>(obstacleForMotionType ?BLOCK ?TYPE) means that the Object ?BLOCK is 

an obstacle to the type of Motion ?TYPE.</rdfs:comment>
    <rdfs:domain rdf:resource="&SUMO;Object"/>
    <rdfs:range rdf:resource="&SUMO;Motion"/>
  </SUMO:BinaryPredicate>

  <SUMO:BinaryPredicate rdf:about="#obstacleForTransitway">
    <rdf:type rdf:resource="&owl;ObjectProperty"/>
    <rdfs:comment>(obstacleForTransitway ?BLOCK ?WAY) means that the Object ?BLOCK 

presents an obstacle to the Transitway ?WAY.</rdfs:comment>
    <rdfs:domain rdf:resource="&SUMO;Object"/>
    <rdfs:range rdf:resource="&SUMO;Transitway"/>
  </SUMO:BinaryPredicate>

  <SUMO:BinaryPredicate rdf:about="#obstacleForTransitwayType">
    <rdf:type rdf:resource="&owl;ObjectProperty"/>
    <rdfs:comment>(obstacleForTransitwayType ?BLOCK ?TYPE) means that the Object ?BLOCK 

presents an obstacle to Transitways of ?TYPE.</rdfs:comment>
    <rdfs:domain rdf:resource="&SUMO;Object"/>
    <rdfs:range rdf:resource="&SUMO;Transitway"/>
  </SUMO:BinaryPredicate>

  <SUMO:BinaryPredicate rdf:about="#originInSchedule">
    <rdf:type rdf:resource="&owl;ObjectProperty"/>
    <rdfs:comment>(originInSchedule ?SCHED ?PLACE) 

means that the TransportationSchedule ?SCHED contains information 

about Trips that originate from the Object ?PLACE.</rdfs:comment>
    <rdfs:domain rdf:resource="#TransportationSchedule"/>
    <rdfs:range rdf:resource="&SUMO;Object"/>
  </SUMO:BinaryPredicate>

  <SUMO:BinaryPredicate rdf:about="#passportNumber">
    <rdf:type rdf:resource="&owl;ObjectProperty"/>
    <rdfs:comment>(passportNumber ?DOC ?STRING) means that 

the Passport ?DOC has the uniqueIdentifier ?STRING.</rdfs:comment>
    <rdfs:domain rdf:resource="#Passport"/>
    <rdfs:range rdf:resource="&SUMO;SymbolicString"/>
    <rdfs:subPropertyOf rdf:resource="#documentNumber"/>
  </SUMO:BinaryPredicate>

  <SUMO:BinaryPredicate rdf:about="#pathInSystem">
    <rdf:type rdf:resource="&owl;ObjectProperty"/>
    <rdfs:comment>(pathInSystem ?PATH ?SYSTEM) means that 

the Physical thing ?PATH consists of one or more connected routes in 

the PhysicalSystem ?SYSTEM.</rdfs:comment>
    <rdfs:domain rdf:resource="&SUMO;Transitway"/>
    <rdfs:range rdf:resource="#TransportationSystem"/>
  </SUMO:BinaryPredicate>

  <SUMO:BinaryPredicate rdf:about="#personCapacityMaxWeight">
    <rdf:type rdf:resource="&owl;ObjectProperty"/>
    <rdfs:comment>(personCapacityMaxWeight ?THING ?WEIGHT) means that the Object ?THING 

has a safe carrying capacity for a total ?WEIGHT of persons, as occupants, 

crew, or passengers, combined.</rdfs:comment>
    <rdfs:domain rdf:resource="&SUMO;Object"/>
    <rdfs:range rdf:resource="&SUMO;MassMeasure"/>
  </SUMO:BinaryPredicate>

  <SUMO:BinaryPredicate rdf:about="#routeInSystem">
    <rdf:type rdf:resource="&owl;ObjectProperty"/>
    <rdfs:comment>(routeInSystem ?PART ?SYSTEM) means that 

the Transitway ?PART is an established route of the 

TransportationSystem ?SYSTEM.</rdfs:comment>
    <rdfs:domain rdf:resource="&SUMO;Transitway"/>
    <rdfs:range rdf:resource="#TransportationSystem"/>
    <rdfs:subPropertyOf rdf:resource="#pathInSystem"/>
  </SUMO:BinaryPredicate>

  <SUMO:BinaryPredicate rdf:about="#speed">
    <rdf:type rdf:resource="&owl;ObjectProperty"/>
    <rdfs:comment>(speed ?OBJECT ?SPEED) means that the 

instantaneous speed of ?OBJECT is the PhysicalQuantity ?SPEED.  

Speed may be given in KnotUnitOfSpeed or in other units with SpeedFn.  

Assertions with speed should be temporally qualified.</rdfs:comment>
    <rdfs:domain rdf:resource="&SUMO;Object"/>
    <rdfs:range rdf:resource="&SUMO;PhysicalQuantity"/>
  </SUMO:BinaryPredicate>

  <SUMO:BinaryPredicate rdf:about="#subSystem">
    <rdf:type rdf:resource="&owl;ObjectProperty"/>
    <rdfs:comment>(subSystem ?SUB ?SYSTEM) means that the TransportationSystem ?SUB 

is a part of the TransportationSystem ?SYSTEM.</rdfs:comment>
    <rdfs:domain rdf:resource="#TransportationSystem"/>
    <rdfs:range rdf:resource="#TransportationSystem"/>
  </SUMO:BinaryPredicate>

  <SUMO:BinaryPredicate rdf:about="#telephoneNumberAtLocation">
    <rdf:type rdf:resource="&owl;ObjectProperty"/>
    <rdfs:comment>(telephoneNumberAtLocation ?NUMBER ?PLACE) means that the 

SymbolicString ?NUMBER is a telephone number at the Object ?PLACE.</rdfs:comment>
    <rdfs:domain rdf:resource="&SUMO;SymbolicString"/>
    <rdfs:range rdf:resource="&SUMO;Object"/>
  </SUMO:BinaryPredicate>

  <SUMO:BinaryPredicate rdf:about="#telephoneNumberOfHolder">
    <rdf:type rdf:resource="&owl;ObjectProperty"/>
    <rdfs:comment>(telephoneNumberOfHolder ?DOC ?NUMBER) means that the telephone number 

of the holder of the Certificate ?DOC is given as the SymbolicString 

?NUMBER.</rdfs:comment>
    <rdfs:domain rdf:resource="&SUMO;Certificate"/>
    <rdfs:range rdf:resource="&SUMO;SymbolicString"/>
  </SUMO:BinaryPredicate>

  <SUMO:BinaryPredicate rdf:about="#totalLengthOfHighwaySystem">
    <rdf:type rdf:resource="&owl;ObjectProperty"/>
    <rdfs:comment>(totalLengthOfHighwaySystem ?AREA ?LENGTH) means that the total 

length of the highway system in the GeographicArea ?AREA is ?LENGTH.  

The figure includes both paved and unpaved roads.</rdfs:comment>
    <rdfs:domain rdf:resource="&SUMO;GeographicArea"/>
    <rdfs:range rdf:resource="&SUMO;LengthMeasure"/>
  </SUMO:BinaryPredicate>

  <SUMO:BinaryPredicate rdf:about="#totalLengthOfRailwaySystem">
    <rdf:type rdf:resource="&owl;ObjectProperty"/>
    <rdfs:comment>(totalLengthOfRailwaySystem ?AREA ?LENGTH) means that the sum  

length of all railway routes in the GeographicArea ?AREA 

is the LengthMeasure ?LENGTH.</rdfs:comment>
    <rdfs:domain rdf:resource="&SUMO;GeographicArea"/>
    <rdfs:range rdf:resource="&SUMO;LengthMeasure"/>
  </SUMO:BinaryPredicate>

  <SUMO:BinaryPredicate rdf:about="#totalLengthOfWaterways">
    <rdf:type rdf:resource="&owl;ObjectProperty"/>
    <rdfs:comment>(totalLengthOfWaterways ?AREA ?LENGTH) means that the 

total length of navigable Waterways in the GeographicArea ?AREA 

is the LengthMeasure ?LENGTH.</rdfs:comment>
    <rdfs:domain rdf:resource="&SUMO;GeographicArea"/>
    <rdfs:range rdf:resource="&SUMO;LengthMeasure"/>
  </SUMO:BinaryPredicate>

  <SUMO:BinaryPredicate rdf:about="#totalPipelineInArea">
    <rdf:type rdf:resource="&owl;ObjectProperty"/>
    <rdfs:comment>(totalPipelineInArea ?AREA ?LENGTH) means that the GeopoliticalArea 

?AREA has the quantity ?LENGTH of Pipelines.</rdfs:comment>
    <rdfs:domain rdf:resource="&SUMO;GeographicArea"/>
    <rdfs:range rdf:resource="&SUMO;LengthMeasure"/>
  </SUMO:BinaryPredicate>

  <SUMO:BinaryPredicate rdf:about="#trafficableForTrafficType">
    <rdf:type rdf:resource="&owl;ObjectProperty"/>
    <rdfs:comment>(trafficableForTrafficType ?WAY ?TYPE) means that Objects of ?TYPE 

can move on or in the Transitway ?WAY.</rdfs:comment>
    <rdfs:domain rdf:resource="&SUMO;Object"/>
    <rdfs:range rdf:resource="&SUMO;SelfConnectedObject"/>
  </SUMO:BinaryPredicate>

  <SUMO:BinaryPredicate rdf:about="#transitwayMaximumSpeed">
    <rdf:type rdf:resource="&owl;ObjectProperty"/>
    <rdfs:comment>(transitwayMaximumSpeed ?WAY ?SPEED) means that the Transitway 

?WAY has a maximum allowed speed of ?SPEED, set and enforced by some 

authority.</rdfs:comment>
    <rdfs:domain rdf:resource="&SUMO;Transitway"/>
    <rdfs:range rdf:resource="&SUMO;PhysicalQuantity"/>
  </SUMO:BinaryPredicate>

  <SUMO:BinaryPredicate rdf:about="#transitwayMaximumWeight">
    <rdf:type rdf:resource="&owl;ObjectProperty"/>
    <rdfs:comment>(transitwayMaximumWeight ?WAY ?WEIGHT) means that the Transitway 

?WAY has a maximum safe or allowed weight of ?WEIGHT, e.g., the 

maximum weight that a Bridge can support.</rdfs:comment>
    <rdfs:domain rdf:resource="&SUMO;Transitway"/>
    <rdfs:range rdf:resource="&SUMO;PhysicalQuantity"/>
  </SUMO:BinaryPredicate>

  <SUMO:BinaryPredicate rdf:about="#transitwayMinimumSpeed">
    <rdf:type rdf:resource="&owl;ObjectProperty"/>
    <rdfs:comment>(transitwayMinimumSpeed ?WAY ?SPEED) means that the Transitway 

?WAY has a minimum allowed speed of ?SPEED, set and enforced by some 

authority.</rdfs:comment>
    <rdfs:domain rdf:resource="&SUMO;Transitway"/>
    <rdfs:range rdf:resource="&SUMO;PhysicalQuantity"/>
  </SUMO:BinaryPredicate>

  <SUMO:BinaryPredicate rdf:about="#transportedItem">
    <rdf:type rdf:resource="&SUMO;CaseRole"/>
    <rdf:type rdf:resource="&owl;ObjectProperty"/>
    <rdfs:comment>(transportedItem ?MOVEMENT ?ITEM) means 

that in the Transportation ?MOVEMENT, the Object ?ITEM is 

moved from one place to another using a TransportationDevice.</rdfs:comment>
    <rdfs:domain rdf:resource="&SUMO;Transportation"/>
    <rdfs:range rdf:resource="&SUMO;Object"/>
  </SUMO:BinaryPredicate>

  <SUMO:BinaryPredicate rdf:about="#vehicleCapacityMaxWeight">
    <rdf:type rdf:resource="&owl;ObjectProperty"/>
    <rdfs:comment>(vehicleCapacityMaxWeight ?TRANSPORT ?WEIGHT) means that the 

TransportationDevice ?TRANSPORT has a safe carrying capacity for 

a total MassMeasure of ?WEIGHT.</rdfs:comment>
    <rdfs:domain rdf:resource="&SUMO;TransportationDevice"/>
    <rdfs:range rdf:resource="&SUMO;MassMeasure"/>
  </SUMO:BinaryPredicate>

  <SUMO:BinaryPredicate rdf:about="#vehicleCruisingSpeed">
    <rdf:type rdf:resource="&owl;ObjectProperty"/>
    <rdfs:comment>(vehicleCruisingSpeed ?TRANSPORT ?SPEED) means that the typical cruising 

speed of the Vehicle ?TRANSPORT is the PhysicalQuantity ?SPEED.  This 

predicate need not be used with a temporal constraint.  For actual vehicle 

speed at a given time, use speed or measure with SpeedFn and an 

appropriate temporal qualification.</rdfs:comment>
    <rdfs:domain rdf:resource="&SUMO;Vehicle"/>
    <rdfs:range rdf:resource="&SUMO;PhysicalQuantity"/>
  </SUMO:BinaryPredicate>

  <SUMO:BinaryPredicate rdf:about="#vehicleMaximumSpeed">
    <rdf:type rdf:resource="&owl;ObjectProperty"/>
    <rdfs:comment>(vehicleMaximumSpeed ?TRANSPORT ?SPEED) 

means that the maximum speed of which the Vehicle ?TRANSPORT is capable is 

the PhysicalQuantity ?SPEED.  This is independent of legally allowed 

maximum speeds.</rdfs:comment>
    <rdfs:domain rdf:resource="&SUMO;Vehicle"/>
    <rdfs:range rdf:resource="&SUMO;PhysicalQuantity"/>
  </SUMO:BinaryPredicate>

  <SUMO:AsymmetricRelation rdf:about="#vehicleOperator">
    <rdf:type rdf:resource="&SUMO;BinaryPredicate"/>
    <rdf:type rdf:resource="&SUMO;IrreflexiveRelation"/>
    <rdf:type rdf:resource="&owl;ObjectProperty"/>
    <rdfs:comment>(vehicleOperator ?AGENT ?OBJECT) means 

that the CommericalAgent ?AGENT is the commercial operator of the 

Vehicle ?OBJECT, that is, the agent that owns or leases the vehicle and 

supplies the crew which physically runs it.</rdfs:comment>
    <rdfs:domain rdf:resource="&SUMO;CommercialAgent"/>
    <rdfs:range rdf:resource="&SUMO;Object"/>
  </SUMO:AsymmetricRelation>

  <SUMO:BinaryPredicate rdf:about="#vesselDeadWeightTonnage">
    <rdf:type rdf:resource="&owl;ObjectProperty"/>
    <rdfs:comment>(vesselDeadWeightTonnage ?VESSEL ?AMOUNT) means that the 

Watercraft ?VESSEL has a carrying capacity when fully loaded of 

?AMOUNT in LongTons.  This is the Dead Weight Tonnage, or DWT, 

of the vessel, which is the total weight of cargo plus stores 

that the vessel can carry when immersed to the proper load line.</rdfs:comment>
    <rdfs:domain rdf:resource="&Mid-level-ontology;Watercraft"/>
    <rdfs:range rdf:resource="&SUMO;MassMeasure"/>
    <rdfs:subPropertyOf rdf:resource="#vesselDisplacement"/>
  </SUMO:BinaryPredicate>

  <SUMO:BinaryPredicate rdf:about="#vesselDisplacement">
    <rdf:type rdf:resource="&owl;ObjectProperty"/>
    <rdfs:comment>(vesselDisplacement ?VESSEL ?AMOUNT) means that the displacement 

of Watercraft ?VESSEL is the PhysicalQuantity ?AMOUNT.  The 

displacement of a vessel may be measured in LongTons (Dead Weight 

Tonnage, or DWT) or by volume (Gross Registered Tonnage, or GRT).</rdfs:comment>
    <rdfs:domain rdf:resource="&Mid-level-ontology;Watercraft"/>
    <rdfs:range rdf:resource="&SUMO;PhysicalQuantity"/>
  </SUMO:BinaryPredicate>

  <SUMO:BinaryPredicate rdf:about="#vesselGrossRegisteredTonnage">
    <rdf:type rdf:resource="&owl;ObjectProperty"/>
    <rdfs:comment>(vesselGrossRegisteredTonnage ?VESSEL ?AMOUNT) means that the 

Watercraft ?VESSEL has a carrying capacity when fully loaded of 

?AMOUNT, where ?AMOUNT is the Gross Registered Tonnage (GRT) of the 

vessel, which is based on the total sheltered volume of the vessel 

measured in hundreds of cubic feet, and converted to gross tons 

at an equivalence of 100 cubic feet per ton.</rdfs:comment>
    <rdfs:domain rdf:resource="&Mid-level-ontology;Watercraft"/>
    <rdfs:range rdf:resource="&SUMO;PhysicalQuantity"/>
    <rdfs:subPropertyOf rdf:resource="#vesselDisplacement"/>
  </SUMO:BinaryPredicate>

  <SUMO:UnaryFunction rdf:about="&Mid-level-ontology;OperatingFn">
    <SUMO:rangeSubclass rdf:resource="&SUMO;Process"/>
    <rdf:type rdf:resource="&owl;ObjectProperty"/>
    <rdfs:comment>(OperatingFn ?TYPE) denotes the class 

of events in which a Device of ?TYPE is being operated.</rdfs:comment>
    <rdfs:domain rdf:resource="&SUMO;Device"/>
  </SUMO:UnaryFunction>

  <SUMO:BinaryPredicate rdf:about="&Mid-level-ontology;detainee">
    <rdf:type rdf:resource="&SUMO;CaseRole"/>
    <rdf:type rdf:resource="&owl;ObjectProperty"/>
    <rdfs:comment>(detainee ?EVENT ?OBJECT) means that in the 

Keeping ?EVENT, the Object ?OBJECT is restrained by force, threat, or 

other form of intimidation.</rdfs:comment>
    <rdfs:domain rdf:resource="&SUMO;Keeping"/>
    <rdfs:range rdf:resource="&SUMO;Object"/>
  </SUMO:BinaryPredicate>

  <SUMO:BinaryPredicate rdf:about="&Mid-level-ontology;deviceState">
    <rdf:type rdf:resource="&owl;ObjectProperty"/>
    <rdfs:comment>(deviceState ?DEVICE ?STATE) means that 

the Object ?DEVICE is in the DeviceStateAttribute ?STATE.</rdfs:comment>
    <rdfs:domain rdf:resource="&SUMO;Object"/>
    <rdfs:range rdf:resource="&Mid-level-ontology;DeviceStateAttribute"/>
  </SUMO:BinaryPredicate>

  <SUMO:BinaryPredicate rdf:about="&Mid-level-ontology;inventory">
    <rdf:type rdf:resource="&owl;ObjectProperty"/>
    <rdfs:comment>(inventory ?CBO ?COLLECTION) means that 

the ContentBearingObject ?CBO contains a list or enumeration of the 

members of the Collection ?COLLECTION.</rdfs:comment>
    <rdfs:domain rdf:resource="&SUMO;ContentBearingObject"/>
    <rdfs:range rdf:resource="&SUMO;Collection"/>
  </SUMO:BinaryPredicate>

  <SUMO:BinaryPredicate rdf:about="&Mid-level-ontology;memberType">
    <rdf:type rdf:resource="&owl;ObjectProperty"/>
    <rdfs:comment>(memberType ?GROUP ?TYPE) means that all 

the members of the Collection ?GROUP belong to the SetOrClass 

?TYPE.</rdfs:comment>
    <rdfs:domain rdf:resource="&SUMO;Collection"/>
    <rdfs:range rdf:resource="&SUMO;SetOrClass"/>
  </SUMO:BinaryPredicate>

  <SUMO:AsymmetricRelation rdf:about="&Mid-level-ontology;powerPlant">
    <rdf:type rdf:resource="&SUMO;BinaryPredicate"/>
    <rdf:type rdf:resource="&SUMO;IrreflexiveRelation"/>
    <rdf:type rdf:resource="&owl;ObjectProperty"/>
    <rdfs:comment>(powerPlant ?GENERATOR ?THING) means that 

the Device ?GENERATOR is the power-producing component of the Artifact 

?THING which provides the energy for its operation.</rdfs:comment>
    <rdfs:domain rdf:resource="&SUMO;Device"/>
    <rdfs:range rdf:resource="&SUMO;Artifact"/>
  </SUMO:AsymmetricRelation>

  <SUMO:BinaryPredicate rdf:about="&Mid-level-ontology;registeredItem">
    <rdf:type rdf:resource="&owl;ObjectProperty"/>
    <rdfs:comment>(registeredItem ?DOCUMENT ?ITEM) means 

that the Text ?DOCUMENT contains an official record of the Physical 

thing ?ITEM.  The registered item could be an object or an event, e.g., 

an automobile, a ship, a marriage, an adoption.</rdfs:comment>
    <rdfs:domain rdf:resource="&SUMO;Text"/>
    <rdfs:range rdf:resource="&SUMO;Physical"/>
  </SUMO:BinaryPredicate>

  <owl:ObjectProperty rdf:about="&SUMO;contraryAttribute"/>
  <owl:ObjectProperty rdf:about="&SUMO;disjoint"/>
  <owl:ObjectProperty rdf:about="&SUMO;domain"/>
  <owl:ObjectProperty rdf:about="&SUMO;geographicSubregion"/>
  <owl:ObjectProperty rdf:about="&SUMO;located"/>
  <owl:ObjectProperty rdf:about="&SUMO;path"/>
  <owl:ObjectProperty rdf:about="&SUMO;rangeSubclass"/>
  <owl:ObjectProperty rdf:about="&SUMO;relatedInternalConcept"/>
  <owl:ObjectProperty rdf:about="&SUMO;subAttribute"/>
  <owl:ObjectProperty rdf:about="&SUMO;subOrganization"/>

<!-- Instances -->
  <Mid-level-ontology:Profession rdf:about="#AirTrafficController">
    <rdfs:comment>AirTrafficController is the 

attribute that describes someone who is an Air Traffic Controller (ATC).</rdfs:comment>
  </Mid-level-ontology:Profession>

  <SUMO:Position rdf:about="#AircraftNavigator">
    <rdfs:comment>AircraftNavigator is the Position 

of the person who determines the course and position of an individual 

Aircraft, usually while on board, in order to guide its movements, the 

execution of which may be carried out by the AircraftPilot or copilot.</rdfs:comment>
  </SUMO:Position>

  <SUMO:Position rdf:about="#AircraftPilot">
    <rdfs:comment>AircraftPilot is the Position attribute 

of an individual who is authorized to fly aircraft of some kind.</rdfs:comment>
  </SUMO:Position>

  <Transportation:AirportByRunwaySurface rdf:about="#AirportWithPavedRunway">
    <rdfs:comment>AirportWithPavedRunway is an 

AirportClassification attribute used to describe an airport whose 

longest runway is a PavedRunway.</rdfs:comment>
  </Transportation:AirportByRunwaySurface>

  <Transportation:AirportByRunwaySurface rdf:about="#AirportWithUnpavedRunway">
    <rdfs:comment>AirportWithUnpavedRunway is 

an AirportClassification attribute used to describe an airport whose 

longest runway is an UnpavedRunway.</rdfs:comment>
  </Transportation:AirportByRunwaySurface>

  <Transportation:TrackGauge rdf:about="#BroadGauge">
    <rdfs:comment>BroadGauge is the attribute of 

any Railway that has a TrackGauge wider than StandardGauge 

(i.e., wider than 1.44 Meters).</rdfs:comment>
  </Transportation:TrackGauge>

  <SUMO:Position rdf:about="#ChiefMate">
    <rdfs:comment>ChiefMate is the Position attribute of an 

individual who is a ship's deck officer second in command below captain 

on a commercial vessel (i.e., MerchantMarineShip).</rdfs:comment>
    <rdfs:label>chief mate</rdfs:label>
    <rdfs:label>first mate</rdfs:label>
  </SUMO:Position>

  <Transportation:TransitwayState rdf:about="#ClosedForAllTraffic"/>
  <Transportation:TransportationSystem rdf:about="#DefenseTransportationSystem">
    <rdfs:comment>DefenseTransportationSystem 

is a worldwide transportation infrastructure used by the U.S. Department of 

Defense to move personnel and materials.  DTS comprises both military-owned 

transportation systems and commercial transit facilities under contract to 

the U.S. military or DOD.</rdfs:comment>
  </Transportation:TransportationSystem>

  <Mid-level-ontology:DeviceStateAttribute rdf:about="#DeviceClosed">
    <rdf:type rdf:resource="&SUMO;RelationalAttribute"/>
  </Mid-level-ontology:DeviceStateAttribute>

  <Mid-level-ontology:DeviceStateAttribute rdf:about="#DeviceOff">
    <rdf:type rdf:resource="&SUMO;InternalAttribute"/>
  </Mid-level-ontology:DeviceStateAttribute>

  <Mid-level-ontology:DeviceStateAttribute rdf:about="#DeviceOn">
    <SUMO:contraryAttribute rdf:resource="&Mid-level-ontology;DeviceOff"/>
    <rdf:type rdf:resource="&SUMO;InternalAttribute"/>
  </Mid-level-ontology:DeviceStateAttribute>

  <Mid-level-ontology:DeviceStateAttribute rdf:about="#DeviceOpen">
    <SUMO:contraryAttribute rdf:resource="&Mid-level-ontology;DeviceClosed"/>
    <rdf:type rdf:resource="&SUMO;RelationalAttribute"/>
  </Mid-level-ontology:DeviceStateAttribute>

  <Transportation:TrackGauge rdf:about="#DualGauge">
    <rdfs:comment>DualGauge is the attribute of  

any Railway that has three parallel rails, thus allowing 

two different gauges of rolling stock to travel over it.</rdfs:comment>
  </Transportation:TrackGauge>

  <Transportation:VehicleClassForFHWA rdf:about="#FHWAVehicleClass3">
    <rdfs:comment>FHWAVehicleClass3 designates Vehicle 

Class 3 of the UnitedStatesFederalHighwayAdministration, which includes 

all two-axle, four-tire single unit Vehicles other than PassengerCars.  

Examples: SUVs and 4-wheel pickup trucks.</rdfs:comment>
  </Transportation:VehicleClassForFHWA>

  <SUMO:GovernmentOrganization rdf:about="#FederalAviationAdministration">
    <SUMO:subOrganization rdf:resource="#UnitedStatesDepartmentOfTransportation"/>
    <rdfs:comment>The FederalAviationAdministration is the part of the 

UnitedStatesDepartmentOfTransportation that is responsible for the 

safety of civilian aviation in the United States.</rdfs:comment>
  </SUMO:GovernmentOrganization>

  <SUMO:GovernmentOrganization rdf:about="#FederalHighwayAdministration">
    <SUMO:subOrganization rdf:resource="#UnitedStatesDepartmentOfTransportation"/>
    <rdfs:comment>FederalHighwayAdministration 

is the part of the UnitedStatesDepartmentOfTransportation whose goal is 

to develop and maintain the Federal highway system of the United States, to 

assist U.S. states in development and maintenance of their highway systems, 

to protect the environment where highways intersect with it, and to provide 

access to Federal lands.</rdfs:comment>
  </SUMO:GovernmentOrganization>

  <SUMO:GovernmentOrganization rdf:about="#FederalRailroadAdministration">
    <SUMO:subOrganization rdf:resource="#UnitedStatesDepartmentOfTransportation"/>
    <rdfs:comment>The FederalRailroadAdministration is the part of the 

UnitedStatesDepartmentOfTransportation that is responsible for the 

safety and environmental impact of railroad travel in the United States.</rdfs:comment>
  </SUMO:GovernmentOrganization>

  <Mid-level-ontology:InternationalLaw rdf:about="#HagueRules">
    <rdfs:comment>The HagueRules are rules applicable to 

transportation of cargo that specify the duties of owners and shippers. 

The rules were published in 1924 after an international convention and 

subsequently made into law by many maritime nations.</rdfs:comment>
  </Mid-level-ontology:InternationalLaw>

  <Mid-level-ontology:InternationalLaw rdf:about="#HagueVisbyRules">
    <rdfs:comment>The HagueVisbyRules are an amendment 

to the HagueRules.  They were published in 1968.</rdfs:comment>
  </Mid-level-ontology:InternationalLaw>

  <SUMO:Obligation rdf:about="#HamburgRules">
    <rdfs:comment>The HamburgRules are rules concerned with 

cargo owner and carriers that may be incorporated into contracts for sea 

transportation of goods.  Adopted by UNCCGS in 1978.</rdfs:comment>
  </SUMO:Obligation>

  <SUMO:Position rdf:about="#Helmsman">
    <rdfs:comment>Helmsman is the Position attribute of an 

individual who is qualified at Steering a vessel.</rdfs:comment>
  </SUMO:Position>

  <Transportation:MovingViolation rdf:about="#IllegalTurn"/>
  <SUMO:PositionalAttribute rdf:about="#LengthwiseEquidistant">
    <rdfs:comment>LengthwiseEquidistant is the 

PositionalAttribute that describes things that are equidistant from one 

another along their length.  Unlike its specialization, Parallel, 

LengthwiseEquidistant allows for the objects to have curved lengths 

or edges.</rdfs:comment>
  </SUMO:PositionalAttribute>

  <Transportation:CIAAirportLengthClassification rdf:about="#LongRunwayAirport">
    <rdfs:comment>LongRunwayAirport is a CIA 

category for Airports whose longest runway has a length between  

2,438 meters and 3,047 meters, inclusive.</rdfs:comment>
  </Transportation:CIAAirportLengthClassification>

  <SUMO:GovernmentOrganization rdf:about="#MaritimeAdministration">
    <SUMO:subOrganization rdf:resource="#UnitedStatesDepartmentOfTransportation"/>
    <rdfs:comment>MaritimeAdministration is the 

United States government agency that administers the laws for maintaining 

the U.S. MerchantMarine.  The goals of the MaritimeAdministration are 

to support U.S. National Security, Shipbuilding, Intermodalism, and Trade.</rdfs:comment>
  </SUMO:GovernmentOrganization>

  <Transportation:CIAAirportLengthClassification rdf:about="#MediumLengthRunwayAirport">
    <rdfs:comment>MediumLengthRunwayAirport is a 

CIA category for Airports whose longest runway has a length between  

1,524 meters and 2,437 meters, inclusive.</rdfs:comment>
  </Transportation:CIAAirportLengthClassification>

  <Transportation:TrackGauge rdf:about="#NarrowGauge">
    <rdfs:comment>NarrowGauge is the attribute  

of any Railway that has a TrackGauge narrower than 

StandardGauge.  There are several common track widths 

among NarrowGauge railways.</rdfs:comment>
  </Transportation:TrackGauge>

  <Mid-level-ontology:Waterway rdf:about="#NorthernSeaRoute"
                               rdfs:label="Northern Sea Route">
    <SUMO:geographicSubregion rdf:resource="http://reliant.teknowledge.com/DAML/Geography.owl#ArcticOcean"/>
    <SUMO:geographicSubregion rdf:resource="http://reliant.teknowledge.com/DAML/Geography.owl#EasternHemisphere"/>
    <rdfs:comment>NorthernSeaRoute represents the 

seasonal waterway in the ArcticOcean adjacent to Russia and 

Norway.</rdfs:comment>
  </Mid-level-ontology:Waterway>

  <Mid-level-ontology:Waterway rdf:about="#NorthwestPassage"
                               rdfs:label="Northwest Passage">
    <SUMO:geographicSubregion rdf:resource="http://reliant.teknowledge.com/DAML/Geography.owl#ArcticOcean"/>
    <SUMO:geographicSubregion rdf:resource="http://reliant.teknowledge.com/DAML/Geography.owl#WesternHemisphere"/>
    <rdfs:comment>NorthwestPassage represents the 

seasonal waterway in the ArcticOcean adjacent to Canada and the 

UnitedStates.</rdfs:comment>
  </Mid-level-ontology:Waterway>

  <SUMO:PositionalAttribute rdf:about="#Parallel">
    <SUMO:subAttribute rdf:resource="#LengthwiseEquidistant"/>
    <rdfs:comment>Parallel is the PositionalAttribute that 

describes things that are parallel to one another, i.e., they are 

LengthwiseEquidistant along a straight length or edge.</rdfs:comment>
  </SUMO:PositionalAttribute>

  <SUMO:TextureAttribute rdf:about="#Paved">
    <rdfs:comment>Paved is the TextureAttribute that applies to 

LandTransitway surfaces that are paved.</rdfs:comment>
  </SUMO:TextureAttribute>

  <SUMO:Position rdf:about="#RadioOperator">
    <rdfs:comment>RadioOperator is the Position attribute 

of a person who is qualified to operate a TwoWayRadio.</rdfs:comment>
  </SUMO:Position>

  <SUMO:TextureAttribute rdf:about="#RoughSurface">
    <rdfs:comment>RoughSurface is the TextureAttribute 

that represents a rough-textured surface of an Object.</rdfs:comment>
  </SUMO:TextureAttribute>

  <SUMO:Position rdf:about="#ShipMaster">
    <rdfs:comment>ShipMaster is the class of persons who are 

licensed to command a commercial vessel (i.e., MerchantMarineShip).</rdfs:comment>
    <rdfs:label>captain</rdfs:label>
    <rdfs:label>master</rdfs:label>
  </SUMO:Position>

  <SUMO:Position rdf:about="#ShipNavigator">
    <rdfs:comment>ShipNavigator is the Position 

of the person who determines the course and position of an individual 

Watercraft, usually while on board, in order to guide its movements, the 

execution of which may be carried out by the captain, skipper, or helm.</rdfs:comment>
  </SUMO:Position>

  <SUMO:Position rdf:about="#ShipPilot">
    <rdfs:comment>ShipPilot is the Position attribute of an 

individual who is qualified (and usually licensed) to guide ships in and 

out of a specified Harbor or WaterArea, such as a River.  Contrast 

with Helmsman.</rdfs:comment>
  </SUMO:Position>

  <Transportation:CIAAirportLengthClassification rdf:about="#ShortRunwayAirport">
    <rdfs:comment>ShortRunwayAirport is a CIA 

category for Airports whose longest runway has a length between 914 

meters and 1523 meters, inclusive.</rdfs:comment>
  </Transportation:CIAAirportLengthClassification>

  <SUMO:TextureAttribute rdf:about="#SmoothSurface">
    <rdfs:comment>SmoothSurface is the TextureAttribute 

that represents a smooth-textured surface of an Object.</rdfs:comment>
  </SUMO:TextureAttribute>

  <Transportation:MovingViolation rdf:about="#Speeding"/>
  <Transportation:TrackGauge rdf:about="#StandardGauge">
    <rdfs:comment>StandardGauge is the attribute  

of Railways having the standardized track width that is 

used in North America and most Western European countries.  

The standard is typically a distance of 4 ft., 8 and one-half 

inches (1.44 meters). There is some variation within which usage is 

compatible, e.g., 1.35 meters. Standard gauge originated in 

England and was mandated by the U.S. Federal government for the 

U.S. Transcontinental Railroad.  It is also used in Canada, 

Great Britain, and most of Western Europe (but not in Ireland, 

or Spain and Portugal.</rdfs:comment>
  </Transportation:TrackGauge>

  <Transportation:MovingViolation rdf:about="#TooFastForConditions"/>
  <Government:InternationalOrganization rdf:about="#UnitedNationsConventionOnTheCarriageOfGoodsBySea">
    <SUMO:subOrganization rdf:resource="&Government;UnitedNations"/>
    <rdfs:label>United Nations Convention on the Carriage of Goods by Sea</rdfs:label>
  </Government:InternationalOrganization>

  <Transportation:DepartmentOfTransportation rdf:about="#UnitedStatesDepartmentOfTransportation">
    <rdfs:comment>UnitedStatesDepartmentOfTransportation represents the cabinet-level 

executive department of the U.S. Government that is charged with 

developing and coordinating national transportation policies including 

highway, railway, airway, and maritime transportation, with consideration 

for economic needs, ecological impact, and national defense.</rdfs:comment>
  </Transportation:DepartmentOfTransportation>

  <SUMO:GovernmentOrganization rdf:about="#UnitedStatesPassportAgency">
    <SUMO:located rdf:resource="&Mid-level-ontology;WashingtonDC"/>
    <rdfs:comment>UnitedStatesPassportAgency is 

the U.S. government agency that issues Passports.</rdfs:comment>
  </SUMO:GovernmentOrganization>

  <SUMO:TextureAttribute rdf:about="#Unpaved">
    <rdfs:comment>Unpaved is the TextureAttribute that applies 

to LandTransitway surfaces that are unpaved.</rdfs:comment>
  </SUMO:TextureAttribute>

  <Transportation:CIAAirportLengthClassification rdf:about="#VeryLongRunwayAirport">
    <rdfs:comment>VeryLongRunwayAirport is a CIA 

category for Airports whose longest runway has a length greater 

than 3,047 meters.</rdfs:comment>
  </Transportation:CIAAirportLengthClassification>

  <Transportation:CIAAirportLengthClassification rdf:about="#VeryShortRunwayAirport">
    <rdfs:comment>VeryShortRunwayAirport is a CIA 

category for Airports whose longest runway is less than 914 meters 

long.</rdfs:comment>
  </Transportation:CIAAirportLengthClassification>

  <owl:Thing rdf:about="http://reliant.teknowledge.com/DAML/Geography.owl#ArcticOcean"/>
  <owl:Thing rdf:about="http://reliant.teknowledge.com/DAML/Geography.owl#EasternHemisphere"/>
  <owl:Thing rdf:about="http://reliant.teknowledge.com/DAML/Geography.owl#WesternHemisphere"/>
  <owl:Thing rdf:about="&Government;UnitedNations"/>
  <SUMO:RelationalAttribute rdf:about="&Mid-level-ontology;ContainerEmpty">
    <rdfs:comment>ContainerEmpty is the Attribute of a 

Container that is empty.</rdfs:comment>
  </SUMO:RelationalAttribute>

  <SUMO:RelationalAttribute rdf:about="&Mid-level-ontology;ContainerFull">
    <rdfs:comment>ContainerFull is the Attribute of a 

Container that is full to capacity.</rdfs:comment>
  </SUMO:RelationalAttribute>

  <owl:Thing rdf:about="&Mid-level-ontology;DeviceClosed"/>
  <owl:Thing rdf:about="&Mid-level-ontology;DeviceOff"/>
  <owl:Thing rdf:about="&Mid-level-ontology;WashingtonDC"/>
  <owl:Thing rdf:about="&SUMO;Process"/>
  <SUMO:DeonticAttribute rdf:about="&SUMO;Prohibition">
    <rdfs:comment>Prohibition is the DeonticAttribute that 

applies to Formulas that an Agent is forbidden, by some authority, 

to make true.</rdfs:comment>
  </SUMO:DeonticAttribute>
</rdf:RDF>
